<?xml version="1.0"?>
<rdf:RDF xmlns="http://ethon.consensys.net/"
     xml:base="http://ethon.consensys.net/"
     xmlns:rdf="http://www.w3.org/1999/02/22-rdf-syntax-ns#"
     xmlns:ns="http://www.w3.org/2003/06/sw-vocab-status/ns#"
     xmlns:owl="http://www.w3.org/2002/07/owl#"
     xmlns:xml="http://www.w3.org/XML/1998/namespace"
     xmlns:swrlb="http://www.w3.org/2003/11/swrlb#"
     xmlns:swrl="http://www.w3.org/2003/11/swrl#"
     xmlns:xsd="http://www.w3.org/2001/XMLSchema#"
     xmlns:rdfs="http://www.w3.org/2000/01/rdf-schema#"
     xmlns:vann="http://purl.org/vocab/vann/"
     xmlns:ethon="http://ethon.consensys.net/"
     xmlns:dc="http://purl.org/dc/elements/1.1/"
     xmlns:swrla="http://swrl.stanford.edu/ontologies/3.3/swrla.owl#">
    <owl:Ontology rdf:about="http://ethon.consensys.net/">
        <owl:versionIRI rdf:resource="http://ethon.consensys.net/0/"/>
        <owl:imports rdf:resource="http://www.w3.org/2003/06/sw-vocab-status/ns"/>
        <rdfs:seeAlso rdf:resource="https://github.com/ethereum/yellowpaper"/>
        <dc:contributor>Shahan Khatchadourian</dc:contributor>
        <dc:creator>Johannes Pfeffer</dc:creator>
        <ns:term_status>testing</ns:term_status>
        <rdfs:seeAlso rdf:resource="https://github.com/ethereum/wiki/wiki/White-Paper"/>
        <dc:contributor>Joseph Chow</dc:contributor>
        <rdfs:comment xml:lang="en">The EthOn Ethereum ontology, described using W3C RDF Schema and the Web Ontology Language. It is closely aligned with Gavin Wood&apos;s Ethereum yellow paper.</rdfs:comment>
        <dc:contributor>Casey Detrio</dc:contributor>
        <dc:contributor>Maurycy Pietrzak</dc:contributor>
        <dc:contributor>Alex Beregszazi</dc:contributor>
        <rdfs:seeAlso rdf:resource="https://github.com/ConsenSys/EthOn"/>
        <dc:title>EthOn - An Ethereum Ontology</dc:title>
        <dc:contributor>Herman Junge</dc:contributor>
        <owl:versionInfo>0.2</owl:versionInfo>
        <vann:preferredNamespacePrefix>ethon</vann:preferredNamespacePrefix>
        <dc:contributor>Stefano Bertolo</dc:contributor>
        <dc:contributor>Marian Oancea</dc:contributor>
        <dc:contributor>William E Bodell III</dc:contributor>
    </owl:Ontology>



    <!--
    ///////////////////////////////////////////////////////////////////////////////////////
    //
    // Annotation properties
    //
    ///////////////////////////////////////////////////////////////////////////////////////
     -->




    <!-- http://ethon.consensys.net/DASE_RULE -->

    <owl:AnnotationProperty rdf:about="http://ethon.consensys.net/DASE_RULE"/>



    <!-- http://ethon.consensys.net/EthOnAnnotationProperty -->

    <owl:AnnotationProperty rdf:about="http://ethon.consensys.net/EthOnAnnotationProperty">
        <rdfs:comment xml:lang="en">Superclass of all EthOn specific annotation properties.</rdfs:comment>
        <ns:term_status>unstable</ns:term_status>
    </owl:AnnotationProperty>



    <!-- http://ethon.consensys.net/simpleDefinition -->

    <owl:AnnotationProperty rdf:about="http://ethon.consensys.net/simpleDefinition">
        <rdfs:comment>This property relates an EthOn concept to a definition in Simple English, intended especially for non-technical users.</rdfs:comment>
        <ns:term_status>unstable</ns:term_status>
        <rdfs:subPropertyOf rdf:resource="http://ethon.consensys.net/EthOnAnnotationProperty"/>
        <rdfs:domain rdf:resource="http://ethon.consensys.net/EthOnConcept"/>
    </owl:AnnotationProperty>



    <!-- http://ethon.consensys.net/suggestedStringRepresentation -->

    <owl:AnnotationProperty rdf:about="http://ethon.consensys.net/suggestedStringRepresentation">
        <rdfs:comment xml:lang="en">This property relates an EthOn concept with a suggested string representation. It can be used to give the term a name, e.g. in program code.</rdfs:comment>
        <ns:term_status>unstable</ns:term_status>
        <rdfs:subPropertyOf rdf:resource="http://ethon.consensys.net/EthOnAnnotationProperty"/>
        <rdfs:domain rdf:resource="http://ethon.consensys.net/EthOnConcept"/>
    </owl:AnnotationProperty>



    <!-- http://swrl.stanford.edu/ontologies/3.3/swrla.owl#isRuleEnabled -->

    <owl:AnnotationProperty rdf:about="http://swrl.stanford.edu/ontologies/3.3/swrla.owl#isRuleEnabled"/>



    <!--
    ///////////////////////////////////////////////////////////////////////////////////////
    //
    // Object Properties
    //
    ///////////////////////////////////////////////////////////////////////////////////////
     -->




    <!-- http://ethon.consensys.net/AccountObjectProperty -->

    <owl:ObjectProperty rdf:about="http://ethon.consensys.net/AccountObjectProperty">
        <rdfs:subPropertyOf rdf:resource="http://ethon.consensys.net/EthOnObjectProperty"/>
        <rdfs:comment xml:lang="en">Groups all EthOn account object properties</rdfs:comment>
        <rdfs:label xml:lang="en">EthOn Account Object Property</rdfs:label>
        <ns:term_status>unstable</ns:term_status>
    </owl:ObjectProperty>



    <!-- http://ethon.consensys.net/BlockObjectProperty -->

    <owl:ObjectProperty rdf:about="http://ethon.consensys.net/BlockObjectProperty">
        <rdfs:subPropertyOf rdf:resource="http://ethon.consensys.net/EthOnObjectProperty"/>
        <rdfs:comment xml:lang="en">Groups all EthOn block object properties</rdfs:comment>
        <rdfs:label xml:lang="en">EthOn Block Object Property</rdfs:label>
        <ns:term_status>unstable</ns:term_status>
    </owl:ObjectProperty>



    <!-- http://ethon.consensys.net/EthOnObjectProperty -->

    <owl:ObjectProperty rdf:about="http://ethon.consensys.net/EthOnObjectProperty">
        <rdfs:comment xml:lang="en">Groups all EthOn object properties</rdfs:comment>
        <rdfs:label xml:lang="en">EthOn Object Property</rdfs:label>
        <ns:term_status>unstable</ns:term_status>
    </owl:ObjectProperty>



    <!-- http://ethon.consensys.net/MessageObjectProperty -->

    <owl:ObjectProperty rdf:about="http://ethon.consensys.net/MessageObjectProperty">
        <rdfs:subPropertyOf rdf:resource="http://ethon.consensys.net/EthOnObjectProperty"/>
        <rdfs:comment xml:lang="en">Groups all EthOn message object properties.</rdfs:comment>
        <rdfs:label xml:lang="en">EthOn Message Object Property</rdfs:label>
        <ns:term_status>unstable</ns:term_status>
    </owl:ObjectProperty>



    <!-- http://ethon.consensys.net/NetworkObjectProperty -->

    <owl:ObjectProperty rdf:about="http://ethon.consensys.net/NetworkObjectProperty">
        <rdfs:subPropertyOf rdf:resource="http://ethon.consensys.net/EthOnObjectProperty"/>
        <rdfs:comment xml:lang="en">Groups all EthOn network object properties.</rdfs:comment>
        <rdfs:label xml:lang="en">EthOn Network Object Property</rdfs:label>
        <ns:term_status>unstable</ns:term_status>
    </owl:ObjectProperty>



    <!-- http://ethon.consensys.net/StateObjectProperty -->

    <owl:ObjectProperty rdf:about="http://ethon.consensys.net/StateObjectProperty">
        <rdfs:subPropertyOf rdf:resource="http://ethon.consensys.net/EthOnObjectProperty"/>
        <rdfs:comment xml:lang="en">Groups all EthOn state object properties.</rdfs:comment>
        <rdfs:label xml:lang="en">EthOn State Object Property</rdfs:label>
        <ns:term_status>unstable</ns:term_status>
    </owl:ObjectProperty>



    <!-- http://ethon.consensys.net/conformsTo -->

    <owl:ObjectProperty rdf:about="http://ethon.consensys.net/conformsTo">
        <rdfs:subPropertyOf rdf:resource="http://ethon.consensys.net/NetworkObjectProperty"/>
        <rdfs:domain rdf:resource="http://ethon.consensys.net/EthOnConcept"/>
        <suggestedStringRepresentation>conformsTo</suggestedStringRepresentation>
        <rdfs:comment xml:lang="en">Relates an Ethereum concept to the Ethereum protocol variant it conforms to.</rdfs:comment>
        <rdfs:label>conforms to</rdfs:label>
        <ns:term_status>unstable</ns:term_status>
    </owl:ObjectProperty>



    <!-- http://ethon.consensys.net/containsTx -->

    <owl:ObjectProperty rdf:about="http://ethon.consensys.net/containsTx">
        <rdfs:subPropertyOf rdf:resource="http://ethon.consensys.net/BlockObjectProperty"/>
        <rdf:type rdf:resource="http://www.w3.org/2002/07/owl#InverseFunctionalProperty"/>
        <rdfs:domain rdf:resource="http://ethon.consensys.net/Block"/>
        <rdfs:range rdf:resource="http://ethon.consensys.net/Tx"/>
        <suggestedStringRepresentation>containsTx</suggestedStringRepresentation>
        <rdfs:comment xml:lang="en">Relates a block to a transaction included in it. All containsTx relations of a block comprise the block&apos;s transaction list. The order of the transactions is determined by their index value. The property is inverse functional because a transaction can only be included in one block.</rdfs:comment>
        <rdfs:label xml:lang="en">contains Transaction</rdfs:label>
        <ns:term_status>unstable</ns:term_status>
    </owl:ObjectProperty>



    <!-- http://ethon.consensys.net/controlsAccount -->

    <owl:ObjectProperty rdf:about="http://ethon.consensys.net/controlsAccount">
        <rdfs:subPropertyOf rdf:resource="http://ethon.consensys.net/AccountObjectProperty"/>
        <rdfs:domain rdf:resource="http://ethon.consensys.net/ExternalActor"/>
        <rdfs:range rdf:resource="http://ethon.consensys.net/Account"/>
        <suggestedStringRepresentation>controlsAccount</suggestedStringRepresentation>
        <rdfs:comment xml:lang="en">This property connects an External Actor an Account that it controls. This means the External Actor has control over the private Key for the Account. The control is not necessarily legitimate.</rdfs:comment>
        <rdfs:label xml:lang="en">controls Account</rdfs:label>
        <ns:term_status>unstable</ns:term_status>
    </owl:ObjectProperty>



    <!-- http://ethon.consensys.net/creates -->

    <owl:ObjectProperty rdf:about="http://ethon.consensys.net/creates">
        <rdfs:subPropertyOf rdf:resource="http://ethon.consensys.net/to"/>
        <rdfs:domain>
            <owl:Class>
                <owl:unionOf rdf:parseType="Collection">
                    <rdf:Description rdf:about="http://ethon.consensys.net/CreateContractMsg"/>
                    <rdf:Description rdf:about="http://ethon.consensys.net/CreateTx"/>
                </owl:unionOf>
            </owl:Class>
        </rdfs:domain>
        <rdfs:range rdf:resource="http://ethon.consensys.net/ContractAccount"/>
        <suggestedStringRepresentation>creates</suggestedStringRepresentation>
        <rdfs:comment xml:lang="en">Relates a create transaction to the contract account it creates.</rdfs:comment>
        <rdfs:label xml:lang="en">creates</rdfs:label>
        <ns:term_status>unstable</ns:term_status>
    </owl:ObjectProperty>



    <!-- http://ethon.consensys.net/createsPostBlockState -->

    <owl:ObjectProperty rdf:about="http://ethon.consensys.net/createsPostBlockState">
        <rdfs:subPropertyOf rdf:resource="http://ethon.consensys.net/createsState"/>
        <rdf:type rdf:resource="http://www.w3.org/2002/07/owl#FunctionalProperty"/>
        <rdf:type rdf:resource="http://www.w3.org/2002/07/owl#InverseFunctionalProperty"/>
        <rdfs:domain rdf:resource="http://ethon.consensys.net/Block"/>
        <rdfs:range rdf:resource="http://ethon.consensys.net/WorldState"/>
        <suggestedStringRepresentation>createsPostBlockState</suggestedStringRepresentation>
        <rdfs:comment xml:lang="en">Relates a block to the global state of the system after all transactions in the block have been executed.</rdfs:comment>
        <rdfs:label xml:lang="en">creates post Block execution State</rdfs:label>
        <ns:term_status>unstable</ns:term_status>
    </owl:ObjectProperty>



    <!-- http://ethon.consensys.net/createsPostMsgState -->

    <owl:ObjectProperty rdf:about="http://ethon.consensys.net/createsPostMsgState">
        <rdfs:subPropertyOf rdf:resource="http://ethon.consensys.net/createsState"/>
        <rdf:type rdf:resource="http://www.w3.org/2002/07/owl#FunctionalProperty"/>
        <rdfs:comment>Relates a message to the global state of the system after all the message has been executed.</rdfs:comment>
        <rdfs:label>creates post Message execution State</rdfs:label>
        <ns:term_status>unstable</ns:term_status>
    </owl:ObjectProperty>



    <!-- http://ethon.consensys.net/createsPostTxState -->

    <owl:ObjectProperty rdf:about="http://ethon.consensys.net/createsPostTxState">
        <rdfs:subPropertyOf rdf:resource="http://ethon.consensys.net/createsState"/>
        <rdf:type rdf:resource="http://www.w3.org/2002/07/owl#FunctionalProperty"/>
        <rdfs:domain rdf:resource="http://ethon.consensys.net/Tx"/>
        <rdfs:range rdf:resource="http://ethon.consensys.net/WorldState"/>
        <suggestedStringRepresentation>createsPostTxState</suggestedStringRepresentation>
        <rdfs:comment xml:lang="en">Relates a transaction to the global state of the system after the transaction has been executed.</rdfs:comment>
        <rdfs:label xml:lang="en">creates post Transaction execution State</rdfs:label>
        <ns:term_status>unstable</ns:term_status>
    </owl:ObjectProperty>



    <!-- http://ethon.consensys.net/createsState -->

    <owl:ObjectProperty rdf:about="http://ethon.consensys.net/createsState">
        <rdfs:subPropertyOf rdf:resource="http://ethon.consensys.net/MessageObjectProperty"/>
        <rdfs:subPropertyOf rdf:resource="http://ethon.consensys.net/StateObjectProperty"/>
        <rdfs:domain rdf:resource="http://ethon.consensys.net/StateTransition"/>
        <rdfs:range rdf:resource="http://ethon.consensys.net/State"/>
        <suggestedStringRepresentation>createsState</suggestedStringRepresentation>
        <rdfs:comment xml:lang="en">Relates a transition to the state it creates.</rdfs:comment>
        <rdfs:label xml:lang="en">creates State</rdfs:label>
        <ns:term_status>unstable</ns:term_status>
    </owl:ObjectProperty>



    <!-- http://ethon.consensys.net/from -->

    <owl:ObjectProperty rdf:about="http://ethon.consensys.net/from">
        <rdfs:subPropertyOf rdf:resource="http://ethon.consensys.net/MessageObjectProperty"/>
        <suggestedStringRepresentation>fromAccount</suggestedStringRepresentation>
        <rdfs:comment xml:lang="en">Relates a message to the account it originates from.</rdfs:comment>
        <rdfs:label xml:lang="en">from</rdfs:label>
        <ns:term_status>unstable</ns:term_status>
    </owl:ObjectProperty>



    <!-- http://ethon.consensys.net/hasAccountStorage -->

    <owl:ObjectProperty rdf:about="http://ethon.consensys.net/hasAccountStorage">
        <rdfs:subPropertyOf rdf:resource="http://ethon.consensys.net/AccountObjectProperty"/>
        <rdf:type rdf:resource="http://www.w3.org/2002/07/owl#FunctionalProperty"/>
        <rdf:type rdf:resource="http://www.w3.org/2002/07/owl#InverseFunctionalProperty"/>
        <rdfs:range rdf:resource="http://ethon.consensys.net/AccountStorage"/>
        <suggestedStringRepresentation>hasAccountStorage</suggestedStringRepresentation>
        <rdfs:comment xml:lang="en">Relates an account to the Merkle Patricia tree that encodes its storage contents at a certain account state. This property is Functional because an account state can have only one instance of account storage and inverse functional because an account storage can have only one associated account state.</rdfs:comment>
        <rdfs:label xml:lang="en">has Account Storage</rdfs:label>
        <ns:term_status>unstable</ns:term_status>
    </owl:ObjectProperty>



    <!-- http://ethon.consensys.net/hasBeneficiary -->

    <owl:ObjectProperty rdf:about="http://ethon.consensys.net/hasBeneficiary">
        <rdfs:subPropertyOf rdf:resource="http://ethon.consensys.net/BlockObjectProperty"/>
        <rdf:type rdf:resource="http://www.w3.org/2002/07/owl#FunctionalProperty"/>
        <rdfs:domain rdf:resource="http://ethon.consensys.net/Block"/>
        <rdfs:range rdf:resource="http://ethon.consensys.net/Account"/>
        <suggestedStringRepresentation>hasBeneficiary</suggestedStringRepresentation>
        <rdfs:comment xml:lang="en">Relates a block to the account to which all fees collected from the successful mining of this block are transferred.</rdfs:comment>
        <rdfs:label xml:lang="en">has beneficiary</rdfs:label>
        <ns:term_status>unstable</ns:term_status>
    </owl:ObjectProperty>



    <!-- http://ethon.consensys.net/hasCurrentState -->

    <owl:ObjectProperty rdf:about="http://ethon.consensys.net/hasCurrentState">
        <rdfs:subPropertyOf rdf:resource="http://ethon.consensys.net/hasState"/>
        <rdf:type rdf:resource="http://www.w3.org/2002/07/owl#InverseFunctionalProperty"/>
        <rdfs:domain rdf:resource="http://ethon.consensys.net/Account"/>
        <rdfs:range rdf:resource="http://ethon.consensys.net/AccountState"/>
        <suggestedStringRepresentation>hasCurrentState</suggestedStringRepresentation>
        <rdfs:comment>This property relates an EthOn concept to its most current state.</rdfs:comment>
        <rdfs:label>has current State</rdfs:label>
        <ns:term_status>unstable</ns:term_status>
    </owl:ObjectProperty>



    <!-- http://ethon.consensys.net/hasFork -->

    <owl:ObjectProperty rdf:about="http://ethon.consensys.net/hasFork">
        <rdfs:subPropertyOf rdf:resource="http://ethon.consensys.net/NetworkObjectProperty"/>
        <rdf:type rdf:resource="http://www.w3.org/2002/07/owl#TransitiveProperty"/>
        <rdfs:domain rdf:resource="http://ethon.consensys.net/Blockchain"/>
        <rdfs:range rdf:resource="http://ethon.consensys.net/Blockchain"/>
        <suggestedStringRepresentation>hasFork</suggestedStringRepresentation>
        <rdfs:comment xml:lang="en">Relates a blockchain to a forked version of it. It is inverse functional because a forked blockchain can have only one blockchain it forked from. It is transitive because if a blockchain C that was forked from blockchain B that in turn was forked from blockchain A, blockchain C was also forked from blockchain A. It is asymetric because if blockchain A is forked from blockchain B, B cannot be also forked from A. It is irreflexive because a blockchain cannot be a fork of itself.</rdfs:comment>
        <rdfs:label xml:lang="en">has Fork</rdfs:label>
        <ns:term_status>unstable</ns:term_status>
    </owl:ObjectProperty>



    <!-- http://ethon.consensys.net/hasLogEntry -->

    <owl:ObjectProperty rdf:about="http://ethon.consensys.net/hasLogEntry">
        <rdfs:subPropertyOf rdf:resource="http://ethon.consensys.net/MessageObjectProperty"/>
        <rdfs:domain rdf:resource="http://ethon.consensys.net/Tx"/>
        <rdfs:range rdf:resource="http://ethon.consensys.net/LogEntry"/>
        <suggestedStringRepresentation>hasLogEntry</suggestedStringRepresentation>
        <rdfs:comment xml:lang="en">Relates a transaction to a log entry it creates.</rdfs:comment>
        <rdfs:label xml:lang="en">has Log Entry</rdfs:label>
        <ns:term_status>unstable</ns:term_status>
    </owl:ObjectProperty>



    <!-- http://ethon.consensys.net/hasLogTopic -->

    <owl:ObjectProperty rdf:about="http://ethon.consensys.net/hasLogTopic">
        <rdfs:subPropertyOf rdf:resource="http://ethon.consensys.net/MessageObjectProperty"/>
        <rdfs:domain rdf:resource="http://ethon.consensys.net/LogEntry"/>
        <rdfs:range rdf:resource="http://ethon.consensys.net/LogTopic"/>
        <suggestedStringRepresentation>hasLogTopic</suggestedStringRepresentation>
        <rdfs:comment xml:lang="en">Relates a log entry to a log topic.</rdfs:comment>
        <rdfs:label xml:lang="en">has Log Topic</rdfs:label>
        <ns:term_status>unstable</ns:term_status>
    </owl:ObjectProperty>



    <!-- http://ethon.consensys.net/hasOriginatorTx -->

    <owl:ObjectProperty rdf:about="http://ethon.consensys.net/hasOriginatorTx">
        <rdfs:subPropertyOf rdf:resource="http://ethon.consensys.net/MessageObjectProperty"/>
        <rdf:type rdf:resource="http://www.w3.org/2002/07/owl#InverseFunctionalProperty"/>
        <rdfs:domain rdf:resource="http://ethon.consensys.net/ContractMsg"/>
        <rdfs:range rdf:resource="http://ethon.consensys.net/Tx"/>
        <suggestedStringRepresentation>hasOriginatorTx</suggestedStringRepresentation>
        <rdfs:comment xml:lang="en">Relates a contract message to the transaction it originated from.</rdfs:comment>
        <rdfs:label xml:lang="en">has Originator Transaction</rdfs:label>
        <ns:term_status>unstable</ns:term_status>
    </owl:ObjectProperty>



    <!-- http://ethon.consensys.net/hasParentBlock -->

    <owl:ObjectProperty rdf:about="http://ethon.consensys.net/hasParentBlock">
        <rdfs:subPropertyOf rdf:resource="http://ethon.consensys.net/BlockObjectProperty"/>
        <rdf:type rdf:resource="http://www.w3.org/2002/07/owl#FunctionalProperty"/>
        <rdf:type rdf:resource="http://www.w3.org/2002/07/owl#AsymmetricProperty"/>
        <rdf:type rdf:resource="http://www.w3.org/2002/07/owl#IrreflexiveProperty"/>
        <rdfs:domain rdf:resource="http://ethon.consensys.net/Block"/>
        <rdfs:range rdf:resource="http://ethon.consensys.net/Block"/>
        <suggestedStringRepresentation>hasParentBlock</suggestedStringRepresentation>
        <rdfs:comment xml:lang="en">Relates a block to its parent in the chain. It always points to the block with a number that is decreased by one, compared to the block it originates from. The relation is asymmetric because if block A is parent to block B then block B can not be parent to block A. It is also irreflexive because a block cannot be parent to itself.</rdfs:comment>
        <rdfs:label xml:lang="en">has parent Block</rdfs:label>
        <ns:term_status>unstable</ns:term_status>
    </owl:ObjectProperty>



    <!-- http://ethon.consensys.net/hasReceipt -->

    <owl:ObjectProperty rdf:about="http://ethon.consensys.net/hasReceipt">
        <rdfs:subPropertyOf rdf:resource="http://ethon.consensys.net/MessageObjectProperty"/>
        <rdfs:domain rdf:resource="http://ethon.consensys.net/Tx"/>
        <rdfs:range rdf:resource="http://ethon.consensys.net/TxReceipt"/>
        <suggestedStringRepresentation>hasTransactionReceipt</suggestedStringRepresentation>
        <rdfs:comment xml:lang="en">Relates a transaction to its receipt.</rdfs:comment>
        <rdfs:label xml:lang="en">has transaction receipt</rdfs:label>
        <ns:term_status>unstable</ns:term_status>
    </owl:ObjectProperty>



    <!-- http://ethon.consensys.net/hasReceiptsTrie -->

    <owl:ObjectProperty rdf:about="http://ethon.consensys.net/hasReceiptsTrie">
        <rdfs:subPropertyOf rdf:resource="http://ethon.consensys.net/BlockObjectProperty"/>
        <rdf:type rdf:resource="http://www.w3.org/2002/07/owl#FunctionalProperty"/>
        <rdf:type rdf:resource="http://www.w3.org/2002/07/owl#InverseFunctionalProperty"/>
        <suggestedStringRepresentation>hasReceiptsTrie</suggestedStringRepresentation>
        <rdfs:comment xml:lang="en">Relates a block to the trie that contains the block&apos;s receipt data.</rdfs:comment>
        <rdfs:label xml:lang="en">has receipts trie</rdfs:label>
        <ns:term_status>unstable</ns:term_status>
    </owl:ObjectProperty>



    <!-- http://ethon.consensys.net/hasState -->

    <owl:ObjectProperty rdf:about="http://ethon.consensys.net/hasState">
        <rdfs:subPropertyOf rdf:resource="http://ethon.consensys.net/StateObjectProperty"/>
        <rdf:type rdf:resource="http://www.w3.org/2002/07/owl#InverseFunctionalProperty"/>
        <rdfs:domain rdf:resource="http://ethon.consensys.net/Account"/>
        <rdfs:range rdf:resource="http://ethon.consensys.net/AccountState"/>
        <suggestedStringRepresentation>hasState</suggestedStringRepresentation>
        <rdfs:comment xml:lang="en">This property relates an EthOn concept to a state. It is inverse functional because a state can only belong to one single EthOn concept.</rdfs:comment>
        <rdfs:label xml:lang="en">has state</rdfs:label>
        <ns:term_status>unstable</ns:term_status>
    </owl:ObjectProperty>



    <!-- http://ethon.consensys.net/hasTransition -->

    <owl:ObjectProperty rdf:about="http://ethon.consensys.net/hasTransition">
        <rdfs:subPropertyOf rdf:resource="http://ethon.consensys.net/StateObjectProperty"/>
        <suggestedStringRepresentation>hasTransition</suggestedStringRepresentation>
        <rdfs:comment xml:lang="en">Relates a state to a transition (i.e. a message) that creates a new state.</rdfs:comment>
        <rdfs:label xml:lang="en">has Transition</rdfs:label>
        <ns:term_status>unstable</ns:term_status>
    </owl:ObjectProperty>



    <!-- http://ethon.consensys.net/hasTxTrie -->

    <owl:ObjectProperty rdf:about="http://ethon.consensys.net/hasTxTrie">
        <rdfs:subPropertyOf rdf:resource="http://ethon.consensys.net/BlockObjectProperty"/>
        <rdf:type rdf:resource="http://www.w3.org/2002/07/owl#FunctionalProperty"/>
        <rdf:type rdf:resource="http://www.w3.org/2002/07/owl#InverseFunctionalProperty"/>
        <rdfs:domain rdf:resource="http://ethon.consensys.net/Block"/>
        <rdfs:range rdf:resource="http://ethon.consensys.net/TxTrie"/>
        <suggestedStringRepresentation>hasTxTrie</suggestedStringRepresentation>
        <rdfs:comment xml:lang="en">Relates a block to the trie that contains the data of the transactions contained in the block.</rdfs:comment>
        <rdfs:label xml:lang="en">has transactions trie</rdfs:label>
        <ns:term_status>unstable</ns:term_status>
    </owl:ObjectProperty>



    <!-- http://ethon.consensys.net/knowsOfUncle -->

    <owl:ObjectProperty rdf:about="http://ethon.consensys.net/knowsOfUncle">
        <rdfs:subPropertyOf rdf:resource="http://ethon.consensys.net/BlockObjectProperty"/>
        <suggestedStringRepresentation>knowsOfUncle</suggestedStringRepresentation>
        <rdfs:comment xml:lang="en">Relates a block to a known uncle.</rdfs:comment>
        <rdfs:label xml:lang="en">knows of Uncle</rdfs:label>
        <ns:term_status>unstable</ns:term_status>
    </owl:ObjectProperty>



    <!-- http://ethon.consensys.net/loggedBy -->

    <owl:ObjectProperty rdf:about="http://ethon.consensys.net/loggedBy">
        <rdfs:subPropertyOf rdf:resource="http://ethon.consensys.net/MessageObjectProperty"/>
        <rdfs:domain rdf:resource="http://ethon.consensys.net/LogEntry"/>
        <rdfs:range rdf:resource="http://ethon.consensys.net/Account"/>
        <suggestedStringRepresentation>loggedBy</suggestedStringRepresentation>
        <rdfs:comment xml:lang="en">Relates a log entry to the contract account that created the log when its code was executed.</rdfs:comment>
        <rdfs:label xml:lang="en">logged by</rdfs:label>
        <ns:term_status>unstable</ns:term_status>
    </owl:ObjectProperty>



    <!-- http://ethon.consensys.net/minesFor -->

    <owl:ObjectProperty rdf:about="http://ethon.consensys.net/minesFor">
        <rdfs:subPropertyOf rdf:resource="http://ethon.consensys.net/NetworkObjectProperty"/>
        <rdfs:domain rdf:resource="http://ethon.consensys.net/Node"/>
        <rdfs:range rdf:resource="http://ethon.consensys.net/Blockchain"/>
        <suggestedStringRepresentation>minesFor</suggestedStringRepresentation>
        <rdfs:comment xml:lang="en">Relates a mining node to the blockchain it mines for. Mining is the process of dedicating effort (working) to bolster one series of transactions (a block) over any other potential competitor block. It is achieved thanks to a cryptographically secure proof.</rdfs:comment>
        <rdfs:label xml:lang="en">mines for</rdfs:label>
        <ns:term_status>unstable</ns:term_status>
    </owl:ObjectProperty>



    <!-- http://ethon.consensys.net/nextBlockState -->

    <owl:ObjectProperty rdf:about="http://ethon.consensys.net/nextBlockState">
        <rdfs:subPropertyOf rdf:resource="http://ethon.consensys.net/nextTxState"/>
        <rdfs:domain rdf:resource="http://ethon.consensys.net/PostBlockState"/>
        <rdfs:range rdf:resource="http://ethon.consensys.net/PostBlockState"/>
        <suggestedStringRepresentation>nextBlockState</suggestedStringRepresentation>
        <rdfs:comment xml:lang="en">Relates a post block state to the following post block state.</rdfs:comment>
        <rdfs:label xml:lang="en">next Post Block State</rdfs:label>
        <ns:term_status>unstable</ns:term_status>
    </owl:ObjectProperty>



    <!-- http://ethon.consensys.net/nextMsgState -->

    <owl:ObjectProperty rdf:about="http://ethon.consensys.net/nextMsgState">
        <rdfs:subPropertyOf rdf:resource="http://ethon.consensys.net/nextState"/>
        <rdfs:domain rdf:resource="http://ethon.consensys.net/PostMsgState"/>
        <rdfs:range rdf:resource="http://ethon.consensys.net/PostMsgState"/>
        <suggestedStringRepresentation>nextMsgState</suggestedStringRepresentation>
        <rdfs:comment xml:lang="en">Relates a post message state to the following post message state.</rdfs:comment>
        <rdfs:label xml:lang="en">next Post Message State</rdfs:label>
        <ns:term_status>unstable</ns:term_status>
    </owl:ObjectProperty>



    <!-- http://ethon.consensys.net/nextState -->

    <owl:ObjectProperty rdf:about="http://ethon.consensys.net/nextState">
        <rdfs:subPropertyOf rdf:resource="http://ethon.consensys.net/StateObjectProperty"/>
        <rdfs:domain rdf:resource="http://ethon.consensys.net/WorldState"/>
        <rdfs:range rdf:resource="http://ethon.consensys.net/WorldState"/>
        <suggestedStringRepresentation>nextState</suggestedStringRepresentation>
        <rdfs:comment xml:lang="en">Relates a state to the following state. In EthOn the state transition system has no branches.</rdfs:comment>
        <rdfs:label xml:lang="en">next State</rdfs:label>
        <ns:term_status>unstable</ns:term_status>
    </owl:ObjectProperty>



    <!-- http://ethon.consensys.net/nextTxState -->

    <owl:ObjectProperty rdf:about="http://ethon.consensys.net/nextTxState">
        <rdfs:subPropertyOf rdf:resource="http://ethon.consensys.net/nextMsgState"/>
        <rdfs:domain rdf:resource="http://ethon.consensys.net/PostTxState"/>
        <rdfs:range rdf:resource="http://ethon.consensys.net/PostTxState"/>
        <suggestedStringRepresentation>nextTxState</suggestedStringRepresentation>
        <rdfs:comment xml:lang="en">Relates a post transaction state to the following post transaction state.</rdfs:comment>
        <rdfs:label xml:lang="en">next Post Transaction State</rdfs:label>
        <ns:term_status>unstable</ns:term_status>
    </owl:ObjectProperty>



    <!-- http://ethon.consensys.net/partOf -->

    <owl:ObjectProperty rdf:about="http://ethon.consensys.net/partOf">
        <rdfs:subPropertyOf rdf:resource="http://ethon.consensys.net/EthOnObjectProperty"/>
        <rdf:type rdf:resource="http://www.w3.org/2002/07/owl#TransitiveProperty"/>
        <suggestedStringRepresentation>partOf</suggestedStringRepresentation>
        <rdfs:comment xml:lang="en">This is a general relation to express part of relationships. The classic study of parts and wholes, mereology, has three axioms: 1. the part-of relation is Transitive - &quot;parts of parts are parts of the whole&quot; - If A is part of B and B is part of C, then A is part of C Reflexive - &quot;Everything is part of itself&quot; - A is part of A Antisymmetric - &quot;Nothing is a part of its parts&quot; - if A is part of B and A != B then B is not part of A.</rdfs:comment>
        <rdfs:label xml:lang="en">part of</rdfs:label>
        <rdfs:seeAlso rdf:resource="https://www.w3.org/2001/sw/BestPractices/OEP/SimplePartWhole/"/>
        <ns:term_status>testing</ns:term_status>
    </owl:ObjectProperty>



    <!-- http://ethon.consensys.net/refunds -->

    <owl:ObjectProperty rdf:about="http://ethon.consensys.net/refunds">
        <rdfs:subPropertyOf rdf:resource="http://ethon.consensys.net/to"/>
        <rdf:type rdf:resource="http://www.w3.org/2002/07/owl#FunctionalProperty"/>
        <rdfs:domain rdf:resource="http://ethon.consensys.net/ContractAccount"/>
        <rdfs:range rdf:resource="http://ethon.consensys.net/Account"/>
        <suggestedStringRepresentation>refunds</suggestedStringRepresentation>
        <rdfs:comment xml:lang="en">Relates a selfdestruct contract message to the contract account it sends its refund balance to.</rdfs:comment>
        <rdfs:label xml:lang="en">refunds</rdfs:label>
        <ns:term_status>unstable</ns:term_status>
    </owl:ObjectProperty>



    <!-- http://ethon.consensys.net/spawnsBlock -->

    <owl:ObjectProperty rdf:about="http://ethon.consensys.net/spawnsBlock">
        <rdfs:subPropertyOf rdf:resource="http://ethon.consensys.net/NetworkObjectProperty"/>
        <rdfs:domain rdf:resource="http://ethon.consensys.net/Node"/>
        <rdfs:range rdf:resource="http://ethon.consensys.net/Block"/>
        <suggestedStringRepresentation>spawnsBlock</suggestedStringRepresentation>
        <rdfs:comment xml:lang="en">Relates an Ethereum node to a valid block it has transmitted to the network. This does not specify the proofing algorithm (e.g. proof of work or proof of authority).</rdfs:comment>
        <rdfs:label>spawns Block</rdfs:label>
        <ns:term_status>unstable</ns:term_status>
    </owl:ObjectProperty>



    <!-- http://ethon.consensys.net/to -->

    <owl:ObjectProperty rdf:about="http://ethon.consensys.net/to">
        <rdfs:subPropertyOf rdf:resource="http://ethon.consensys.net/MessageObjectProperty"/>
        <rdfs:domain rdf:resource="http://ethon.consensys.net/Msg"/>
        <rdfs:range rdf:resource="http://ethon.consensys.net/Msg"/>
        <suggestedStringRepresentation>toAccount</suggestedStringRepresentation>
        <rdfs:comment xml:lang="en">Relates a message with the account it is sent to.</rdfs:comment>
        <rdfs:label xml:lang="en">to</rdfs:label>
        <ns:term_status>unstable</ns:term_status>
    </owl:ObjectProperty>



    <!-- http://ethon.consensys.net/triggersMsg -->

    <owl:ObjectProperty rdf:about="http://ethon.consensys.net/triggersMsg">
        <rdfs:subPropertyOf rdf:resource="http://ethon.consensys.net/MessageObjectProperty"/>
        <rdfs:domain>
            <owl:Class>
                <owl:unionOf rdf:parseType="Collection">
                    <rdf:Description rdf:about="http://ethon.consensys.net/CallContractMsg"/>
                    <rdf:Description rdf:about="http://ethon.consensys.net/CallTx"/>
                    <rdf:Description rdf:about="http://ethon.consensys.net/CreateContractMsg"/>
                    <rdf:Description rdf:about="http://ethon.consensys.net/CreateTx"/>
                </owl:unionOf>
            </owl:Class>
        </rdfs:domain>
        <rdfs:range rdf:resource="http://ethon.consensys.net/ContractMsg"/>
        <suggestedStringRepresentation>triggersMsg</suggestedStringRepresentation>
        <rdfs:comment xml:lang="en">Relates a message that was direct to a contract account to the contract messages that result from the call to the contract account. The chain of triggersMsg relations represents a call graph.</rdfs:comment>
        <rdfs:label xml:lang="en">triggers Contract Message</rdfs:label>
        <ns:term_status>unstable</ns:term_status>
    </owl:ObjectProperty>



    <!--
    ///////////////////////////////////////////////////////////////////////////////////////
    //
    // Data properties
    //
    ///////////////////////////////////////////////////////////////////////////////////////
     -->




    <!-- http://ethon.consensys.net/AccountDataProperty -->

    <owl:DatatypeProperty rdf:about="http://ethon.consensys.net/AccountDataProperty">
        <rdfs:subPropertyOf rdf:resource="http://ethon.consensys.net/EthOnDataProperty"/>
        <rdfs:domain rdf:resource="http://ethon.consensys.net/AccountConcept"/>
        <rdfs:comment xml:lang="en">Groups all data properties that are specific to an account.</rdfs:comment>
        <rdfs:label xml:lang="en">EthOn Account Data Property</rdfs:label>
        <ns:term_status>unstable</ns:term_status>
    </owl:DatatypeProperty>



    <!-- http://ethon.consensys.net/BlockDataProperty -->

    <owl:DatatypeProperty rdf:about="http://ethon.consensys.net/BlockDataProperty">
        <rdfs:subPropertyOf rdf:resource="http://ethon.consensys.net/EthOnDataProperty"/>
        <rdfs:domain rdf:resource="http://ethon.consensys.net/BlockConcept"/>
        <rdfs:comment xml:lang="en">Groups all data properties that are specific to a block. These properties are usually functional because a block can only be associated with a single instance of them.</rdfs:comment>
        <rdfs:label xml:lang="en">EthOn Block Data Property</rdfs:label>
        <ns:term_status>unstable</ns:term_status>
    </owl:DatatypeProperty>



    <!-- http://ethon.consensys.net/EthOnDataProperty -->

    <owl:DatatypeProperty rdf:about="http://ethon.consensys.net/EthOnDataProperty">
        <rdfs:subPropertyOf rdf:resource="http://www.w3.org/2002/07/owl#topDataProperty"/>
        <rdfs:comment xml:lang="en">Groups all data properties specific to EthOn.</rdfs:comment>
        <rdfs:label xml:lang="en">EthOn Data Property</rdfs:label>
        <ns:term_status>unstable</ns:term_status>
    </owl:DatatypeProperty>



    <!-- http://ethon.consensys.net/MessageDataProperty -->

    <owl:DatatypeProperty rdf:about="http://ethon.consensys.net/MessageDataProperty">
        <rdfs:subPropertyOf rdf:resource="http://ethon.consensys.net/EthOnDataProperty"/>
        <rdfs:domain rdf:resource="http://ethon.consensys.net/MessageConcept"/>
        <rdfs:comment xml:lang="en">Groups all EthOn message data properties.</rdfs:comment>
        <rdfs:label>EthOn Message Data Property</rdfs:label>
        <ns:term_status>unstable</ns:term_status>
    </owl:DatatypeProperty>



    <!-- http://ethon.consensys.net/NetworkDataProperty -->

    <owl:DatatypeProperty rdf:about="http://ethon.consensys.net/NetworkDataProperty">
        <rdfs:subPropertyOf rdf:resource="http://ethon.consensys.net/EthOnDataProperty"/>
        <rdfs:comment xml:lang="en">Groups all EthOn network data properties.</rdfs:comment>
        <rdfs:label xml:lang="en">EthOn Network Data Property</rdfs:label>
        <ns:term_status>unstable</ns:term_status>
    </owl:DatatypeProperty>



    <!-- http://ethon.consensys.net/StateDataProperty -->

    <owl:DatatypeProperty rdf:about="http://ethon.consensys.net/StateDataProperty">
        <rdfs:subPropertyOf rdf:resource="http://ethon.consensys.net/EthOnDataProperty"/>
        <rdfs:domain rdf:resource="http://ethon.consensys.net/StateConcept"/>
    </owl:DatatypeProperty>



    <!-- http://ethon.consensys.net/accountBalance -->

    <owl:DatatypeProperty rdf:about="http://ethon.consensys.net/accountBalance">
        <rdfs:subPropertyOf rdf:resource="http://ethon.consensys.net/AccountDataProperty"/>
        <rdf:type rdf:resource="http://www.w3.org/2002/07/owl#FunctionalProperty"/>
        <rdfs:domain rdf:resource="http://ethon.consensys.net/AccountState"/>
        <rdfs:range rdf:resource="http://www.w3.org/2001/XMLSchema#integer"/>
        <suggestedStringRepresentation>accountBalance</suggestedStringRepresentation>
        <rdfs:comment xml:lang="en">A scalar value equal to the number of Wei owned by an account at a given account state.</rdfs:comment>
        <rdfs:label xml:lang="en">Account balance</rdfs:label>
        <ns:term_status>unstable</ns:term_status>
    </owl:DatatypeProperty>



    <!-- http://ethon.consensys.net/accountBalancePrefunded -->

    <owl:DatatypeProperty rdf:about="http://ethon.consensys.net/accountBalancePrefunded">
        <rdfs:subPropertyOf rdf:resource="http://ethon.consensys.net/AccountDataProperty"/>
        <rdfs:domain rdf:resource="http://ethon.consensys.net/ProtocolAccount"/>
        <rdfs:range rdf:resource="http://www.w3.org/2001/XMLSchema#integer"/>
        <suggestedStringRepresentation>accountBalancePrefunded</suggestedStringRepresentation>
        <rdfs:comment xml:lang="en">The amount of Wei an account was prefunded with in a protocol variant. In the case that an account receives multiple prefunds in multiple protocol variants, the amounts are summed. In contrast to the regular account balance it is a property of the account itself and not of its state.</rdfs:comment>
        <rdfs:label xml:lang="en">Account balance prefunded</rdfs:label>
        <ns:term_status>unstable</ns:term_status>
    </owl:DatatypeProperty>



    <!-- http://ethon.consensys.net/accountCode -->

    <owl:DatatypeProperty rdf:about="http://ethon.consensys.net/accountCode">
        <rdfs:subPropertyOf rdf:resource="http://ethon.consensys.net/AccountDataProperty"/>
        <rdf:type rdf:resource="http://www.w3.org/2002/07/owl#FunctionalProperty"/>
        <rdfs:domain rdf:resource="http://ethon.consensys.net/ContractAccount"/>
        <rdfs:range rdf:resource="http://www.w3.org/2001/XMLSchema#hexBinary"/>
        <suggestedStringRepresentation>accountCode</suggestedStringRepresentation>
        <rdfs:comment xml:lang="en">The immutable EVM bytecode of the contract account.</rdfs:comment>
        <rdfs:label xml:lang="en">Account code</rdfs:label>
        <ns:term_status>unstable</ns:term_status>
    </owl:DatatypeProperty>



    <!-- http://ethon.consensys.net/accountCodeHash -->

    <owl:DatatypeProperty rdf:about="http://ethon.consensys.net/accountCodeHash">
        <rdfs:subPropertyOf rdf:resource="http://ethon.consensys.net/AccountDataProperty"/>
        <rdf:type rdf:resource="http://www.w3.org/2002/07/owl#FunctionalProperty"/>
        <rdfs:domain rdf:resource="http://ethon.consensys.net/ContractAccount"/>
        <rdfs:range rdf:resource="http://www.w3.org/2001/XMLSchema#hexBinary"/>
        <suggestedStringRepresentation>accountCodeHash</suggestedStringRepresentation>
        <rdfs:comment xml:lang="en">The immutable Keccak-256 hash of the EVM code of an account.</rdfs:comment>
        <rdfs:label xml:lang="en">Account code hash</rdfs:label>
        <ns:term_status>unstable</ns:term_status>
    </owl:DatatypeProperty>



    <!-- http://ethon.consensys.net/accountNonce -->

    <owl:DatatypeProperty rdf:about="http://ethon.consensys.net/accountNonce">
        <rdfs:subPropertyOf rdf:resource="http://ethon.consensys.net/AccountDataProperty"/>
        <rdf:type rdf:resource="http://www.w3.org/2002/07/owl#FunctionalProperty"/>
        <rdfs:domain rdf:resource="http://ethon.consensys.net/AccountState"/>
        <rdfs:range rdf:resource="http://www.w3.org/2001/XMLSchema#integer"/>
        <suggestedStringRepresentation>accountNonce</suggestedStringRepresentation>
        <rdfs:comment xml:lang="en">A scalar value equal to the number of transactions sent from this account or, in the case of accounts with associated code, the number of contract-creations made by this account.</rdfs:comment>
        <rdfs:label xml:lang="en">Account nonce</rdfs:label>
        <ns:term_status>unstable</ns:term_status>
    </owl:DatatypeProperty>



    <!-- http://ethon.consensys.net/accountPublicKey -->

    <owl:DatatypeProperty rdf:about="http://ethon.consensys.net/accountPublicKey">
        <rdfs:subPropertyOf rdf:resource="http://ethon.consensys.net/AccountDataProperty"/>
        <rdf:type rdf:resource="http://www.w3.org/2002/07/owl#FunctionalProperty"/>
        <rdfs:domain rdf:resource="http://ethon.consensys.net/ExternalAccount"/>
        <rdfs:range rdf:resource="http://www.w3.org/2001/XMLSchema#hexBinary"/>
        <suggestedStringRepresentation>accountPublicKey</suggestedStringRepresentation>
        <rdfs:comment xml:lang="en">The public key of an external account.</rdfs:comment>
        <rdfs:label xml:lang="en">Account public key</rdfs:label>
        <ns:term_status>unstable</ns:term_status>
    </owl:DatatypeProperty>



    <!-- http://ethon.consensys.net/address -->

    <owl:DatatypeProperty rdf:about="http://ethon.consensys.net/address">
        <rdfs:subPropertyOf rdf:resource="http://ethon.consensys.net/AccountDataProperty"/>
        <rdf:type rdf:resource="http://www.w3.org/2002/07/owl#FunctionalProperty"/>
        <rdfs:domain rdf:resource="http://ethon.consensys.net/Account"/>
        <rdfs:range rdf:resource="http://www.w3.org/2001/XMLSchema#hexBinary"/>
        <suggestedStringRepresentation>address</suggestedStringRepresentation>
        <rdfs:comment xml:lang="en">A 160-bit identifier for accounts.</rdfs:comment>
        <rdfs:label xml:lang="en">Address</rdfs:label>
        <ns:term_status>unstable</ns:term_status>
    </owl:DatatypeProperty>



    <!-- http://ethon.consensys.net/blockBeneficiaryReward -->

    <owl:DatatypeProperty rdf:about="http://ethon.consensys.net/blockBeneficiaryReward">
        <rdfs:subPropertyOf rdf:resource="http://ethon.consensys.net/BlockDataProperty"/>
        <rdf:type rdf:resource="http://www.w3.org/2002/07/owl#FunctionalProperty"/>
        <rdfs:domain rdf:resource="http://ethon.consensys.net/Block"/>
        <rdfs:range rdf:resource="http://www.w3.org/2001/XMLSchema#integer"/>
        <suggestedStringRepresentation>blockBenficiaryReward</suggestedStringRepresentation>
        <rdfs:comment xml:lang="en">The reward the beneficiary receives for mining a block. It is comprised of the base reward (5ETH), rewards for including uncles (1/32 of block reward per uncle) and the fees of the Tx in the block.</rdfs:comment>
        <rdfs:label xml:lang="en">Block beneficiary reward</rdfs:label>
        <ns:term_status>unstable</ns:term_status>
    </owl:DatatypeProperty>



    <!-- http://ethon.consensys.net/blockCreationTime -->

    <owl:DatatypeProperty rdf:about="http://ethon.consensys.net/blockCreationTime">
        <rdfs:subPropertyOf rdf:resource="http://ethon.consensys.net/BlockDataProperty"/>
        <rdf:type rdf:resource="http://www.w3.org/2002/07/owl#FunctionalProperty"/>
        <rdfs:domain>
            <owl:Class>
                <owl:unionOf rdf:parseType="Collection">
                    <rdf:Description rdf:about="http://ethon.consensys.net/Block"/>
                    <rdf:Description rdf:about="http://ethon.consensys.net/Uncle"/>
                </owl:unionOf>
            </owl:Class>
        </rdfs:domain>
        <rdfs:range rdf:resource="http://www.w3.org/2001/XMLSchema#dateTime"/>
        <suggestedStringRepresentation>blockCreationTime</suggestedStringRepresentation>
        <rdfs:comment xml:lang="en">This block&apos;s inception date and time.</rdfs:comment>
        <rdfs:label xml:lang="en">Block creation time</rdfs:label>
        <ns:term_status>unstable</ns:term_status>
    </owl:DatatypeProperty>



    <!-- http://ethon.consensys.net/blockDifficulty -->

    <owl:DatatypeProperty rdf:about="http://ethon.consensys.net/blockDifficulty">
        <rdfs:subPropertyOf rdf:resource="http://ethon.consensys.net/BlockDataProperty"/>
        <rdf:type rdf:resource="http://www.w3.org/2002/07/owl#FunctionalProperty"/>
        <rdfs:domain>
            <owl:Class>
                <owl:unionOf rdf:parseType="Collection">
                    <rdf:Description rdf:about="http://ethon.consensys.net/Block"/>
                    <rdf:Description rdf:about="http://ethon.consensys.net/Uncle"/>
                </owl:unionOf>
            </owl:Class>
        </rdfs:domain>
        <rdfs:range rdf:resource="http://www.w3.org/2001/XMLSchema#integer"/>
        <suggestedStringRepresentation>blockDifficulty</suggestedStringRepresentation>
        <rdfs:comment xml:lang="en">A scalar value corresponding to the difficulty level of this block. This can be calculated from the previous block&apos;s difficulty level and the timestamp.</rdfs:comment>
        <rdfs:label xml:lang="en">Block difficulty</rdfs:label>
        <ns:term_status>unstable</ns:term_status>
    </owl:DatatypeProperty>



    <!-- http://ethon.consensys.net/blockExtraData -->

    <owl:DatatypeProperty rdf:about="http://ethon.consensys.net/blockExtraData">
        <rdfs:subPropertyOf rdf:resource="http://ethon.consensys.net/BlockDataProperty"/>
        <rdf:type rdf:resource="http://www.w3.org/2002/07/owl#FunctionalProperty"/>
        <rdfs:domain>
            <owl:Class>
                <owl:unionOf rdf:parseType="Collection">
                    <rdf:Description rdf:about="http://ethon.consensys.net/Block"/>
                    <rdf:Description rdf:about="http://ethon.consensys.net/Uncle"/>
                </owl:unionOf>
            </owl:Class>
        </rdfs:domain>
        <rdfs:range rdf:resource="http://www.w3.org/2001/XMLSchema#hexBinary"/>
        <suggestedStringRepresentation>blockExtraData</suggestedStringRepresentation>
        <rdfs:comment xml:lang="en">An arbitrary byte array containing data relevant to this block. This must be 32 bytes or fewer.</rdfs:comment>
        <rdfs:label xml:lang="en">Block extra data</rdfs:label>
        <ns:term_status>unstable</ns:term_status>
    </owl:DatatypeProperty>



    <!-- http://ethon.consensys.net/blockGasLimit -->

    <owl:DatatypeProperty rdf:about="http://ethon.consensys.net/blockGasLimit">
        <rdfs:subPropertyOf rdf:resource="http://ethon.consensys.net/BlockDataProperty"/>
        <rdf:type rdf:resource="http://www.w3.org/2002/07/owl#FunctionalProperty"/>
        <rdfs:domain>
            <owl:Class>
                <owl:unionOf rdf:parseType="Collection">
                    <rdf:Description rdf:about="http://ethon.consensys.net/Block"/>
                    <rdf:Description rdf:about="http://ethon.consensys.net/Uncle"/>
                </owl:unionOf>
            </owl:Class>
        </rdfs:domain>
        <rdfs:range rdf:resource="http://www.w3.org/2001/XMLSchema#integer"/>
        <suggestedStringRepresentation>blockGasLimit</suggestedStringRepresentation>
        <rdfs:comment xml:lang="en">A scalar value equal to the current limit of gas expenditure per block.  Its purpose is to keep block propagation and processing time low, thereby allowing for a sufficiently decentralized network. Miners have the option to increase or decrease it every block by a certain factor.</rdfs:comment>
        <rdfs:label xml:lang="en">Block gas limit</rdfs:label>
        <ns:term_status>unstable</ns:term_status>
    </owl:DatatypeProperty>



    <!-- http://ethon.consensys.net/blockGasUsed -->

    <owl:DatatypeProperty rdf:about="http://ethon.consensys.net/blockGasUsed">
        <rdfs:subPropertyOf rdf:resource="http://ethon.consensys.net/BlockDataProperty"/>
        <rdf:type rdf:resource="http://www.w3.org/2002/07/owl#FunctionalProperty"/>
        <rdfs:domain>
            <owl:Class>
                <owl:unionOf rdf:parseType="Collection">
                    <rdf:Description rdf:about="http://ethon.consensys.net/Block"/>
                    <rdf:Description rdf:about="http://ethon.consensys.net/Uncle"/>
                </owl:unionOf>
            </owl:Class>
        </rdfs:domain>
        <rdfs:range rdf:resource="http://www.w3.org/2001/XMLSchema#integer"/>
        <suggestedStringRepresentation>blockGasUsed</suggestedStringRepresentation>
        <rdfs:comment xml:lang="en">A scalar value equal to the total gas used by all transactions in this block.</rdfs:comment>
        <rdfs:label xml:lang="en">Block gas used</rdfs:label>
        <ns:term_status>unstable</ns:term_status>
    </owl:DatatypeProperty>



    <!-- http://ethon.consensys.net/blockHash -->

    <owl:DatatypeProperty rdf:about="http://ethon.consensys.net/blockHash">
        <rdfs:subPropertyOf rdf:resource="http://ethon.consensys.net/BlockDataProperty"/>
        <rdf:type rdf:resource="http://www.w3.org/2002/07/owl#FunctionalProperty"/>
        <rdfs:domain>
            <owl:Class>
                <owl:unionOf rdf:parseType="Collection">
                    <rdf:Description rdf:about="http://ethon.consensys.net/Block"/>
                    <rdf:Description rdf:about="http://ethon.consensys.net/Uncle"/>
                </owl:unionOf>
            </owl:Class>
        </rdfs:domain>
        <rdfs:range rdf:resource="http://www.w3.org/2001/XMLSchema#hexBinary"/>
        <suggestedStringRepresentation>blockHash</suggestedStringRepresentation>
        <rdfs:comment xml:lang="en">The Keccak 256-bit hash of the block&apos;s header, in its entierty.</rdfs:comment>
        <rdfs:label xml:lang="en">Block hash</rdfs:label>
        <ns:term_status>unstable</ns:term_status>
    </owl:DatatypeProperty>



    <!-- http://ethon.consensys.net/blockHeader -->

    <owl:DatatypeProperty rdf:about="http://ethon.consensys.net/blockHeader">
        <rdfs:subPropertyOf rdf:resource="http://ethon.consensys.net/BlockDataProperty"/>
        <rdf:type rdf:resource="http://www.w3.org/2002/07/owl#FunctionalProperty"/>
        <rdfs:domain>
            <owl:Class>
                <owl:unionOf rdf:parseType="Collection">
                    <rdf:Description rdf:about="http://ethon.consensys.net/Block"/>
                    <rdf:Description rdf:about="http://ethon.consensys.net/Uncle"/>
                </owl:unionOf>
            </owl:Class>
        </rdfs:domain>
        <rdfs:range rdf:resource="http://www.w3.org/2001/XMLSchema#hexBinary"/>
        <suggestedStringRepresentation>blockHeader</suggestedStringRepresentation>
        <rdfs:comment xml:lang="en">Relates a block to its block header data. The block header data contains 15 pieces of information: 1. the parent hash, 2. the Uncle hash, 3. a beneficiary address, 4. a state root hash, 5. a transactions root hash, 6. a receipts root hash, 7. a log bloom filter, 8. the difficulty value, 9. the block number, 10. the gas limit of the block, 11. the gas used by all transactions in the block, 12. a scalar timestamp in unix time() format, 13. a byte array containing extra data, 14. a mix hash and 15. the block nonce. The property is functional because a block can have only exactly one block header.</rdfs:comment>
        <rdfs:label xml:lang="en">Block header</rdfs:label>
        <ns:term_status>unstable</ns:term_status>
    </owl:DatatypeProperty>



    <!-- http://ethon.consensys.net/blockLogsBloom -->

    <owl:DatatypeProperty rdf:about="http://ethon.consensys.net/blockLogsBloom">
        <rdfs:subPropertyOf rdf:resource="http://ethon.consensys.net/BlockDataProperty"/>
        <rdf:type rdf:resource="http://www.w3.org/2002/07/owl#FunctionalProperty"/>
        <rdfs:domain>
            <owl:Class>
                <owl:unionOf rdf:parseType="Collection">
                    <rdf:Description rdf:about="http://ethon.consensys.net/Block"/>
                    <rdf:Description rdf:about="http://ethon.consensys.net/Uncle"/>
                </owl:unionOf>
            </owl:Class>
        </rdfs:domain>
        <rdfs:range rdf:resource="http://www.w3.org/2001/XMLSchema#hexBinary"/>
        <suggestedStringRepresentation>blockLogsBloom</suggestedStringRepresentation>
        <rdfs:comment xml:lang="en">The Bloom filter composed from indexable information (logger address and log topics) contained in each log entry from the receipt of each transaction in the transactions list.</rdfs:comment>
        <rdfs:label xml:lang="en">Block logs bloom filter</rdfs:label>
        <ns:term_status>unstable</ns:term_status>
    </owl:DatatypeProperty>



    <!-- http://ethon.consensys.net/blockMixHash -->

    <owl:DatatypeProperty rdf:about="http://ethon.consensys.net/blockMixHash">
        <rdfs:subPropertyOf rdf:resource="http://ethon.consensys.net/BlockDataProperty"/>
        <rdf:type rdf:resource="http://www.w3.org/2002/07/owl#FunctionalProperty"/>
        <rdfs:domain>
            <owl:Class>
                <owl:unionOf rdf:parseType="Collection">
                    <rdf:Description rdf:about="http://ethon.consensys.net/Block"/>
                    <rdf:Description rdf:about="http://ethon.consensys.net/Uncle"/>
                </owl:unionOf>
            </owl:Class>
        </rdfs:domain>
        <rdfs:range rdf:resource="http://www.w3.org/2001/XMLSchema#hexBinary"/>
        <suggestedStringRepresentation>blockMixHash</suggestedStringRepresentation>
        <rdfs:comment xml:lang="en">A 256-bit hash which proves combined with the nonce that a sufficient amount of computation has been carried out on this block.</rdfs:comment>
        <rdfs:label xml:lang="en">Block mix hash</rdfs:label>
        <ns:term_status>unstable</ns:term_status>
    </owl:DatatypeProperty>



    <!-- http://ethon.consensys.net/blockNonce -->

    <owl:DatatypeProperty rdf:about="http://ethon.consensys.net/blockNonce">
        <rdfs:subPropertyOf rdf:resource="http://ethon.consensys.net/BlockDataProperty"/>
        <rdf:type rdf:resource="http://www.w3.org/2002/07/owl#FunctionalProperty"/>
        <rdfs:domain>
            <owl:Class>
                <owl:unionOf rdf:parseType="Collection">
                    <rdf:Description rdf:about="http://ethon.consensys.net/Block"/>
                    <rdf:Description rdf:about="http://ethon.consensys.net/Uncle"/>
                </owl:unionOf>
            </owl:Class>
        </rdfs:domain>
        <rdfs:range rdf:resource="http://www.w3.org/2001/XMLSchema#hexBinary"/>
        <suggestedStringRepresentation>blockNonce</suggestedStringRepresentation>
        <rdfs:comment xml:lang="en">A 64 bit hash which proves combined with the mix-hash that a sufficient amount of computation has been carried out on this block.</rdfs:comment>
        <rdfs:label xml:lang="en">Block nonce</rdfs:label>
        <ns:term_status>unstable</ns:term_status>
    </owl:DatatypeProperty>



    <!-- http://ethon.consensys.net/blockSize -->

    <owl:DatatypeProperty rdf:about="http://ethon.consensys.net/blockSize">
        <rdfs:subPropertyOf rdf:resource="http://ethon.consensys.net/BlockDataProperty"/>
        <rdf:type rdf:resource="http://www.w3.org/2002/07/owl#FunctionalProperty"/>
        <rdfs:domain rdf:resource="http://ethon.consensys.net/Block"/>
        <rdfs:range rdf:resource="http://www.w3.org/2001/XMLSchema#integer"/>
        <suggestedStringRepresentation>blockSize</suggestedStringRepresentation>
        <rdfs:comment xml:lang="en">The size of the block header in RLP format in bytes.</rdfs:comment>
        <rdfs:label xml:lang="en">Block size</rdfs:label>
        <rdfs:seeAlso rdf:resource="https://github.com/ethereum/wiki/wiki/RLP"/>
        <ns:term_status>unstable</ns:term_status>
    </owl:DatatypeProperty>



    <!-- http://ethon.consensys.net/clientVersion -->

    <owl:DatatypeProperty rdf:about="http://ethon.consensys.net/clientVersion">
        <rdfs:subPropertyOf rdf:resource="http://ethon.consensys.net/NetworkDataProperty"/>
        <rdfs:domain rdf:resource="http://ethon.consensys.net/Node"/>
        <rdfs:range rdf:resource="http://www.w3.org/2001/XMLSchema#string"/>
        <suggestedStringRepresentation>clientVersion</suggestedStringRepresentation>
        <rdfs:comment xml:lang="en">Relates a node to a string identifying the Ethereum client version it runs. It composed of the client name (e.g. Geth) and a version identifier (e.g. v1.5.4).</rdfs:comment>
        <rdfs:label xml:lang="en">runs client</rdfs:label>
        <ns:term_status>unstable</ns:term_status>
    </owl:DatatypeProperty>



    <!-- http://ethon.consensys.net/cumulativeGasUsed -->

    <owl:DatatypeProperty rdf:about="http://ethon.consensys.net/cumulativeGasUsed">
        <rdfs:subPropertyOf rdf:resource="http://ethon.consensys.net/MessageDataProperty"/>
        <rdfs:domain rdf:resource="http://ethon.consensys.net/Tx"/>
        <rdfs:range rdf:resource="http://www.w3.org/2001/XMLSchema#integer"/>
        <suggestedStringRepresentation>cumulativeGasUsed</suggestedStringRepresentation>
        <rdfs:comment xml:lang="en">The cumulative gas used in the block containing the transaction as of immediately after the transaction has happened.</rdfs:comment>
        <rdfs:label xml:lang="en">cumulative gas used</rdfs:label>
        <ns:term_status>unstable</ns:term_status>
    </owl:DatatypeProperty>



    <!-- http://ethon.consensys.net/logData -->

    <owl:DatatypeProperty rdf:about="http://ethon.consensys.net/logData">
        <rdfs:subPropertyOf rdf:resource="http://ethon.consensys.net/MessageDataProperty"/>
        <rdfs:domain rdf:resource="http://ethon.consensys.net/LogEntry"/>
        <rdfs:range rdf:resource="http://www.w3.org/2001/XMLSchema#hexBinary"/>
        <suggestedStringRepresentation>logData</suggestedStringRepresentation>
        <rdfs:comment xml:lang="en">Relates a log entry to its data.</rdfs:comment>
        <rdfs:label xml:lang="en">Log data</rdfs:label>
        <ns:term_status>unstable</ns:term_status>
    </owl:DatatypeProperty>



    <!-- http://ethon.consensys.net/logIndex -->

    <owl:DatatypeProperty rdf:about="http://ethon.consensys.net/logIndex">
        <rdfs:subPropertyOf rdf:resource="http://ethon.consensys.net/MessageDataProperty"/>
        <rdf:type rdf:resource="http://www.w3.org/2002/07/owl#FunctionalProperty"/>
        <rdfs:domain rdf:resource="http://ethon.consensys.net/Tx"/>
        <rdfs:range rdf:resource="http://www.w3.org/2001/XMLSchema#integer"/>
        <suggestedStringRepresentation>logIndex</suggestedStringRepresentation>
        <rdfs:comment xml:lang="en">Relates a log entry to its index in the transaction reciept of a transaction. The log index defines the order of the log entries of a transaction.</rdfs:comment>
        <rdfs:label xml:lang="en">Log index</rdfs:label>
        <ns:term_status>unstable</ns:term_status>
    </owl:DatatypeProperty>



    <!-- http://ethon.consensys.net/logTopicData -->

    <owl:DatatypeProperty rdf:about="http://ethon.consensys.net/logTopicData">
        <rdfs:subPropertyOf rdf:resource="http://ethon.consensys.net/MessageDataProperty"/>
        <rdf:type rdf:resource="http://www.w3.org/2002/07/owl#FunctionalProperty"/>
        <rdfs:domain rdf:resource="http://ethon.consensys.net/LogTopic"/>
        <rdfs:range rdf:resource="http://www.w3.org/2001/XMLSchema#hexBinary"/>
        <suggestedStringRepresentation>logTopicData</suggestedStringRepresentation>
        <rdfs:comment xml:lang="en">Relates a log topic to the 32 bytes of data it contains.</rdfs:comment>
        <rdfs:label xml:lang="en">Log Topic data</rdfs:label>
        <ns:term_status>unstable</ns:term_status>
    </owl:DatatypeProperty>



    <!-- http://ethon.consensys.net/logTopicIndex -->

    <owl:DatatypeProperty rdf:about="http://ethon.consensys.net/logTopicIndex">
        <rdfs:subPropertyOf rdf:resource="http://ethon.consensys.net/MessageDataProperty"/>
        <rdf:type rdf:resource="http://www.w3.org/2002/07/owl#FunctionalProperty"/>
        <rdfs:domain rdf:resource="http://ethon.consensys.net/LogTopic"/>
        <rdfs:range rdf:resource="http://www.w3.org/2001/XMLSchema#integer"/>
        <suggestedStringRepresentation>logTopicIndex</suggestedStringRepresentation>
        <rdfs:comment xml:lang="en">Relates a log topic to its index in the log entry. The log topic index defines the order of the log topics of in log entry.</rdfs:comment>
        <rdfs:label xml:lang="en">Log Topic index</rdfs:label>
        <ns:term_status>unstable</ns:term_status>
    </owl:DatatypeProperty>



    <!-- http://ethon.consensys.net/msgCallDepth -->

    <owl:DatatypeProperty rdf:about="http://ethon.consensys.net/msgCallDepth">
        <rdfs:subPropertyOf rdf:resource="http://ethon.consensys.net/MessageDataProperty"/>
        <rdfs:domain rdf:resource="http://ethon.consensys.net/Tx"/>
        <rdfs:range rdf:resource="http://www.w3.org/2001/XMLSchema#integer"/>
        <suggestedStringRepresentation>msgCallDepth</suggestedStringRepresentation>
        <rdfs:comment xml:lang="en">A scalar value equal to the depth of the contract message. A contract message is represented as a call in the Ethereum EVM. This value represents the number of CALL or CREATE opcodes being executed at the time of the message execution.</rdfs:comment>
        <rdfs:label xml:lang="en">Message call depth</rdfs:label>
        <ns:term_status>unstable</ns:term_status>
    </owl:DatatypeProperty>



    <!-- http://ethon.consensys.net/msgData -->

    <owl:DatatypeProperty rdf:about="http://ethon.consensys.net/msgData">
        <rdfs:subPropertyOf rdf:resource="http://ethon.consensys.net/msgPayload"/>
        <rdfs:domain>
            <owl:Class>
                <owl:unionOf rdf:parseType="Collection">
                    <rdf:Description rdf:about="http://ethon.consensys.net/CallContractMsg"/>
                    <rdf:Description rdf:about="http://ethon.consensys.net/CallTx"/>
                </owl:unionOf>
            </owl:Class>
        </rdfs:domain>
        <rdfs:range rdf:resource="http://www.w3.org/2001/XMLSchema#hexBinary"/>
        <suggestedStringRepresentation>msgData</suggestedStringRepresentation>
        <rdfs:comment xml:lang="en">An unlimited size byte array specifying the input data of the call.</rdfs:comment>
        <rdfs:label xml:lang="en">call data</rdfs:label>
        <ns:term_status>unstable</ns:term_status>
    </owl:DatatypeProperty>



    <!-- http://ethon.consensys.net/msgError -->

    <owl:DatatypeProperty rdf:about="http://ethon.consensys.net/msgError">
        <rdfs:subPropertyOf rdf:resource="http://ethon.consensys.net/MessageDataProperty"/>
        <rdf:type rdf:resource="http://www.w3.org/2002/07/owl#FunctionalProperty"/>
        <rdfs:domain rdf:resource="http://ethon.consensys.net/Msg"/>
        <rdfs:range rdf:resource="http://www.w3.org/2001/XMLSchema#boolean"/>
        <suggestedStringRepresentation>msgError</suggestedStringRepresentation>
        <rdfs:comment xml:lang="en">A boolean value indicating whether the message validation resulted in an error. A &quot;true&quot; value indicates an error.</rdfs:comment>
        <rdfs:label xml:lang="en">Message error</rdfs:label>
        <ns:term_status>unstable</ns:term_status>
    </owl:DatatypeProperty>



    <!-- http://ethon.consensys.net/msgErrorString -->

    <owl:DatatypeProperty rdf:about="http://ethon.consensys.net/msgErrorString">
        <rdfs:subPropertyOf rdf:resource="http://ethon.consensys.net/MessageDataProperty"/>
        <rdf:type rdf:resource="http://www.w3.org/2002/07/owl#FunctionalProperty"/>
        <rdfs:domain rdf:resource="http://ethon.consensys.net/Msg"/>
        <rdfs:range rdf:resource="http://www.w3.org/2001/XMLSchema#string"/>
        <suggestedStringRepresentation>msgErrorString</suggestedStringRepresentation>
        <rdfs:comment xml:lang="en">A string informally describing an error that occured during the validation of a message. Only exists if msgError is true.</rdfs:comment>
        <rdfs:label xml:lang="en">Message error string</rdfs:label>
        <ns:term_status>unstable</ns:term_status>
    </owl:DatatypeProperty>



    <!-- http://ethon.consensys.net/msgGasLimit -->

    <owl:DatatypeProperty rdf:about="http://ethon.consensys.net/msgGasLimit">
        <rdfs:subPropertyOf rdf:resource="http://ethon.consensys.net/MessageDataProperty"/>
        <rdfs:domain rdf:resource="http://ethon.consensys.net/Msg"/>
        <rdfs:range rdf:resource="http://www.w3.org/2001/XMLSchema#integer"/>
        <suggestedStringRepresentation>msgGasLimit</suggestedStringRepresentation>
        <rdfs:comment xml:lang="en">A scalar value equal to the maximum amount of gas that should be used in executing this transaction. This is paid up-front, before any computation is done and may not be increased later. If used with contract messages it represents the fraction of the original transaction gas limit still available for execution of the contract message. After all resulting computations are done, excess gas is returned to the sender of the original transaction.</rdfs:comment>
        <rdfs:label xml:lang="en">Message gas limit</rdfs:label>
        <ns:term_status>unstable</ns:term_status>
    </owl:DatatypeProperty>



    <!-- http://ethon.consensys.net/msgGasUsed -->

    <owl:DatatypeProperty rdf:about="http://ethon.consensys.net/msgGasUsed">
        <rdfs:subPropertyOf rdf:resource="http://ethon.consensys.net/MessageDataProperty"/>
        <rdf:type rdf:resource="http://www.w3.org/2002/07/owl#FunctionalProperty"/>
        <rdfs:domain rdf:resource="http://ethon.consensys.net/Msg"/>
        <rdfs:range rdf:resource="http://www.w3.org/2001/XMLSchema#integer"/>
        <owl:propertyDisjointWith rdf:resource="http://ethon.consensys.net/txGasUsed"/>
        <suggestedStringRepresentation>msgGasUsed</suggestedStringRepresentation>
        <rdfs:comment xml:lang="en">The amount of gas that was used for processing a single message, regardless of which type of message it may be.</rdfs:comment>
        <rdfs:label xml:lang="en">Msg gas used</rdfs:label>
        <ns:term_status>unstable</ns:term_status>
    </owl:DatatypeProperty>



    <!-- http://ethon.consensys.net/msgInit -->

    <owl:DatatypeProperty rdf:about="http://ethon.consensys.net/msgInit">
        <rdfs:subPropertyOf rdf:resource="http://ethon.consensys.net/msgPayload"/>
        <rdfs:domain>
            <owl:Class>
                <owl:unionOf rdf:parseType="Collection">
                    <rdf:Description rdf:about="http://ethon.consensys.net/CreateContractMsg"/>
                    <rdf:Description rdf:about="http://ethon.consensys.net/CreateTx"/>
                </owl:unionOf>
            </owl:Class>
        </rdfs:domain>
        <rdfs:range rdf:resource="http://www.w3.org/2001/XMLSchema#hexBinary"/>
        <suggestedStringRepresentation>msgInit</suggestedStringRepresentation>
        <rdfs:comment xml:lang="en">An unlimited size byte array specifying the EVM-code for the contract account initialisation procedure.</rdfs:comment>
        <rdfs:label xml:lang="en">Message init code</rdfs:label>
        <ns:term_status>unstable</ns:term_status>
    </owl:DatatypeProperty>



    <!-- http://ethon.consensys.net/msgOutput -->

    <owl:DatatypeProperty rdf:about="http://ethon.consensys.net/msgOutput">
        <rdfs:subPropertyOf rdf:resource="http://ethon.consensys.net/MessageDataProperty"/>
        <rdf:type rdf:resource="http://www.w3.org/2002/07/owl#FunctionalProperty"/>
	<rdfs:domain>
            <owl:Class>
                <owl:unionOf rdf:parseType="Collection">
                    <rdf:Description rdf:about="http://ethon.consensys.net/CallContractMsg"/>
                    <rdf:Description rdf:about="http://ethon.consensys.net/CallTx"/>
                </owl:unionOf>
            </owl:Class>
        </rdfs:domain>
        <rdfs:range rdf:resource="http://www.w3.org/2001/XMLSchema#hexBinary"/>
        <suggestedStringRepresentation>msgOutput</suggestedStringRepresentation>
        <rdfs:comment xml:lang="en">The resulting output data from a call tx or call contract message. This is the return value from the (function) call.</rdfs:comment>
        <rdfs:label xml:lang="en">Message output</rdfs:label>
        <ns:term_status>unstable</ns:term_status>
    </owl:DatatypeProperty>



    <!-- http://ethon.consensys.net/msgPayload -->

    <owl:DatatypeProperty rdf:about="http://ethon.consensys.net/msgPayload">
        <rdfs:subPropertyOf rdf:resource="http://ethon.consensys.net/MessageDataProperty"/>
        <rdf:type rdf:resource="http://www.w3.org/2002/07/owl#FunctionalProperty"/>
        <rdfs:domain rdf:resource="http://ethon.consensys.net/Msg"/>
        <rdfs:range rdf:resource="http://www.w3.org/2001/XMLSchema#hexBinary"/>
        <suggestedStringRepresentation>msgPayload</suggestedStringRepresentation>
        <rdfs:comment xml:lang="en">An unlimited size byte array specifying the data payload of the message.</rdfs:comment>
        <rdfs:label xml:lang="en">Message payload</rdfs:label>
        <ns:term_status>unstable</ns:term_status>
    </owl:DatatypeProperty>



    <!-- http://ethon.consensys.net/msgRefundBalance -->

    <owl:DatatypeProperty rdf:about="http://ethon.consensys.net/msgRefundBalance">
        <rdfs:subPropertyOf rdf:resource="http://ethon.consensys.net/MessageDataProperty"/>
        <rdf:type rdf:resource="http://www.w3.org/2002/07/owl#FunctionalProperty"/>
        <rdfs:domain rdf:resource="http://ethon.consensys.net/SelfdestructContractMsg"/>
        <rdfs:range rdf:resource="http://www.w3.org/2001/XMLSchema#integer"/>
        <suggestedStringRepresentation>msgRefundBalance</suggestedStringRepresentation>
        <rdfs:comment xml:lang="en">A scalar value equal to the number of Wei that will be refunded as the result of a selfdestruct contract message.</rdfs:comment>
        <rdfs:label xml:lang="en">contract balance in Wei</rdfs:label>
        <ns:term_status>unstable</ns:term_status>
    </owl:DatatypeProperty>



    <!-- http://ethon.consensys.net/number -->

    <owl:DatatypeProperty rdf:about="http://ethon.consensys.net/number">
        <rdfs:subPropertyOf rdf:resource="http://ethon.consensys.net/BlockDataProperty"/>
        <rdf:type rdf:resource="http://www.w3.org/2002/07/owl#FunctionalProperty"/>
        <rdfs:domain>
            <owl:Class>
                <owl:unionOf rdf:parseType="Collection">
                    <rdf:Description rdf:about="http://ethon.consensys.net/Block"/>
                    <rdf:Description rdf:about="http://ethon.consensys.net/Uncle"/>
                </owl:unionOf>
            </owl:Class>
        </rdfs:domain>
        <rdfs:range rdf:resource="http://www.w3.org/2001/XMLSchema#integer"/>
        <suggestedStringRepresentation>number</suggestedStringRepresentation>
        <rdfs:comment xml:lang="en">A scalar value equal to the number of ancestor blocks. The genesis block has a number of zero.</rdfs:comment>
        <rdfs:label xml:lang="en">Block number</rdfs:label>
        <ns:term_status>unstable</ns:term_status>
    </owl:DatatypeProperty>



    <!-- http://ethon.consensys.net/receiptsRoot -->

    <owl:DatatypeProperty rdf:about="http://ethon.consensys.net/receiptsRoot">
        <rdfs:subPropertyOf rdf:resource="http://ethon.consensys.net/MessageDataProperty"/>
        <rdf:type rdf:resource="http://www.w3.org/2002/07/owl#FunctionalProperty"/>
        <rdfs:domain rdf:resource="http://ethon.consensys.net/ReceiptsTrie"/>
        <rdfs:range rdf:resource="http://www.w3.org/2001/XMLSchema#hexBinary"/>
        <suggestedStringRepresentation>blockReceiptsRoot</suggestedStringRepresentation>
        <rdfs:comment xml:lang="en">The Keccak 256-bit hash of the root node of the trie structure populated with the receipts of each transaction in the transactions list portion of the block.</rdfs:comment>
        <rdfs:label xml:lang="en">Receipts root</rdfs:label>
        <ns:term_status>unstable</ns:term_status>
    </owl:DatatypeProperty>



    <!-- http://ethon.consensys.net/startBlockNumber -->

    <owl:DatatypeProperty rdf:about="http://ethon.consensys.net/startBlockNumber">
        <rdfs:subPropertyOf rdf:resource="http://ethon.consensys.net/NetworkDataProperty"/>
        <rdfs:domain rdf:resource="http://ethon.consensys.net/Blockchain"/>
        <rdfs:range rdf:resource="http://www.w3.org/2001/XMLSchema#integer"/>
        <suggestedStringRepresentation>startBlockNumber</suggestedStringRepresentation>
        <rdfs:comment xml:lang="en">The block number of the first block in a new blockchain after a hard fork.</rdfs:comment>
        <rdfs:label xml:lang="en">start Block number</rdfs:label>
        <ns:term_status>unstable</ns:term_status>
    </owl:DatatypeProperty>



    <!-- http://ethon.consensys.net/stateRoot -->

    <owl:DatatypeProperty rdf:about="http://ethon.consensys.net/stateRoot">
        <rdfs:subPropertyOf rdf:resource="http://ethon.consensys.net/StateDataProperty"/>
        <rdf:type rdf:resource="http://www.w3.org/2002/07/owl#FunctionalProperty"/>
        <rdfs:domain rdf:resource="http://ethon.consensys.net/State"/>
        <rdfs:range rdf:resource="http://www.w3.org/2001/XMLSchema#hexBinary"/>
        <suggestedStringRepresentation>stateRoot</suggestedStringRepresentation>
        <rdfs:comment xml:lang="en">The Keccak 256-bit hash of the root node of the state trie that represents this state.</rdfs:comment>
        <rdfs:label xml:lang="en">State root</rdfs:label>
        <ns:term_status>unstable</ns:term_status>
    </owl:DatatypeProperty>



    <!-- http://ethon.consensys.net/storageRoot -->

    <owl:DatatypeProperty rdf:about="http://ethon.consensys.net/storageRoot">
        <rdfs:subPropertyOf rdf:resource="http://ethon.consensys.net/AccountDataProperty"/>
        <rdf:type rdf:resource="http://www.w3.org/2002/07/owl#FunctionalProperty"/>
        <rdfs:domain rdf:resource="http://ethon.consensys.net/AccountStorage"/>
        <rdfs:range rdf:resource="http://www.w3.org/2001/XMLSchema#hexBinary"/>
        <suggestedStringRepresentation>storageRoot</suggestedStringRepresentation>
        <rdfs:comment xml:lang="en">A 256-bit hash of the root node of a Merkle Patricia tree that encodes the storage contents of the account (a mapping between 265-bit integer values), encoded into the trie as a mapping from the Keccak 256-bit hash of the 256-bit integer keys to the RLP-encoded 256-bit integer values.</rdfs:comment>
        <rdfs:label xml:lang="en">Storage root</rdfs:label>
        <ns:term_status>unstable</ns:term_status>
    </owl:DatatypeProperty>



    <!-- http://ethon.consensys.net/transactionsRoot -->

    <owl:DatatypeProperty rdf:about="http://ethon.consensys.net/transactionsRoot">
        <rdfs:subPropertyOf rdf:resource="http://ethon.consensys.net/MessageDataProperty"/>
        <rdf:type rdf:resource="http://www.w3.org/2002/07/owl#FunctionalProperty"/>
        <rdfs:domain rdf:resource="http://ethon.consensys.net/TxTrie"/>
        <rdfs:range rdf:resource="http://www.w3.org/2001/XMLSchema#hexBinary"/>
        <suggestedStringRepresentation>blockTransactionsRoot</suggestedStringRepresentation>
        <rdfs:comment xml:lang="en">The Keccak 256-bit hash of the root node of the trie structure populated with each transaction in the transactions list portion of the block.</rdfs:comment>
        <rdfs:label xml:lang="en">Transactions root</rdfs:label>
        <ns:term_status>unstable</ns:term_status>
    </owl:DatatypeProperty>



    <!-- http://ethon.consensys.net/txGasPrice -->

    <owl:DatatypeProperty rdf:about="http://ethon.consensys.net/txGasPrice">
        <rdfs:subPropertyOf rdf:resource="http://ethon.consensys.net/MessageDataProperty"/>
        <rdfs:domain rdf:resource="http://ethon.consensys.net/Tx"/>
        <rdfs:range rdf:resource="http://www.w3.org/2001/XMLSchema#integer"/>
        <suggestedStringRepresentation>txGasPrice</suggestedStringRepresentation>
        <rdfs:comment xml:lang="en">A scalar value equal to the number of Wei to be paid per unit of gas for all computation costs incurred as a result of the execution of this transaction.</rdfs:comment>
        <rdfs:label xml:lang="en">Transaction gas price</rdfs:label>
        <ns:term_status>unstable</ns:term_status>
    </owl:DatatypeProperty>



    <!-- http://ethon.consensys.net/txGasUsed -->

    <owl:DatatypeProperty rdf:about="http://ethon.consensys.net/txGasUsed">
        <rdfs:subPropertyOf rdf:resource="http://ethon.consensys.net/MessageDataProperty"/>
        <rdf:type rdf:resource="http://www.w3.org/2002/07/owl#FunctionalProperty"/>
        <rdfs:domain rdf:resource="http://ethon.consensys.net/Tx"/>
        <rdfs:range rdf:resource="http://www.w3.org/2001/XMLSchema#integer"/>
        <suggestedStringRepresentation>txGasUsed</suggestedStringRepresentation>
        <rdfs:comment xml:lang="en">The total amount of gas that was used for processing this Tx and all contract messages resulting from it. It is the sum of all msgGasUsed by this Tx and resulting contract messages.</rdfs:comment>
        <rdfs:label xml:lang="en">Tx gas used</rdfs:label>
        <ns:term_status>unstable</ns:term_status>
    </owl:DatatypeProperty>



    <!-- http://ethon.consensys.net/txHash -->

    <owl:DatatypeProperty rdf:about="http://ethon.consensys.net/txHash">
        <rdfs:subPropertyOf rdf:resource="http://ethon.consensys.net/MessageDataProperty"/>
        <rdfs:domain rdf:resource="http://ethon.consensys.net/Tx"/>
        <rdfs:range rdf:resource="http://www.w3.org/2001/XMLSchema#hexBinary"/>
        <suggestedStringRepresentation>txHash</suggestedStringRepresentation>
        <rdfs:comment xml:lang="en">The Keccak 256-bit hash of the transaction</rdfs:comment>
        <rdfs:label xml:lang="en">Tx hash</rdfs:label>
        <ns:term_status>unstable</ns:term_status>
    </owl:DatatypeProperty>



    <!-- http://ethon.consensys.net/txIndex -->

    <owl:DatatypeProperty rdf:about="http://ethon.consensys.net/txIndex">
        <rdfs:subPropertyOf rdf:resource="http://ethon.consensys.net/MessageDataProperty"/>
        <rdfs:domain rdf:resource="http://ethon.consensys.net/Tx"/>
        <rdfs:range rdf:resource="http://www.w3.org/2001/XMLSchema#integer"/>
        <suggestedStringRepresentation>txIndex</suggestedStringRepresentation>
        <rdfs:comment xml:lang="en">The position of a transaction in a block.</rdfs:comment>
        <rdfs:label xml:lang="en">Transaction index</rdfs:label>
        <ns:term_status>unstable</ns:term_status>
    </owl:DatatypeProperty>



    <!-- http://ethon.consensys.net/txLogsBloom -->

    <owl:DatatypeProperty rdf:about="http://ethon.consensys.net/txLogsBloom">
        <rdfs:subPropertyOf rdf:resource="http://ethon.consensys.net/MessageDataProperty"/>
        <rdfs:domain rdf:resource="http://ethon.consensys.net/Tx"/>
        <rdfs:range rdf:resource="http://www.w3.org/2001/XMLSchema#hexBinary"/>
        <suggestedStringRepresentation>txLogsBloom</suggestedStringRepresentation>
        <rdfs:comment xml:lang="en">Relates a transaction to the Bloom filter of its log entries.</rdfs:comment>
        <rdfs:label xml:lang="en">Transaction Logs Bloom filter</rdfs:label>
        <ns:term_status>unstable</ns:term_status>
    </owl:DatatypeProperty>



    <!-- http://ethon.consensys.net/txNonce -->

    <owl:DatatypeProperty rdf:about="http://ethon.consensys.net/txNonce">
        <rdfs:subPropertyOf rdf:resource="http://ethon.consensys.net/MessageDataProperty"/>
        <rdfs:domain rdf:resource="http://ethon.consensys.net/Tx"/>
        <rdfs:range rdf:resource="http://www.w3.org/2001/XMLSchema#integer"/>
        <suggestedStringRepresentation>txNonce</suggestedStringRepresentation>
        <rdfs:comment xml:lang="en">A scalar value equal to the number of transactions sent by the sender.</rdfs:comment>
        <rdfs:label xml:lang="en">Transaction nonce</rdfs:label>
        <ns:term_status>unstable</ns:term_status>
    </owl:DatatypeProperty>



    <!-- http://ethon.consensys.net/txR -->

    <owl:DatatypeProperty rdf:about="http://ethon.consensys.net/txR">
        <rdfs:subPropertyOf rdf:resource="http://ethon.consensys.net/MessageDataProperty"/>
        <rdfs:domain rdf:resource="http://ethon.consensys.net/Tx"/>
        <rdfs:range rdf:resource="http://www.w3.org/2001/XMLSchema#hexBinary"/>
        <suggestedStringRepresentation>txR</suggestedStringRepresentation>
        <rdfs:comment xml:lang="en">The values txV, txR and txS correspond to the signature of the transaction and are used to determine the sender of the transaction. The txR value is a Byte array of length 32.</rdfs:comment>
        <rdfs:label xml:lang="en">Transaction r-value</rdfs:label>
        <ns:term_status>unstable</ns:term_status>
    </owl:DatatypeProperty>



    <!-- http://ethon.consensys.net/txS -->

    <owl:DatatypeProperty rdf:about="http://ethon.consensys.net/txS">
        <rdfs:subPropertyOf rdf:resource="http://ethon.consensys.net/MessageDataProperty"/>
        <rdfs:domain rdf:resource="http://ethon.consensys.net/Tx"/>
        <rdfs:range rdf:resource="http://www.w3.org/2001/XMLSchema#hexBinary"/>
        <suggestedStringRepresentation>txS</suggestedStringRepresentation>
        <rdfs:comment xml:lang="en">The values txV, txR and txS correspond to the signature of the transaction and are used to determine the sender of the transaction. The value txS is a byte array of length 32.</rdfs:comment>
        <rdfs:label xml:lang="en">Transaction s-value</rdfs:label>
        <ns:term_status>unstable</ns:term_status>
    </owl:DatatypeProperty>



    <!-- http://ethon.consensys.net/txV -->

    <owl:DatatypeProperty rdf:about="http://ethon.consensys.net/txV">
        <rdfs:subPropertyOf rdf:resource="http://ethon.consensys.net/MessageDataProperty"/>
        <rdfs:domain rdf:resource="http://ethon.consensys.net/Tx"/>
        <rdfs:range rdf:resource="http://www.w3.org/2001/XMLSchema#byte"/>
        <suggestedStringRepresentation>txV</suggestedStringRepresentation>
        <rdfs:comment xml:lang="en">The values txV, txR and txS correspond to the signature of the transaction and are used to determine the sender of the transaction. The value txV specifies the sign and finiteness of the curve point. Since EIP-155 it is used to realize a replay attack protection. It is calculated in the following way: txV = CHAIN_ID * 2 + 36</rdfs:comment>
        <rdfs:label xml:lang="en">Transaction v-value</rdfs:label>
        <rdfs:seeAlso rdf:resource="https://github.com/ethereum/EIPs/issues/155"/>
        <ns:term_status>unstable</ns:term_status>
    </owl:DatatypeProperty>



    <!-- http://ethon.consensys.net/uncleBeneficiaryReward -->

    <owl:DatatypeProperty rdf:about="http://ethon.consensys.net/uncleBeneficiaryReward">
        <rdfs:subPropertyOf rdf:resource="http://ethon.consensys.net/BlockDataProperty"/>
        <rdf:type rdf:resource="http://www.w3.org/2002/07/owl#FunctionalProperty"/>
        <rdfs:domain rdf:resource="http://ethon.consensys.net/Uncle"/>
        <rdfs:range rdf:resource="http://www.w3.org/2001/XMLSchema#integer"/>
        <suggestedStringRepresentation>uncleBenficiaryReward</suggestedStringRepresentation>
        <rdfs:comment xml:lang="en">The reward the beneficiary of an uncle receives if a block includes it. The reward amount depends how far up the Uncle is in the blockchain (the number of the block in which it is included minus the uncle&apos;s number). An uncle reward is only paid if the distance is smaller than 8. For a distance of 1 the reward is 7/8 of the block reward, for a distance of 7 the reward is 1/8 of the block reward.</rdfs:comment>
        <rdfs:label xml:lang="en">Uncle beneficiary reward</rdfs:label>
        <ns:term_status>unstable</ns:term_status>
    </owl:DatatypeProperty>



    <!-- http://ethon.consensys.net/value -->

    <owl:DatatypeProperty rdf:about="http://ethon.consensys.net/value">
        <rdfs:subPropertyOf rdf:resource="http://ethon.consensys.net/MessageDataProperty"/>
        <rdf:type rdf:resource="http://www.w3.org/2002/07/owl#FunctionalProperty"/>
        <rdfs:domain rdf:resource="http://ethon.consensys.net/Msg"/>
        <rdfs:range rdf:resource="http://www.w3.org/2001/XMLSchema#integer"/>
        <suggestedStringRepresentation>value</suggestedStringRepresentation>
        <rdfs:comment xml:lang="en">A scalar value equal to the number of Wei to be transferred to the Message call&apos;s recipient. In the case of contract creation it is the initial balance of the contract account, paid by the sending account.</rdfs:comment>
        <rdfs:label xml:lang="en">value in Wei</rdfs:label>
        <ns:term_status>unstable</ns:term_status>
    </owl:DatatypeProperty>



    <!--
    ///////////////////////////////////////////////////////////////////////////////////////
    //
    // Classes
    //
    ///////////////////////////////////////////////////////////////////////////////////////
     -->




    <!-- http://ethon.consensys.net/Account -->

    <owl:Class rdf:about="http://ethon.consensys.net/Account">
        <rdfs:subClassOf rdf:resource="http://ethon.consensys.net/AccountConcept"/>
        <rdfs:subClassOf>
            <owl:Restriction>
                <owl:onProperty rdf:resource="http://ethon.consensys.net/hasState"/>
                <owl:someValuesFrom rdf:resource="http://ethon.consensys.net/AccountState"/>
            </owl:Restriction>
        </rdfs:subClassOf>
        <rdfs:subClassOf>
            <owl:Restriction>
                <owl:onProperty rdf:resource="http://ethon.consensys.net/address"/>
                <owl:qualifiedCardinality rdf:datatype="http://www.w3.org/2001/XMLSchema#nonNegativeInteger">1</owl:qualifiedCardinality>
                <owl:onDataRange rdf:resource="http://www.w3.org/2001/XMLSchema#hexBinary"/>
            </owl:Restriction>
        </rdfs:subClassOf>
        <owl:hasKey rdf:parseType="Collection">
            <rdf:Description rdf:about="http://ethon.consensys.net/address"/>
        </owl:hasKey>
        <simpleDefinition>There are two main types of accounts: external accounts (often referred to as "wallet" or simply "account") and contract accounts (usually just called "contract" or "smart contract"). An external account is what you need to use Ethereum. It is usually protected by a password. If you have the password you can send Ether from your account to another or use a contract. It has an Ethereum address (0x...) by which it is identified.</simpleDefinition>
        <suggestedStringRepresentation xml:lang="en">Account</suggestedStringRepresentation>
        <rdfs:comment xml:lang="en">*Account* is the superclass of all account types in Ethereum. All accounts are identified by an address (which, however, is derived differently for external and contract accounts) and an account state that contains the contract's balance and total message count, which is called its nonce. Contract accounts also have an associated storage state and EVM code. The address of an external account is derived from the public key of a public and private keypair, while a contract account address is a concatenation of the creator account&apos;s address and its nonce. Both contract accounts and external accounts can also be of type *protocol account* if they are specified in the Ethereum blockchain, i.e. the accounts pre-funded by the Ethereum crowdsale.</rdfs:comment>
        <rdfs:label xml:lang="en">Account</rdfs:label>
        <ns:term_status>unstable</ns:term_status>
    </owl:Class>
    <owl:Axiom>
        <owl:annotatedSource rdf:resource="http://ethon.consensys.net/Account"/>
        <owl:annotatedProperty rdf:resource="http://www.w3.org/2000/01/rdf-schema#subClassOf"/>
        <owl:annotatedTarget>
            <owl:Restriction>
                <owl:onProperty rdf:resource="http://ethon.consensys.net/hasState"/>
                <owl:someValuesFrom rdf:resource="http://ethon.consensys.net/AccountState"/>
            </owl:Restriction>
        </owl:annotatedTarget>
        <rdfs:comment xml:lang="en">An Account must have at least 1 state.</rdfs:comment>
    </owl:Axiom>
    <owl:Axiom>
        <owl:annotatedSource rdf:resource="http://ethon.consensys.net/Account"/>
        <owl:annotatedProperty rdf:resource="http://www.w3.org/2002/07/owl#hasKey"/>
        <owl:annotatedTarget rdf:parseType="Collection">
            <rdf:Description rdf:about="http://ethon.consensys.net/address"/>
        </owl:annotatedTarget>
        <rdfs:comment xml:lang="en">An Address is the unique 160-bit identifier of an Account.</rdfs:comment>
    </owl:Axiom>



    <!-- http://ethon.consensys.net/AccountConcept -->

    <owl:Class rdf:about="http://ethon.consensys.net/AccountConcept">
        <rdfs:subClassOf rdf:resource="http://ethon.consensys.net/EthOnConcept"/>
        <suggestedStringRepresentation xml:lang="en">AccountConcept</suggestedStringRepresentation>
        <rdfs:comment xml:lang="en">The group of all EthOn classes related to accounts.</rdfs:comment>
        <rdfs:label xml:lang="en">EthOn Account concept</rdfs:label>
        <ns:term_status>unstable</ns:term_status>
    </owl:Class>



    <!-- http://ethon.consensys.net/AccountState -->

    <owl:Class rdf:about="http://ethon.consensys.net/AccountState">
        <rdfs:subClassOf rdf:resource="http://ethon.consensys.net/AccountConcept"/>
        <rdfs:subClassOf rdf:resource="http://ethon.consensys.net/State"/>
        <suggestedStringRepresentation xml:lang="en">AccountState</suggestedStringRepresentation>
        <rdfs:comment xml:lang="en">State of an Ethereum account. It is comprised on four pieces of information: nonce, balance, storage root and code hash. The data is stored in a Merkle Patricia tree as a mapping between addresses and account states. The account state is part of the world state, as it resembles the state of exactly one account.</rdfs:comment>
        <rdfs:label xml:lang="en">Account State</rdfs:label>
        <ns:term_status>unstable</ns:term_status>
    </owl:Class>



    <!-- http://ethon.consensys.net/AccountStorage -->

    <owl:Class rdf:about="http://ethon.consensys.net/AccountStorage">
        <rdfs:subClassOf rdf:resource="http://ethon.consensys.net/AccountConcept"/>
        <rdfs:subClassOf rdf:resource="http://ethon.consensys.net/ModifiedMerklePatriciaTree"/>
        <simpleDefinition>A data structure which contains the current storage state of a smart contract, i.e. the total supply of an ERC20 token and the mapping of account addresses to current balances.</simpleDefinition>
        <suggestedStringRepresentation xml:lang="en">AccountStorage</suggestedStringRepresentation>
        <rdfs:comment xml:lang="en">The account storage is part of the account state and it contains contains the values of all variables defined in the contract's code at a certain point in time. Usually Ethereum clients implement this structure as a Merkle Patricia Tree. Whenever any of the contract's variables are changed a new state is created.</rdfs:comment>
        <rdfs:label xml:lang="en">Storage</rdfs:label>
        <ns:term_status>unstable</ns:term_status>
    </owl:Class>



    <!-- http://ethon.consensys.net/Block -->

    <owl:Class rdf:about="http://ethon.consensys.net/Block">
        <rdfs:subClassOf rdf:resource="http://ethon.consensys.net/BlockConcept"/>
        <rdfs:subClassOf rdf:resource="http://ethon.consensys.net/StateTransition"/>
        <owl:hasKey rdf:parseType="Collection">
            <rdf:Description rdf:about="http://ethon.consensys.net/blockHash"/>
        </owl:hasKey>
        <simpleDefinition>A block is an entry in a blockchain. It contains a series of transactions as well as a cryptographic hash linking it to the previous block in the chain.</simpleDefinition>
        <suggestedStringRepresentation xml:lang="en">Block</suggestedStringRepresentation>
        <rdfs:comment xml:lang="en">A block is the basic element of a &apos;blockchain&apos;. It functions as an entry in a distributed ledger, recording a series of transactions together with a reference to the previous block. A block is chained to its preceeding block by a cryptographic hash of its contents as a means of reference. Blocks contain an identifier for the final state after all transactions contained in it are validated. There is a consensus mechanism that provides incentives for nodes adding new blocks to the chain (&quot;miners&quot; in the Proof of Work protocol used by the main Ethereum network) that comply with the rules of Ethereum by issuing newly generated tokens (&apos;Ether&apos;) to an account specified by the block's author.</rdfs:comment>
        <rdfs:label xml:lang="en">Block</rdfs:label>
        <ns:term_status>unstable</ns:term_status>
    </owl:Class>
    <owl:Axiom>
        <owl:annotatedSource rdf:resource="http://ethon.consensys.net/Block"/>
        <owl:annotatedProperty rdf:resource="http://www.w3.org/2000/01/rdf-schema#subClassOf"/>
        <owl:annotatedTarget rdf:resource="http://ethon.consensys.net/StateTransition"/>
        <DASE_RULE rdf:datatype="http://www.w3.org/2001/XMLSchema#string">YP-2.1___Block(?x)-&gt;StateTransition(?x)___A valid State Transition is one which comes about through a Block.</DASE_RULE>
    </owl:Axiom>
    <owl:Axiom>
        <owl:annotatedSource rdf:resource="http://ethon.consensys.net/Block"/>
        <owl:annotatedProperty rdf:resource="http://www.w3.org/2002/07/owl#hasKey"/>
        <owl:annotatedTarget rdf:parseType="Collection">
            <rdf:Description rdf:about="http://ethon.consensys.net/blockHash"/>
        </owl:annotatedTarget>
        <rdfs:comment xml:lang="en">The blockHash is the unique identifier of a block. It is generated via the Keccak 256-bit hash of its block header.</rdfs:comment>
    </owl:Axiom>



    <!-- http://ethon.consensys.net/BlockConcept -->

    <owl:Class rdf:about="http://ethon.consensys.net/BlockConcept">
        <rdfs:subClassOf rdf:resource="http://ethon.consensys.net/EthOnConcept"/>
        <suggestedStringRepresentation xml:lang="en">BlockConcept</suggestedStringRepresentation>
        <rdfs:comment xml:lang="en">The group of all EthOn classes related to blocks.</rdfs:comment>
        <rdfs:label xml:lang="en">EthOn Block concept</rdfs:label>
        <ns:term_status>unstable</ns:term_status>
    </owl:Class>



    <!-- http://ethon.consensys.net/Blockchain -->

    <owl:Class rdf:about="http://ethon.consensys.net/Blockchain">
        <rdfs:subClassOf rdf:resource="http://ethon.consensys.net/NetworkConcept"/>
        <suggestedStringRepresentation>Blockchain</suggestedStringRepresentation>
        <rdfs:comment xml:lang="en">An Ethereum blockchain is a distributed database that maintains a continuously-growing list of records called *blocks* secured from tampering and revision. Each block contains a timestamp and a link to a previous block in a Merkle tree structure.</rdfs:comment>
        <rdfs:label xml:lang="en">Ethereum Blockchain</rdfs:label>
        <ns:term_status>unstable</ns:term_status>
    </owl:Class>



    <!-- http://ethon.consensys.net/CallContractMsg -->

    <owl:Class rdf:about="http://ethon.consensys.net/CallContractMsg">
        <rdfs:subClassOf rdf:resource="http://ethon.consensys.net/ContractMsg"/>
        <rdfs:subClassOf>
            <owl:Restriction>
                <owl:onProperty rdf:resource="http://ethon.consensys.net/to"/>
                <owl:qualifiedCardinality rdf:datatype="http://www.w3.org/2001/XMLSchema#nonNegativeInteger">1</owl:qualifiedCardinality>
                <owl:onClass rdf:resource="http://ethon.consensys.net/ContractAccount"/>
            </owl:Restriction>
        </rdfs:subClassOf>
        <suggestedStringRepresentation>CallContractMsg</suggestedStringRepresentation>
        <rdfs:comment xml:lang="en">A call contract message is a contract message that calls a function in another contract.</rdfs:comment>
        <rdfs:label xml:lang="en">Call Contract Message</rdfs:label>
        <ns:term_status>unstable</ns:term_status>
    </owl:Class>
    <owl:Axiom>
        <owl:annotatedSource rdf:resource="http://ethon.consensys.net/CallContractMsg"/>
        <owl:annotatedProperty rdf:resource="http://www.w3.org/2000/01/rdf-schema#subClassOf"/>
        <owl:annotatedTarget>
            <owl:Restriction>
                <owl:onProperty rdf:resource="http://ethon.consensys.net/to"/>
                <owl:qualifiedCardinality rdf:datatype="http://www.w3.org/2001/XMLSchema#nonNegativeInteger">1</owl:qualifiedCardinality>
                <owl:onClass rdf:resource="http://ethon.consensys.net/ContractAccount"/>
            </owl:Restriction>
        </owl:annotatedTarget>
        <rdfs:comment>Call contract accounts call functions in other contract accounts.</rdfs:comment>
    </owl:Axiom>



    <!-- http://ethon.consensys.net/CallTx -->

    <owl:Class rdf:about="http://ethon.consensys.net/CallTx">
        <rdfs:subClassOf rdf:resource="http://ethon.consensys.net/Tx"/>
        <rdfs:subClassOf>
            <owl:Restriction>
                <owl:onProperty rdf:resource="http://ethon.consensys.net/to"/>
                <owl:qualifiedCardinality rdf:datatype="http://www.w3.org/2001/XMLSchema#nonNegativeInteger">1</owl:qualifiedCardinality>
                <owl:onClass rdf:resource="http://ethon.consensys.net/ContractAccount"/>
            </owl:Restriction>
        </rdfs:subClassOf>
        <suggestedStringRepresentation>CallTx</suggestedStringRepresentation>
        <rdfs:comment xml:lang="en">A type of transaction that is directed towards a contract account and calls a method in the contract&apos;s code.</rdfs:comment>
        <rdfs:label xml:lang="en">Call Transaction</rdfs:label>
        <ns:term_status>unstable</ns:term_status>
    </owl:Class>
    <owl:Axiom>
        <owl:annotatedSource rdf:resource="http://ethon.consensys.net/CallTx"/>
        <owl:annotatedProperty rdf:resource="http://www.w3.org/2000/01/rdf-schema#subClassOf"/>
        <owl:annotatedTarget>
            <owl:Restriction>
                <owl:onProperty rdf:resource="http://ethon.consensys.net/to"/>
                <owl:qualifiedCardinality rdf:datatype="http://www.w3.org/2001/XMLSchema#nonNegativeInteger">1</owl:qualifiedCardinality>
                <owl:onClass rdf:resource="http://ethon.consensys.net/ContractAccount"/>
            </owl:Restriction>
        </owl:annotatedTarget>
        <rdfs:comment>Call transactions are directed towards a contract account.</rdfs:comment>
    </owl:Axiom>



    <!-- http://ethon.consensys.net/ContractAccount -->

    <owl:Class rdf:about="http://ethon.consensys.net/ContractAccount">
        <rdfs:subClassOf rdf:resource="http://ethon.consensys.net/Account"/>
        <owl:disjointWith rdf:resource="http://ethon.consensys.net/ExternalAccount"/>
        <simpleDefinition>A type of Ethereum account that represents a smart contract. Its behaviour is controlled by the logic in the smart contract's code. Like external accounts it is identified by an address.</simpleDefinition>
        <suggestedStringRepresentation xml:lang="en">ContractAccount</suggestedStringRepresentation>
        <rdfs:comment xml:lang="en">One of the two main types of accounts on Ethereum, a contract account is an account whose behaviour is controlled by a smart contract. Contract accounts are identified by their address which is derived from the creator account's address and nonce. A contract account has a non-empty associated EVM code. It's state data consists of the bytecode, the contract's balance and the storage state of the contract's code (for example the value of variables). A contract account can only act when it is triggered by a message. It may not create and sign transactions, but it can receive transactions from external accounts as well as send and receive contract messages, which may involve a transfer of Ether. Contract accounts can also contain events which create log entries when triggered.</rdfs:comment>        <rdfs:label xml:lang="en">Contract Account</rdfs:label>
        <ns:term_status>unstable</ns:term_status>
    </owl:Class>



    <!-- http://ethon.consensys.net/ContractMsg -->

    <owl:Class rdf:about="http://ethon.consensys.net/ContractMsg">
        <rdfs:subClassOf rdf:resource="http://ethon.consensys.net/Msg"/>
        <rdfs:subClassOf>
            <owl:Restriction>
                <owl:onProperty rdf:resource="http://ethon.consensys.net/from"/>
                <owl:qualifiedCardinality rdf:datatype="http://www.w3.org/2001/XMLSchema#nonNegativeInteger">1</owl:qualifiedCardinality>
                <owl:onClass rdf:resource="http://ethon.consensys.net/ContractAccount"/>
            </owl:Restriction>
        </rdfs:subClassOf>
        <suggestedStringRepresentation>ContractMsg</suggestedStringRepresentation>
        <rdfs:comment xml:lang="en">A contract message is passed between a contract account and any other account (external or contract). It is the result of an execution chain originally triggered by an external eccount.</rdfs:comment>
        <rdfs:label xml:lang="en">Contract Message</rdfs:label>
        <ns:term_status>unstable</ns:term_status>
    </owl:Class>
    <owl:Axiom>
        <owl:annotatedSource rdf:resource="http://ethon.consensys.net/ContractMsg"/>
        <owl:annotatedProperty rdf:resource="http://www.w3.org/2000/01/rdf-schema#subClassOf"/>
        <owl:annotatedTarget>
            <owl:Restriction>
                <owl:onProperty rdf:resource="http://ethon.consensys.net/from"/>
                <owl:qualifiedCardinality rdf:datatype="http://www.w3.org/2001/XMLSchema#nonNegativeInteger">1</owl:qualifiedCardinality>
                <owl:onClass rdf:resource="http://ethon.consensys.net/ContractAccount"/>
            </owl:Restriction>
        </owl:annotatedTarget>
        <rdfs:comment>Contract messages originate from contract accounts.</rdfs:comment>
    </owl:Axiom>



    <!-- http://ethon.consensys.net/CreateContractMsg -->

    <owl:Class rdf:about="http://ethon.consensys.net/CreateContractMsg">
        <rdfs:subClassOf rdf:resource="http://ethon.consensys.net/ContractMsg"/>
        <rdfs:subClassOf>
            <owl:Restriction>
                <owl:onProperty rdf:resource="http://ethon.consensys.net/creates"/>
                <owl:qualifiedCardinality rdf:datatype="http://www.w3.org/2001/XMLSchema#nonNegativeInteger">1</owl:qualifiedCardinality>
                <owl:onClass rdf:resource="http://ethon.consensys.net/ContractAccount"/>
            </owl:Restriction>
        </rdfs:subClassOf>
        <suggestedStringRepresentation>CreateContractMsg</suggestedStringRepresentation>
        <rdfs:comment xml:lang="en">A create contract message is a subtype of a contract message that results in creation of a new contract account.</rdfs:comment>
        <rdfs:label xml:lang="en">Create Contract Message</rdfs:label>
        <ns:term_status>unstable</ns:term_status>
    </owl:Class>
    <owl:Axiom>
        <owl:annotatedSource rdf:resource="http://ethon.consensys.net/CreateContractMsg"/>
        <owl:annotatedProperty rdf:resource="http://www.w3.org/2000/01/rdf-schema#subClassOf"/>
        <owl:annotatedTarget>
            <owl:Restriction>
                <owl:onProperty rdf:resource="http://ethon.consensys.net/creates"/>
                <owl:qualifiedCardinality rdf:datatype="http://www.w3.org/2001/XMLSchema#nonNegativeInteger">1</owl:qualifiedCardinality>
                <owl:onClass rdf:resource="http://ethon.consensys.net/ContractAccount"/>
            </owl:Restriction>
        </owl:annotatedTarget>
        <rdfs:comment>Create contract messages create contract accounts.</rdfs:comment>
    </owl:Axiom>



    <!-- http://ethon.consensys.net/CreateTx -->

    <owl:Class rdf:about="http://ethon.consensys.net/CreateTx">
        <rdfs:subClassOf rdf:resource="http://ethon.consensys.net/Tx"/>
        <rdfs:subClassOf>
            <owl:Restriction>
                <owl:onProperty rdf:resource="http://ethon.consensys.net/creates"/>
                <owl:qualifiedCardinality rdf:datatype="http://www.w3.org/2001/XMLSchema#nonNegativeInteger">1</owl:qualifiedCardinality>
                <owl:onClass rdf:resource="http://ethon.consensys.net/ContractAccount"/>
            </owl:Restriction>
        </rdfs:subClassOf>
        <suggestedStringRepresentation>CreateTx</suggestedStringRepresentation>
        <rdfs:comment xml:lang="en">A type of transaction that results in creation of a new contract account.</rdfs:comment>
        <rdfs:label xml:lang="en">Create Transaction</rdfs:label>
        <ns:term_status>unstable</ns:term_status>
    </owl:Class>
    <owl:Axiom>
        <owl:annotatedSource rdf:resource="http://ethon.consensys.net/CreateTx"/>
        <owl:annotatedProperty rdf:resource="http://www.w3.org/2000/01/rdf-schema#subClassOf"/>
        <owl:annotatedTarget>
            <owl:Restriction>
                <owl:onProperty rdf:resource="http://ethon.consensys.net/creates"/>
                <owl:qualifiedCardinality rdf:datatype="http://www.w3.org/2001/XMLSchema#nonNegativeInteger">1</owl:qualifiedCardinality>
                <owl:onClass rdf:resource="http://ethon.consensys.net/ContractAccount"/>
            </owl:Restriction>
        </owl:annotatedTarget>
        <rdfs:comment>All create transactions are directed toward a contract account they create.</rdfs:comment>
    </owl:Axiom>



    <!-- http://ethon.consensys.net/EthOnConcept -->

    <owl:Class rdf:about="http://ethon.consensys.net/EthOnConcept">
        <suggestedStringRepresentation xml:lang="en">EthonConcept</suggestedStringRepresentation>
        <rdfs:comment xml:lang="en">Groups all classes and subclasses that are original to the EthOn OWL ontology.</rdfs:comment>
        <rdfs:label xml:lang="en">EthOn Concept</rdfs:label>
        <ns:term_status>unstable</ns:term_status>
    </owl:Class>



    <!-- http://ethon.consensys.net/ExternalAccount -->

    <owl:Class rdf:about="http://ethon.consensys.net/ExternalAccount">
        <rdfs:subClassOf rdf:resource="http://ethon.consensys.net/Account"/>
        <simpleDefinition>An Ethereum account usually controlled by a person. It is identified by an address (0x...) and a public/private key-pair.</simpleDefinition>
        <suggestedStringRepresentation xml:lang="en">ExternalAccount</suggestedStringRepresentation>
        <rdfs:comment xml:lang="en">One of the two main types of accounts on Ethereum, an external account is an account controlled by an external actor (as opposed to a contract account). The unique identifier of an external account is its address. It consists of the rightmost 160 bits of the keccak 256 hash of its public key (example: 0x1a1138875dAB9E0AC8b0fd4a37EEAC5eb26B870B). There is only one way external accounts can actively change the state of the blockchain. They can be used to send a valid transaction to the Ethereum blockchain. The transaction can be directed towards other external accounts or towards contract accounts. Since the private key is needed for sending, a valid transaction can only be created by the person or entity controlling the private key of the external account. Besides being target of transactions, external accounts can also be the target of contract messages, block beneficiary rewards, uncle beneficiary rewards or payouts of contract accounts that have self-destructed.</rdfs:comment>
        <rdfs:label xml:lang="en">Externally Controlled Account</rdfs:label>
        <ns:term_status>unstable</ns:term_status>
    </owl:Class>



    <!-- http://ethon.consensys.net/ExternalActor -->

    <owl:Class rdf:about="http://ethon.consensys.net/ExternalActor">
        <rdfs:subClassOf rdf:resource="http://ethon.consensys.net/AccountConcept"/>
        <rdfs:subClassOf rdf:resource="http://xmlns.com/foaf/0.1/Agent"/>
        <suggestedStringRepresentation xml:lang="en">ExternalActor</suggestedStringRepresentation>
        <rdfs:comment xml:lang="en">A person or other entity able to interface to an Ethereum node, but external to the world of Ethereum. It can interact with Ethereum through depositing signed transactions and inspecting the blockchain and associated state. Has one (or more) intrinsic accounts. While it is assumed that the ultimate external actor will be human in nature, software tools will be used in its construction and dissemination.</rdfs:comment>
        <rdfs:label xml:lang="en">External Actor</rdfs:label>
        <ns:term_status>unstable</ns:term_status>
    </owl:Class>



    <!-- http://ethon.consensys.net/FullNode -->

    <owl:Class rdf:about="http://ethon.consensys.net/FullNode">
        <rdfs:subClassOf rdf:resource="http://ethon.consensys.net/Node"/>
        <owl:disjointWith rdf:resource="http://ethon.consensys.net/LightNode"/>
        <simpleDefinition>A piece of software which connects fully to an Ethereum network, storing its complete history and having the ability to submit new blocks to the blockchain (i.e. through mining).</simpleDefinition>
        <suggestedStringRepresentation>FullNode</suggestedStringRepresentation>
        <rdfs:comment xml:lang="en">A full node is a participant in an Ethereum network that keeps a record of the full blockchain, the full state and may engage in mining.</rdfs:comment>
        <rdfs:label xml:lang="en">Ethereum Full Node</rdfs:label>
        <ns:term_status>unstable</ns:term_status>
    </owl:Class>



    <!-- http://ethon.consensys.net/GenesisBlock -->

    <owl:Class rdf:about="http://ethon.consensys.net/GenesisBlock">
        <rdfs:subClassOf rdf:resource="http://ethon.consensys.net/Block"/>
        <suggestedStringRepresentation>GenesisBlock</suggestedStringRepresentation>
        <rdfs:comment xml:lang="en">A genesis block is the unmined, deliberately created, very first block in a blockchain. It has no predecessors, i.e. no parent block.</rdfs:comment>
        <rdfs:label xml:lang="en">Genesis Block</rdfs:label>
        <ns:term_status>unstable</ns:term_status>
    </owl:Class>



    <!-- http://ethon.consensys.net/LightNode -->

    <owl:Class rdf:about="http://ethon.consensys.net/LightNode">
        <rdfs:subClassOf rdf:resource="http://ethon.consensys.net/Node"/>
        <simpleDefinition>A piece of software which connects to an Ethereum network in a limited capacity, i.e. a smart phone wallet app which neither mines nor downloads the full blockchain, but can still send and receive messages.</simpleDefinition>
        <suggestedStringRepresentation>LightNode</suggestedStringRepresentation>
        <rdfs:comment xml:lang="en">A light node is a participant in an Ethereum network that does not completely do any of the following: store the complete blockchain, store the complete world state, engage in mining.</rdfs:comment>
        <rdfs:label xml:lang="en">Ethereum Light Node</rdfs:label>
        <ns:term_status>unstable</ns:term_status>
    </owl:Class>



    <!-- http://ethon.consensys.net/LogEntry -->

    <owl:Class rdf:about="http://ethon.consensys.net/LogEntry">
        <rdfs:subClassOf rdf:resource="http://ethon.consensys.net/MessageConcept"/>
        <suggestedStringRepresentation>LogEntry</suggestedStringRepresentation>
        <rdfs:comment xml:lang="en">A log ntry is the result of an event in a smart contract, emitted during creation or execution of a contract account&apos;s code. It is related to the TxReceipt it was created in, the contract account that had the event, a series of 32-bytes log topics and a number of bytes of data.</rdfs:comment>
        <rdfs:label xml:lang="en">Log Entry</rdfs:label>
        <ns:term_status>unstable</ns:term_status>
    </owl:Class>



    <!-- http://ethon.consensys.net/LogTopic -->

    <owl:Class rdf:about="http://ethon.consensys.net/LogTopic">
        <rdfs:subClassOf rdf:resource="http://ethon.consensys.net/MessageConcept"/>
        <suggestedStringRepresentation>LogTopic</suggestedStringRepresentation>
        <rdfs:comment xml:lang="en">A 32-bytes long topic of a log entry. The log topics of a log entry have an order given by a topic index value.</rdfs:comment>
        <rdfs:label xml:lang="en">Log Topic</rdfs:label>
        <ns:term_status>unstable</ns:term_status>
    </owl:Class>



    <!-- http://ethon.consensys.net/MessageConcept -->

    <owl:Class rdf:about="http://ethon.consensys.net/MessageConcept">
        <rdfs:subClassOf rdf:resource="http://ethon.consensys.net/EthOnConcept"/>
        <rdfs:comment xml:lang="en">The group of all EthOn classes related to messages.</rdfs:comment>
        <rdfs:label xml:lang="en">EthOn Message concept</rdfs:label>
        <ns:term_status>unstable</ns:term_status>
    </owl:Class>



    <!-- http://ethon.consensys.net/ModifiedMerklePatriciaTree -->

    <owl:Class rdf:about="http://ethon.consensys.net/ModifiedMerklePatriciaTree">
        <rdfs:subClassOf rdf:resource="http://ethon.consensys.net/EthOnConcept"/>
        <suggestedStringRepresentation xml:lang="en">ModifiedMerklePatriciaTree</suggestedStringRepresentation>
        <rdfs:comment xml:lang="en">Merkle Patricia trees provide a cryptographically authenticated data structure that can be used to store all (key, value) bindings, although for the scope of this paper we are restricting keys and values to strings (to remove this restriction, just use any serialization format for other data types). They are fully deterministic, meaning that a Patricia tree with the same (key,value) bindings is guaranteed to be exactly the same down to the last byte and therefore have the same root hash, provide the holy grail of O(log(n)) efficiency for inserts, lookups and deletes, and are much easier to understand and code than more complex comparison-based alternatives like red-black trees.</rdfs:comment>
        <rdfs:label xml:lang="en">Merkle Patricia Tree</rdfs:label>
        <rdfs:seeAlso rdf:resource="https://github.com/ethereum/wiki/wiki/Patricia-Tree"/>
        <ns:term_status>unstable</ns:term_status>
    </owl:Class>



    <!-- http://ethon.consensys.net/Msg -->

    <owl:Class rdf:about="http://ethon.consensys.net/Msg">
        <rdfs:subClassOf rdf:resource="http://ethon.consensys.net/MessageConcept"/>
        <rdfs:subClassOf rdf:resource="http://ethon.consensys.net/StateTransition"/>
        <suggestedStringRepresentation>Msg</suggestedStringRepresentation>
        <rdfs:comment xml:lang="en">Data (as a set of bytes) and value (specified as Ether) that is passed between two accounts, either through the deterministic operation of an autonomous object (contract account) or the cryptographically secure signature of an external account.</rdfs:comment>
        <rdfs:label xml:lang="en">Message</rdfs:label>
        <ns:term_status>unstable</ns:term_status>
    </owl:Class>
    <owl:Axiom>
        <owl:annotatedSource rdf:resource="http://ethon.consensys.net/Msg"/>
        <owl:annotatedProperty rdf:resource="http://www.w3.org/2000/01/rdf-schema#subClassOf"/>
        <owl:annotatedTarget rdf:resource="http://ethon.consensys.net/StateTransition"/>
        <DASE_RULE rdf:datatype="http://www.w3.org/2001/XMLSchema#string">YP-1.1___Msg(?x)-&gt;StateTransition(?x)___A valid State Transition is one which comes about through a Message.</DASE_RULE>
    </owl:Axiom>



    <!-- http://ethon.consensys.net/Network -->

    <owl:Class rdf:about="http://ethon.consensys.net/Network">
        <rdfs:subClassOf rdf:resource="http://ethon.consensys.net/NetworkConcept"/>
        <suggestedStringRepresentation>Network</suggestedStringRepresentation>
        <rdfs:comment xml:lang="en">An Ethereum network is the group of all nodes that conform to a certain protocol variant.</rdfs:comment>
        <rdfs:label xml:lang="en">Ethereum Network</rdfs:label>
        <ns:term_status>unstable</ns:term_status>
    </owl:Class>



    <!-- http://ethon.consensys.net/NetworkConcept -->

    <owl:Class rdf:about="http://ethon.consensys.net/NetworkConcept">
        <rdfs:subClassOf rdf:resource="http://ethon.consensys.net/EthOnConcept"/>
        <suggestedStringRepresentation>NetworkConcept</suggestedStringRepresentation>
        <rdfs:comment xml:lang="en">The group of all EthOn classes related to networks.</rdfs:comment>
        <rdfs:label xml:lang="en">EthOn Network Concept.</rdfs:label>
    </owl:Class>



    <!-- http://ethon.consensys.net/Node -->

    <owl:Class rdf:about="http://ethon.consensys.net/Node">
        <rdfs:subClassOf rdf:resource="http://ethon.consensys.net/NetworkConcept"/>
        <simpleDefinition>A piece of software participating in the Ethereum network.</simpleDefinition>
        <suggestedStringRepresentation>Node</suggestedStringRepresentation>
        <rdfs:comment xml:lang="en">A participant in an Ethereum network, specifically an instance of one of the client implementations, which may be either a full node or a light node.</rdfs:comment>
        <rdfs:label xml:lang="en">Node</rdfs:label>
        <ns:term_status>unstable</ns:term_status>
    </owl:Class>



    <!-- http://ethon.consensys.net/PostBlockState -->

    <owl:Class rdf:about="http://ethon.consensys.net/PostBlockState">
        <rdfs:subClassOf rdf:resource="http://ethon.consensys.net/PostTxState"/>
    </owl:Class>



    <!-- http://ethon.consensys.net/PostMsgState -->

    <owl:Class rdf:about="http://ethon.consensys.net/PostMsgState">
        <rdfs:subClassOf rdf:resource="http://ethon.consensys.net/WorldState"/>
    </owl:Class>



    <!-- http://ethon.consensys.net/PostTxState -->

    <owl:Class rdf:about="http://ethon.consensys.net/PostTxState">
        <rdfs:subClassOf rdf:resource="http://ethon.consensys.net/PostMsgState"/>
    </owl:Class>



    <!-- http://ethon.consensys.net/ProtocolAccount -->

    <owl:Class rdf:about="http://ethon.consensys.net/ProtocolAccount">
        <rdfs:subClassOf rdf:resource="http://ethon.consensys.net/Account"/>
	      <simpleDefinition>An account that was created together with the blockchain itself or during a protcol update and can have an initial balance, e.g. from the crowdfunding of the blockchain.</simpleDefinition>
        <suggestedStringRepresentation xml:lang="en">PrefundedAccount</suggestedStringRepresentation>
        <rdfs:comment xml:lang="en">A protocol account is a type of account in Ethereum. Protocol accounts are specified in the Ethereum protocol, and have so far only been used to store the initial balance for users who participated in the Ethereum crowdsale. Protocol accounts could be added with any protocol change and may be either external accounts or contract accounts.</rdfs:comment>
        <rdfs:label xml:lang="en">Protocol Account</rdfs:label>
        <ns:term_status>unstable</ns:term_status>
    </owl:Class>



    <!-- http://ethon.consensys.net/ProtocolState -->

    <owl:Class rdf:about="http://ethon.consensys.net/ProtocolState">
        <rdfs:subClassOf rdf:resource="http://ethon.consensys.net/AccountState"/>
        <suggestedStringRepresentation xml:lang="en">ProtocolState</suggestedStringRepresentation>
        <rdfs:comment xml:lang="en">This is a special state that can be created after specification of the protocol or any protocol change. It allows for setting balances of accounts, e.g. for prefunded accounts, creating predefined contract accounts with storage or setting any other state property as part of the protocol specification.</rdfs:comment>
        <rdfs:label xml:lang="en">ProtocolState</rdfs:label>
        <ns:term_status>unstable</ns:term_status>
    </owl:Class>



    <!-- http://ethon.consensys.net/ProtocolVariant -->

    <owl:Class rdf:about="http://ethon.consensys.net/ProtocolVariant">
        <rdfs:subClassOf rdf:resource="http://ethon.consensys.net/NetworkConcept"/>
        <suggestedStringRepresentation>EthereumProtocolVariant</suggestedStringRepresentation>
        <rdfs:comment xml:lang="en">A variant of the Ethereum protocol. Changes in the protocol result in a hard or soft fork.</rdfs:comment>
        <rdfs:label xml:lang="en">Ethereum Protocol Variant</rdfs:label>
        <ns:term_status>unstable</ns:term_status>
    </owl:Class>



    <!-- http://ethon.consensys.net/ReceiptsTrie -->

    <owl:Class rdf:about="http://ethon.consensys.net/ReceiptsTrie">
        <rdfs:subClassOf rdf:resource="http://ethon.consensys.net/BlockConcept"/>
        <rdfs:subClassOf rdf:resource="http://ethon.consensys.net/MessageConcept"/>
        <rdfs:subClassOf rdf:resource="http://ethon.consensys.net/ModifiedMerklePatriciaTree"/>
        <suggestedStringRepresentation>ReceiptsTrie</suggestedStringRepresentation>
        <rdfs:comment xml:lang="en">A trie structure that stores transaction receipts. Each block has a reference to the root hash of a receipts trie that stores the receipts of the transactions included in the block.</rdfs:comment>
        <rdfs:label xml:lang="en">Receipts Trie</rdfs:label>
        <ns:term_status>unstable</ns:term_status>
    </owl:Class>



    <!-- http://ethon.consensys.net/SelfdestructContractMsg -->

    <owl:Class rdf:about="http://ethon.consensys.net/SelfdestructContractMsg">
        <rdfs:subClassOf rdf:resource="http://ethon.consensys.net/ContractMsg"/>
        <suggestedStringRepresentation>SelfdestructContractMsg</suggestedStringRepresentation>
        <rdfs:comment xml:lang="en">A selfdestruct contract message is a contract message that deletes the originating contract and refunds its balance to the receiver of the message.</rdfs:comment>
        <rdfs:label xml:lang="en">Selfdestruct Contract Message</rdfs:label>
        <rdfs:seeAlso rdf:resource="https://github.com/ethereum/EIPs/blob/master/EIPS/eip-6.md"/>
        <ns:term_status>unstable</ns:term_status>
    </owl:Class>



    <!-- http://ethon.consensys.net/State -->

    <owl:Class rdf:about="http://ethon.consensys.net/State">
        <rdfs:subClassOf rdf:resource="http://ethon.consensys.net/StateConcept"/>
        <owl:disjointWith rdf:resource="http://ethon.consensys.net/StateTransition"/>
        <suggestedStringRepresentation>State</suggestedStringRepresentation>
        <rdfs:comment xml:lang="en">The concept of a state in a generic state transition system.</rdfs:comment>
        <rdfs:label xml:lang="en">State</rdfs:label>
        <rdfs:seeAlso rdf:resource="https://en.wikipedia.org/wiki/Transition_system"/>
        <rdfs:seeAlso rdf:resource="https://en.wikipedia.org/wiki/State_(computer_science)"/>
        <ns:term_status>unstable</ns:term_status>
    </owl:Class>



    <!-- http://ethon.consensys.net/StateConcept -->

    <owl:Class rdf:about="http://ethon.consensys.net/StateConcept">
        <rdfs:subClassOf rdf:resource="http://ethon.consensys.net/EthOnConcept"/>
        <rdfs:comment xml:lang="en">The group of all EthOn classes related to state.</rdfs:comment>
        <rdfs:label xml:lang="en">EthOn State Concept</rdfs:label>
        <ns:term_status>unstable</ns:term_status>
    </owl:Class>



    <!-- http://ethon.consensys.net/StateTransition -->

    <owl:Class rdf:about="http://ethon.consensys.net/StateTransition">
        <rdfs:subClassOf rdf:resource="http://ethon.consensys.net/StateConcept"/>
        <suggestedStringRepresentation>StateTransition</suggestedStringRepresentation>
        <rdfs:comment xml:lang="en">The concept of a transition in a state transition system.</rdfs:comment>
        <rdfs:label xml:lang="en">State Transition</rdfs:label>
        <rdfs:seeAlso rdf:resource="https://en.wikipedia.org/wiki/Transition_system"/>
        <ns:term_status>unstable</ns:term_status>
    </owl:Class>



    <!-- http://ethon.consensys.net/Tx -->

    <owl:Class rdf:about="http://ethon.consensys.net/Tx">
        <rdfs:subClassOf rdf:resource="http://ethon.consensys.net/Msg"/>
        <rdfs:subClassOf>
            <owl:Restriction>
                <owl:onProperty rdf:resource="http://ethon.consensys.net/from"/>
                <owl:qualifiedCardinality rdf:datatype="http://www.w3.org/2001/XMLSchema#nonNegativeInteger">1</owl:qualifiedCardinality>
                <owl:onClass rdf:resource="http://ethon.consensys.net/ExternalAccount"/>
            </owl:Restriction>
        </rdfs:subClassOf>
        <suggestedStringRepresentation>Tx</suggestedStringRepresentation>
        <rdfs:comment xml:lang="en">Transactions are messages between two accounts that may transfer Ether and may contain a payload. Transactions always originate from an external account that is controlled by an external actor by means of a private key.  The execution of a transaction creates a &apos;transaction receipt&apos;.</rdfs:comment>
        <rdfs:label xml:lang="en">Transaction</rdfs:label>
        <ns:term_status>unstable</ns:term_status>
    </owl:Class>
    <owl:Axiom>
        <owl:annotatedSource rdf:resource="http://ethon.consensys.net/Tx"/>
        <owl:annotatedProperty rdf:resource="http://www.w3.org/2000/01/rdf-schema#subClassOf"/>
        <owl:annotatedTarget rdf:resource="http://ethon.consensys.net/Msg"/>
        <DASE_RULE rdf:datatype="http://www.w3.org/2001/XMLSchema#string">YP-1.2___Tx(?x)-&gt;Msg(?x)___A valid State Transition is one which comes about through a Transaction.</DASE_RULE>
    </owl:Axiom>
    <owl:Axiom>
        <owl:annotatedSource rdf:resource="http://ethon.consensys.net/Tx"/>
        <owl:annotatedProperty rdf:resource="http://www.w3.org/2000/01/rdf-schema#subClassOf"/>
        <owl:annotatedTarget>
            <owl:Restriction>
                <owl:onProperty rdf:resource="http://ethon.consensys.net/from"/>
                <owl:qualifiedCardinality rdf:datatype="http://www.w3.org/2001/XMLSchema#nonNegativeInteger">1</owl:qualifiedCardinality>
                <owl:onClass rdf:resource="http://ethon.consensys.net/ExternalAccount"/>
            </owl:Restriction>
        </owl:annotatedTarget>
        <rdfs:comment>All transactions originate from an external account.</rdfs:comment>
    </owl:Axiom>



    <!-- http://ethon.consensys.net/TxReceipt -->

    <owl:Class rdf:about="http://ethon.consensys.net/TxReceipt">
        <rdfs:subClassOf rdf:resource="http://ethon.consensys.net/MessageConcept"/>
        <suggestedStringRepresentation>TxReceipt</suggestedStringRepresentation>
        <rdfs:comment xml:lang="en">The transaction receipt is a tuple of four items comprising the post-transaction-state, the cumulative gas used in the block containing the transaction receipt as of immediately after the transaction has happened, the set of logs created through execution of the transaction and the bloom filter composed from information in those logs.</rdfs:comment>
        <rdfs:label xml:lang="en">Transaction Receipt</rdfs:label>
        <ns:term_status>unstable</ns:term_status>
    </owl:Class>



    <!-- http://ethon.consensys.net/TxTrie -->

    <owl:Class rdf:about="http://ethon.consensys.net/TxTrie">
        <rdfs:subClassOf rdf:resource="http://ethon.consensys.net/BlockConcept"/>
        <rdfs:subClassOf rdf:resource="http://ethon.consensys.net/MessageConcept"/>
        <rdfs:subClassOf rdf:resource="http://ethon.consensys.net/ModifiedMerklePatriciaTree"/>
        <suggestedStringRepresentation>TxTrie</suggestedStringRepresentation>
        <rdfs:comment xml:lang="en">A trie structure that stores transactions. The header of a block contains a reference to the root of a Tx trie with all transactions contained in the block.</rdfs:comment>
        <rdfs:label xml:lang="en">Transactions Trie</rdfs:label>
        <ns:term_status>unstable</ns:term_status>
    </owl:Class>



    <!-- http://ethon.consensys.net/Uncle -->

    <owl:Class rdf:about="http://ethon.consensys.net/Uncle">
        <rdfs:subClassOf rdf:resource="http://ethon.consensys.net/BlockConcept"/>
        <rdfs:subClassOf>
            <owl:Restriction>
                <owl:onProperty rdf:resource="http://ethon.consensys.net/containsTx"/>
                <owl:qualifiedCardinality rdf:datatype="http://www.w3.org/2001/XMLSchema#nonNegativeInteger">0</owl:qualifiedCardinality>
                <owl:onClass rdf:resource="http://ethon.consensys.net/Tx"/>
            </owl:Restriction>
        </rdfs:subClassOf>
        <suggestedStringRepresentation xml:lang="en">Uncle</suggestedStringRepresentation>
        <rdfs:comment xml:lang="en">An uncle is the direct child of the k&apos;th generation ancestor of a block B, where 2&lt;=k&lt;=7 but not a direct ancestor of B. Uncles are blockchain blocks found by a miner, when a different miner has already found another block for the corresponding place in the blockchain. They are also known as “stale blocks”. The parent of an uncle is an ancestor of the inserting block, located at the tip of the blockchain.</rdfs:comment>
        <rdfs:label xml:lang="en">Uncle</rdfs:label>
        <ns:term_status>unstable</ns:term_status>
    </owl:Class>



    <!-- http://ethon.consensys.net/ValueContractMsg -->

    <owl:Class rdf:about="http://ethon.consensys.net/ValueContractMsg">
        <rdfs:subClassOf rdf:resource="http://ethon.consensys.net/ContractMsg"/>
        <rdfs:subClassOf>
            <owl:Restriction>
                <owl:onProperty rdf:resource="http://ethon.consensys.net/to"/>
                <owl:qualifiedCardinality rdf:datatype="http://www.w3.org/2001/XMLSchema#nonNegativeInteger">1</owl:qualifiedCardinality>
                <owl:onClass rdf:resource="http://ethon.consensys.net/Account"/>
            </owl:Restriction>
        </rdfs:subClassOf>
        <suggestedStringRepresentation>ValueContractMsg</suggestedStringRepresentation>
        <rdfs:comment xml:lang="en">A Value Contract Message is a Contract Message that does not call a function in a smart contract and doesn&apos;t create a new smart contract. Even though it is called &quot;value&quot; Contract Message, it can have a value of 0 Ether. Value Contract Messages can have a payload as long as that payload doesn&apos;t trigger the execution of a function in a smart contract.</rdfs:comment>
        <rdfs:label xml:lang="en">Value Contract Message</rdfs:label>
        <ns:term_status>unstable</ns:term_status>
    </owl:Class>
    <owl:Axiom>
        <owl:annotatedSource rdf:resource="http://ethon.consensys.net/ValueContractMsg"/>
        <owl:annotatedProperty rdf:resource="http://www.w3.org/2000/01/rdf-schema#subClassOf"/>
        <owl:annotatedTarget>
            <owl:Restriction>
                <owl:onProperty rdf:resource="http://ethon.consensys.net/to"/>
                <owl:qualifiedCardinality rdf:datatype="http://www.w3.org/2001/XMLSchema#nonNegativeInteger">1</owl:qualifiedCardinality>
                <owl:onClass rdf:resource="http://ethon.consensys.net/Account"/>
            </owl:Restriction>
        </owl:annotatedTarget>
        <rdfs:comment>Value Contract Messages are always directed to an External Account.</rdfs:comment>
    </owl:Axiom>



    <!-- http://ethon.consensys.net/ValueTx -->

    <owl:Class rdf:about="http://ethon.consensys.net/ValueTx">
        <rdfs:subClassOf rdf:resource="http://ethon.consensys.net/Tx"/>
        <rdfs:subClassOf>
            <owl:Restriction>
                <owl:onProperty rdf:resource="http://ethon.consensys.net/to"/>
                <owl:qualifiedCardinality rdf:datatype="http://www.w3.org/2001/XMLSchema#nonNegativeInteger">1</owl:qualifiedCardinality>
                <owl:onClass rdf:resource="http://ethon.consensys.net/Account"/>
            </owl:Restriction>
        </rdfs:subClassOf>
        <suggestedStringRepresentation>ValueTx</suggestedStringRepresentation>
        <rdfs:comment xml:lang="en">A Value Transaction is a Transaction that does not call a function in a smart contract and doesn&apos;t create a new smart contract. Even though it is called &quot;value&quot; Transaction, Transactions with a value of 0 Ether can be Value Transaction. Value Transactions can have a payload as long as that payload doesn&apos;t trigger the execution of a function in a smart contract.</rdfs:comment>
        <rdfs:label xml:lang="en">Value Transaction</rdfs:label>
        <ns:term_status>unstable</ns:term_status>
    </owl:Class>
    <owl:Axiom>
        <owl:annotatedSource rdf:resource="http://ethon.consensys.net/ValueTx"/>
        <owl:annotatedProperty rdf:resource="http://www.w3.org/2000/01/rdf-schema#subClassOf"/>
        <owl:annotatedTarget>
            <owl:Restriction>
                <owl:onProperty rdf:resource="http://ethon.consensys.net/to"/>
                <owl:qualifiedCardinality rdf:datatype="http://www.w3.org/2001/XMLSchema#nonNegativeInteger">1</owl:qualifiedCardinality>
                <owl:onClass rdf:resource="http://ethon.consensys.net/Account"/>
            </owl:Restriction>
        </owl:annotatedTarget>
        <rdfs:comment>Value transactions are directed to External Accounts.</rdfs:comment>
    </owl:Axiom>



    <!-- http://ethon.consensys.net/WorldState -->

    <owl:Class rdf:about="http://ethon.consensys.net/WorldState">
        <rdfs:subClassOf rdf:resource="http://ethon.consensys.net/ModifiedMerklePatriciaTree"/>
        <rdfs:subClassOf rdf:resource="http://ethon.consensys.net/State"/>
        <suggestedStringRepresentation xml:lang="en">State</suggestedStringRepresentation>
        <rdfs:comment xml:lang="en">The world state, is a mapping between addresses (160-bit identifiers) of all accounts and their states (a data structure serialised as Recursive Length Prefix). The mapping is not stored on the blockchain itself but in a modified Merkle Patricia tree. An individual state is identified by the root hash of the trie.</rdfs:comment>
        <rdfs:label xml:lang="en">World State</rdfs:label>
        <ns:term_status>unstable</ns:term_status>
    </owl:Class>



    <!-- http://xmlns.com/foaf/0.1/Agent -->

    <owl:Class rdf:about="http://xmlns.com/foaf/0.1/Agent">
        <rdfs:isDefinedBy rdf:resource="http://xmlns.com/foaf/0.1/"/>
    </owl:Class>



    <!--
    ///////////////////////////////////////////////////////////////////////////////////////
    //
    // General axioms
    //
    ///////////////////////////////////////////////////////////////////////////////////////
     -->

    <owl:Axiom>
        <owl:annotatedSource>
            <owl:Class>
                <owl:intersectionOf rdf:parseType="Collection">
                    <rdf:Description rdf:about="http://ethon.consensys.net/Account"/>
                    <owl:Restriction>
                        <owl:onProperty rdf:resource="http://ethon.consensys.net/hasState"/>
                        <owl:someValuesFrom>
                            <owl:Class>
                                <owl:intersectionOf rdf:parseType="Collection">
                                    <rdf:Description rdf:about="http://ethon.consensys.net/AccountState"/>
                                    <owl:Restriction>
                                        <owl:onProperty rdf:resource="http://ethon.consensys.net/accountCodeHash"/>
                                        <owl:someValuesFrom>
                                            <rdfs:Datatype>
                                                <owl:oneOf>
                                                    <rdf:Description>
                                                        <rdf:type rdf:resource="http://www.w3.org/1999/02/22-rdf-syntax-ns#List"/>
                                                        <rdf:first rdf:datatype="http://www.w3.org/2001/XMLSchema#string">c5d2460186f7233c927e7db2dcc703c0e500b653ca82273b7bfad8045d85a470</rdf:first>
                                                        <rdf:rest rdf:resource="http://www.w3.org/1999/02/22-rdf-syntax-ns#nil"/>
                                                    </rdf:Description>
                                                </owl:oneOf>
                                            </rdfs:Datatype>
                                        </owl:someValuesFrom>
                                    </owl:Restriction>
                                </owl:intersectionOf>
                            </owl:Class>
                        </owl:someValuesFrom>
                    </owl:Restriction>
                </owl:intersectionOf>
                <rdfs:subClassOf rdf:resource="http://ethon.consensys.net/ExternalAccount"/>
            </owl:Class>
        </owl:annotatedSource>
        <owl:annotatedProperty rdf:resource="http://www.w3.org/2000/01/rdf-schema#subClassOf"/>
        <owl:annotatedTarget rdf:resource="http://ethon.consensys.net/ExternalAccount"/>
        <DASE_RULE rdf:datatype="http://www.w3.org/2001/XMLSchema#string">YP-p4.1___Account(?x)^AccountState(?y)^hasState(?x,?y)^accountCodeHash(?y,&quot;c5d2460186f7233c927e7db2dcc703c0e500b653ca82273b7bfad8045d85a470&quot;)-&gt;ExternalAccount(?x)___If the codeHash field of an Account is the Keccac-256 hash of the empty string, then the node represents an External Account.</DASE_RULE>
    </owl:Axiom>
    <owl:Axiom>
        <owl:annotatedSource>
            <owl:Class>
                <owl:intersectionOf rdf:parseType="Collection">
                    <rdf:Description rdf:about="http://ethon.consensys.net/Block"/>
                    <owl:Restriction>
                        <owl:onProperty rdf:resource="http://ethon.consensys.net/createsPostBlockState"/>
                        <owl:someValuesFrom rdf:resource="http://ethon.consensys.net/PostBlockState"/>
                    </owl:Restriction>
                </owl:intersectionOf>
                <rdfs:subClassOf rdf:resource="http://ethon.consensys.net/StateTransition"/>
            </owl:Class>
        </owl:annotatedSource>
        <owl:annotatedProperty rdf:resource="http://www.w3.org/2000/01/rdf-schema#subClassOf"/>
        <owl:annotatedTarget rdf:resource="http://ethon.consensys.net/StateTransition"/>
        <DASE_RULE rdf:datatype="http://www.w3.org/2001/XMLSchema#string">YP-1.1___Block(?b)^hasPostBlockState(?b,?s)^PostBlockState(?s)-&gt;StateTransition(?b)___A valid Message State Transition is one which comes about through a Message.</DASE_RULE>
    </owl:Axiom>
    <owl:Axiom>
        <owl:annotatedSource>
            <owl:Restriction>
                <owl:onProperty rdf:resource="http://ethon.consensys.net/hasTxTrie"/>
                <owl:someValuesFrom rdf:resource="http://www.w3.org/2002/07/owl#Thing"/>
                <rdfs:subClassOf rdf:resource="http://ethon.consensys.net/Block"/>
            </owl:Restriction>
        </owl:annotatedSource>
        <owl:annotatedProperty rdf:resource="http://www.w3.org/2000/01/rdf-schema#subClassOf"/>
        <owl:annotatedTarget rdf:resource="http://ethon.consensys.net/Block"/>
        <DASE_RULE rdf:datatype="http://www.w3.org/2001/XMLSchema#string">YP-3.1___hasTxTrie(?x,?y)-&gt;Block(?x)___Anything that has a TxTrie is a Block.</DASE_RULE>
    </owl:Axiom>
    <rdf:Description>
        <rdf:type rdf:resource="http://www.w3.org/2002/07/owl#AllDisjointClasses"/>
        <owl:members rdf:parseType="Collection">
            <rdf:Description rdf:about="http://ethon.consensys.net/Block"/>
            <rdf:Description rdf:about="http://ethon.consensys.net/ReceiptsTrie"/>
            <rdf:Description rdf:about="http://ethon.consensys.net/TxTrie"/>
            <rdf:Description rdf:about="http://ethon.consensys.net/Uncle"/>
        </owl:members>
    </rdf:Description>
    <rdf:Description>
        <rdf:type rdf:resource="http://www.w3.org/2002/07/owl#AllDisjointClasses"/>
        <owl:members rdf:parseType="Collection">
            <rdf:Description rdf:about="http://ethon.consensys.net/Blockchain"/>
            <rdf:Description rdf:about="http://ethon.consensys.net/Network"/>
            <rdf:Description rdf:about="http://ethon.consensys.net/Node"/>
            <rdf:Description rdf:about="http://ethon.consensys.net/ProtocolVariant"/>
        </owl:members>
    </rdf:Description>
    <rdf:Description>
        <rdf:type rdf:resource="http://www.w3.org/2002/07/owl#AllDisjointClasses"/>
        <owl:members rdf:parseType="Collection">
            <rdf:Description rdf:about="http://ethon.consensys.net/CallContractMsg"/>
            <rdf:Description rdf:about="http://ethon.consensys.net/CreateContractMsg"/>
            <rdf:Description rdf:about="http://ethon.consensys.net/ValueContractMsg"/>
        </owl:members>
    </rdf:Description>
    <rdf:Description>
        <rdf:type rdf:resource="http://www.w3.org/2002/07/owl#AllDisjointClasses"/>
        <owl:members rdf:parseType="Collection">
            <rdf:Description rdf:about="http://ethon.consensys.net/CallTx"/>
            <rdf:Description rdf:about="http://ethon.consensys.net/CreateTx"/>
            <rdf:Description rdf:about="http://ethon.consensys.net/ValueTx"/>
        </owl:members>
    </rdf:Description>



    <!--
    ///////////////////////////////////////////////////////////////////////////////////////
    //
    // Rules
    //
    ///////////////////////////////////////////////////////////////////////////////////////
     -->

    <rdf:Description rdf:about="http://ethon.consensys.net/x">
        <rdf:type rdf:resource="http://www.w3.org/2003/11/swrl#Variable"/>
    </rdf:Description>
    <rdf:Description rdf:about="http://ethon.consensys.net/y">
        <rdf:type rdf:resource="http://www.w3.org/2003/11/swrl#Variable"/>
    </rdf:Description>
    <rdf:Description>
        <swrla:isRuleEnabled rdf:datatype="http://www.w3.org/2001/XMLSchema#boolean">true</swrla:isRuleEnabled>
        <rdfs:comment rdf:datatype="http://www.w3.org/2001/XMLSchema#string">The Block level state transition function is the collection of all Transaction level state transition functions.</rdfs:comment>
        <rdfs:label rdf:datatype="http://www.w3.org/2001/XMLSchema#string">YP-4.1</rdfs:label>
        <rdf:type rdf:resource="http://www.w3.org/2003/11/swrl#Imp"/>
        <swrl:body>
            <rdf:Description>
                <rdf:type rdf:resource="http://www.w3.org/2003/11/swrl#AtomList"/>
                <rdf:first>
                    <rdf:Description>
                        <rdf:type rdf:resource="http://www.w3.org/2003/11/swrl#IndividualPropertyAtom"/>
                        <swrl:propertyPredicate rdf:resource="http://ethon.consensys.net/containsTx"/>
                        <swrl:argument1 rdf:resource="http://ethon.consensys.net/x"/>
                        <swrl:argument2 rdf:resource="http://ethon.consensys.net/y"/>
                    </rdf:Description>
                </rdf:first>
                <rdf:rest>
                    <rdf:Description>
                        <rdf:type rdf:resource="http://www.w3.org/2003/11/swrl#AtomList"/>
                        <rdf:first>
                            <rdf:Description>
                                <rdf:type rdf:resource="http://www.w3.org/2003/11/swrl#ClassAtom"/>
                                <swrl:classPredicate rdf:resource="http://ethon.consensys.net/Tx"/>
                                <swrl:argument1 rdf:resource="http://ethon.consensys.net/y"/>
                            </rdf:Description>
                        </rdf:first>
                        <rdf:rest>
                            <rdf:Description>
                                <rdf:type rdf:resource="http://www.w3.org/2003/11/swrl#AtomList"/>
                                <rdf:first>
                                    <rdf:Description>
                                        <rdf:type rdf:resource="http://www.w3.org/2003/11/swrl#ClassAtom"/>
                                        <swrl:classPredicate rdf:resource="http://ethon.consensys.net/Block"/>
                                        <swrl:argument1 rdf:resource="http://ethon.consensys.net/x"/>
                                    </rdf:Description>
                                </rdf:first>
                                <rdf:rest rdf:resource="http://www.w3.org/1999/02/22-rdf-syntax-ns#nil"/>
                            </rdf:Description>
                        </rdf:rest>
                    </rdf:Description>
                </rdf:rest>
            </rdf:Description>
        </swrl:body>
        <swrl:head>
            <rdf:Description>
                <rdf:type rdf:resource="http://www.w3.org/2003/11/swrl#AtomList"/>
                <rdf:first>
                    <rdf:Description>
                        <rdf:type rdf:resource="http://www.w3.org/2003/11/swrl#IndividualPropertyAtom"/>
                        <swrl:propertyPredicate rdf:resource="http://ethon.consensys.net/partOf"/>
                        <swrl:argument1 rdf:resource="http://ethon.consensys.net/y"/>
                        <swrl:argument2 rdf:resource="http://ethon.consensys.net/x"/>
                    </rdf:Description>
                </rdf:first>
                <rdf:rest rdf:resource="http://www.w3.org/1999/02/22-rdf-syntax-ns#nil"/>
            </rdf:Description>
        </swrl:head>
    </rdf:Description>
</rdf:RDF>



<!-- Generated by the OWL API (version 4.2.8.20170104-2310) https://github.com/owlcs/owlapi -->
