<?xml version="1.0"?>
<rdf:RDF xmlns="http://www.grid.ac/ontology/"
     xml:base="http://www.grid.ac/ontology/"
     xmlns:rdf="http://www.w3.org/1999/02/22-rdf-syntax-ns#"
     xmlns:owl="http://www.w3.org/2002/07/owl#"
     xmlns:xml="http://www.w3.org/XML/1998/namespace"
     xmlns:gn="http://www.geonames.org/ontology#"
     xmlns:xsd="http://www.w3.org/2001/XMLSchema#"
     xmlns:rdfs="http://www.w3.org/2000/01/rdf-schema#"
     xmlns:dc="http://purl.org/dc/elements/1.1/">
    <owl:Ontology rdf:about="http://www.grid.ac/ontology/">
        <dc:rights xml:lang="en">This work is distributed under a Creative Commons Attribution 4.0 (CC BY 4.0) License &lt;http://creativecommons.org/licenses/by/4.0/&gt;.</dc:rights>
        <rdfs:comment xml:lang="en">Created and maintained by the GRID Team, Digital Science and Research Ltd</rdfs:comment>
        <owl:versionInfo>1.0.2</owl:versionInfo>
        <dc:date>2016-07-14T12:00:00Z</dc:date>
        <rdfs:label xml:lang="en">GRID Ontology version 1.0</rdfs:label>
        <dc:publisher xml:lang="en">Digital Science</dc:publisher>
    </owl:Ontology>
    


    <!-- 
    ///////////////////////////////////////////////////////////////////////////////////////
    //
    // Annotation properties
    //
    ///////////////////////////////////////////////////////////////////////////////////////
     -->

    


    <!-- http://purl.org/dc/elements/1.1/date -->

    <owl:AnnotationProperty rdf:about="http://purl.org/dc/elements/1.1/date"/>
    


    <!-- http://purl.org/dc/elements/1.1/publisher -->

    <owl:AnnotationProperty rdf:about="http://purl.org/dc/elements/1.1/publisher"/>
    


    <!-- http://purl.org/dc/elements/1.1/rights -->

    <owl:AnnotationProperty rdf:about="http://purl.org/dc/elements/1.1/rights"/>
    


    <!-- 
    ///////////////////////////////////////////////////////////////////////////////////////
    //
    // Object Properties
    //
    ///////////////////////////////////////////////////////////////////////////////////////
     -->

    


    <!-- http://www.grid.ac/ontology/hasAddress -->

    <owl:ObjectProperty rdf:about="http://www.grid.ac/ontology/hasAddress">
        <rdfs:domain rdf:resource="http://www.grid.ac/ontology/Organisation"/>
        <rdfs:range rdf:resource="http://www.grid.ac/ontology/Address"/>
        <rdfs:comment xml:lang="en">Links organisations to their locations (as addresses)</rdfs:comment>
        <rdfs:label xml:lang="en">hasAddress</rdfs:label>
    </owl:ObjectProperty>
    


    <!-- http://www.grid.ac/ontology/hasChild -->

    <owl:ObjectProperty rdf:about="http://www.grid.ac/ontology/hasChild">
        <owl:inverseOf rdf:resource="http://www.grid.ac/ontology/hasParent"/>
        <rdfs:domain rdf:resource="http://www.grid.ac/ontology/Organisation"/>
        <rdfs:range rdf:resource="http://www.grid.ac/ontology/Organisation"/>
        <rdfs:comment xml:lang="en">Links organisation that are in a parent / child hierarchy</rdfs:comment>
        <rdfs:label xml:lang="en">hasChild</rdfs:label>
    </owl:ObjectProperty>
    


    <!-- http://www.grid.ac/ontology/hasGeonamesCity -->

    <owl:ObjectProperty rdf:about="http://www.grid.ac/ontology/hasGeonamesCity">
        <rdfs:domain rdf:resource="http://www.grid.ac/ontology/Address"/>
        <rdfs:range rdf:resource="http://www.geonames.org/ontology#Feature"/>
        <rdfs:comment xml:lang="en">Links the organisation&apos;s location to a Geonames identifier. In Geonames you can find region hierarchies, population statistics, geographic positions (lat / long) and more. See http://www.geonames.org/</rdfs:comment>
        <rdfs:label xml:lang="en">hasGeonamesCity</rdfs:label>
    </owl:ObjectProperty>
    


    <!-- http://www.grid.ac/ontology/hasParent -->

    <owl:ObjectProperty rdf:about="http://www.grid.ac/ontology/hasParent">
        <rdfs:domain rdf:resource="http://www.grid.ac/ontology/Organisation"/>
        <rdfs:range rdf:resource="http://www.grid.ac/ontology/Organisation"/>
        <rdfs:comment xml:lang="en">Links organisation that are in a parent / child hierarchy</rdfs:comment>
        <rdfs:label xml:lang="en">hasParent</rdfs:label>
    </owl:ObjectProperty>
    


    <!-- http://www.grid.ac/ontology/hasRelated -->

    <owl:ObjectProperty rdf:about="http://www.grid.ac/ontology/hasRelated">
        <rdfs:domain rdf:resource="http://www.grid.ac/ontology/Organisation"/>
        <rdfs:range rdf:resource="http://www.grid.ac/ontology/Organisation"/>
        <rdfs:comment xml:lang="en">Link organisations that are related (e.g. affiliated, co-located, collaborators)</rdfs:comment>
        <rdfs:label xml:lang="en">hasRelated</rdfs:label>
    </owl:ObjectProperty>
    


    <!-- 
    ///////////////////////////////////////////////////////////////////////////////////////
    //
    // Data properties
    //
    ///////////////////////////////////////////////////////////////////////////////////////
     -->

    


    <!-- http://www.grid.ac/ontology/cityName -->

    <owl:DatatypeProperty rdf:about="http://www.grid.ac/ontology/cityName">
        <rdfs:domain rdf:resource="http://www.grid.ac/ontology/Address"/>
        <rdfs:range rdf:resource="http://www.w3.org/2001/XMLSchema#string"/>
        <rdfs:comment xml:lang="en">The name of the city (in English if available)</rdfs:comment>
        <rdfs:label xml:lang="en">cityName</rdfs:label>
    </owl:DatatypeProperty>
    


    <!-- http://www.grid.ac/ontology/countryCode -->

    <owl:DatatypeProperty rdf:about="http://www.grid.ac/ontology/countryCode">
        <rdfs:domain rdf:resource="http://www.grid.ac/ontology/Address"/>
        <rdfs:range rdf:resource="http://www.w3.org/2001/XMLSchema#string"/>
        <rdfs:comment xml:lang="en">ISO 3166-1 alpha-2</rdfs:comment>
        <rdfs:label xml:lang="en">countryCode</rdfs:label>
    </owl:DatatypeProperty>
    


    <!-- http://www.grid.ac/ontology/countryName -->

    <owl:DatatypeProperty rdf:about="http://www.grid.ac/ontology/countryName">
        <rdfs:domain rdf:resource="http://www.grid.ac/ontology/Address"/>
        <rdfs:range rdf:resource="http://www.w3.org/2001/XMLSchema#string"/>
        <rdfs:comment xml:lang="en">The name of the country or territory in English</rdfs:comment>
        <rdfs:label xml:lang="en">countryName</rdfs:label>
    </owl:DatatypeProperty>
    


    <!-- http://www.grid.ac/ontology/establishedYear -->

    <owl:DatatypeProperty rdf:about="http://www.grid.ac/ontology/establishedYear">
        <rdfs:domain rdf:resource="http://www.grid.ac/ontology/Organisation"/>
        <rdfs:range rdf:resource="http://www.w3.org/2001/XMLSchema#integer"/>
        <rdfs:comment xml:lang="en">The year the organisation was established</rdfs:comment>
        <rdfs:label xml:lang="en">establishedYear</rdfs:label>
    </owl:DatatypeProperty>
    


    <!-- http://www.grid.ac/ontology/hasCrossrefFunderID -->

    <owl:DatatypeProperty rdf:about="http://www.grid.ac/ontology/hasCrossrefFunderID">
        <rdfs:domain rdf:resource="http://www.grid.ac/ontology/Organisation"/>
        <rdfs:range rdf:resource="http://www.w3.org/2001/XMLSchema#string"/>
        <rdfs:comment xml:lang="en">The Crossref Open Funder Registry Id for
 the organisation. See http://www.crossref.org/fundingdata/registry.html</rdfs:comment>
        <rdfs:label xml:lang="en">crossrefFunderId</rdfs:label>
    </owl:DatatypeProperty>
    


    <!-- http://www.grid.ac/ontology/hasISNI -->

    <owl:DatatypeProperty rdf:about="http://www.grid.ac/ontology/hasISNI">
        <rdfs:domain rdf:resource="http://www.grid.ac/ontology/Organisation"/>
        <rdfs:range rdf:resource="http://www.w3.org/2001/XMLSchema#string"/>
        <rdfs:comment xml:lang="en">The International Standard Name Identifier (ISNI) Id for the organisation. See http://isni.oclc.nl/</rdfs:comment>
        <rdfs:label xml:lang="en">isni</rdfs:label>
    </owl:DatatypeProperty>
    


    <!-- http://www.grid.ac/ontology/hasUKPRN -->

    <owl:DatatypeProperty rdf:about="http://www.grid.ac/ontology/hasUKPRN">
        <rdfs:domain rdf:resource="http://www.grid.ac/ontology/Organisation"/>
        <rdfs:range rdf:resource="http://www.w3.org/2001/XMLSchema#string"/>
        <rdfs:comment xml:lang="en">The UK Provider Reference Number (UKPRN) Id for the organisation. See https://www.ukrlp.co.uk/</rdfs:comment>
        <rdfs:label xml:lang="en">ukprn</rdfs:label>
    </owl:DatatypeProperty>
    


    <!-- http://www.grid.ac/ontology/hasWikidataID -->

    <owl:DatatypeProperty rdf:about="http://www.grid.ac/ontology/hasWikidataID">
        <rdfs:domain rdf:resource="http://www.grid.ac/ontology/Organisation"/>
        <rdfs:range rdf:resource="http://www.w3.org/2001/XMLSchema#string"/>
        <rdfs:comment xml:lang="en">The Wikidata id for the organisation. See https://www.wikidata.org</rdfs:comment>
        <rdfs:label xml:lang="en">wikidataId</rdfs:label>
    </owl:DatatypeProperty>
    


    <!-- http://www.grid.ac/ontology/id -->

    <owl:DatatypeProperty rdf:about="http://www.grid.ac/ontology/id">
        <rdfs:domain rdf:resource="http://www.grid.ac/ontology/Organisation"/>
        <rdfs:range rdf:resource="http://www.w3.org/2001/XMLSchema#string"/>
        <rdfs:comment xml:lang="en">A unique, persistent id for the organisation</rdfs:comment>
        <rdfs:label xml:lang="en">id</rdfs:label>
    </owl:DatatypeProperty>
    


    <!-- http://www.grid.ac/ontology/wikipediaPage -->

    <owl:DatatypeProperty rdf:about="http://www.grid.ac/ontology/wikipediaPage">
        <rdfs:domain rdf:resource="http://www.grid.ac/ontology/Organisation"/>
        <rdfs:comment xml:lang="en">The Wikipedia page corresponding to this organisation</rdfs:comment>
        <rdfs:label xml:lang="en">wikipediaPage</rdfs:label>
    </owl:DatatypeProperty>
    


    <!-- 
    ///////////////////////////////////////////////////////////////////////////////////////
    //
    // Classes
    //
    ///////////////////////////////////////////////////////////////////////////////////////
     -->

    


    <!-- http://www.geonames.org/ontology#Feature -->

    <owl:Class rdf:about="http://www.geonames.org/ontology#Feature"/>
    


    <!-- http://www.grid.ac/ontology/Address -->

    <owl:Class rdf:about="http://www.grid.ac/ontology/Address">
        <rdfs:comment xml:lang="en">Information about the location of the organisation.</rdfs:comment>
        <rdfs:label xml:lang="en">Address</rdfs:label>
    </owl:Class>
    


    <!-- http://www.grid.ac/ontology/Archive -->

    <owl:Class rdf:about="http://www.grid.ac/ontology/Archive">
        <rdfs:subClassOf rdf:resource="http://www.grid.ac/ontology/Organisation"/>
        <rdfs:comment xml:lang="en">Repository of documents, artifacts, or specimens. Includes libraries and museums that are not part of a university.</rdfs:comment>
        <rdfs:label xml:lang="en">Archive</rdfs:label>
    </owl:Class>
    


    <!-- http://www.grid.ac/ontology/Company -->

    <owl:Class rdf:about="http://www.grid.ac/ontology/Company">
        <rdfs:subClassOf rdf:resource="http://www.grid.ac/ontology/Organisation"/>
        <rdfs:comment xml:lang="en">Business entity with the aim of gaining profit.</rdfs:comment>
        <rdfs:label xml:lang="en">Company</rdfs:label>
    </owl:Class>
    


    <!-- http://www.grid.ac/ontology/Education -->

    <owl:Class rdf:about="http://www.grid.ac/ontology/Education">
        <rdfs:subClassOf rdf:resource="http://www.grid.ac/ontology/Organisation"/>
        <rdfs:comment xml:lang="en">An educational institution where research takes place. Can grant degrees and includes faculties, departments and schools.</rdfs:comment>
        <rdfs:label xml:lang="en">Education</rdfs:label>
    </owl:Class>
    


    <!-- http://www.grid.ac/ontology/Facility -->

    <owl:Class rdf:about="http://www.grid.ac/ontology/Facility">
        <rdfs:subClassOf rdf:resource="http://www.grid.ac/ontology/Organisation"/>
        <rdfs:comment xml:lang="en">A building or facility dedicated to research of a specific area, usually contains specialised equipment. Includes telescopes, observatories and particle accelerators.</rdfs:comment>
        <rdfs:label xml:lang="en">Facility</rdfs:label>
    </owl:Class>
    


    <!-- http://www.grid.ac/ontology/Government -->

    <owl:Class rdf:about="http://www.grid.ac/ontology/Government">
        <rdfs:subClassOf rdf:resource="http://www.grid.ac/ontology/Organisation"/>
        <rdfs:comment xml:lang="en">An organisation operated mainly by the government of one or multiple countries.</rdfs:comment>
        <rdfs:label xml:lang="en">Government</rdfs:label>
    </owl:Class>
    


    <!-- http://www.grid.ac/ontology/Healthcare -->

    <owl:Class rdf:about="http://www.grid.ac/ontology/Healthcare">
        <rdfs:subClassOf rdf:resource="http://www.grid.ac/ontology/Organisation"/>
        <rdfs:comment xml:lang="en">A health related facility where patients are treated. Includes hospitals, medical centres, health centres, treatment center. Includes trusts and healthcare systems.</rdfs:comment>
        <rdfs:label xml:lang="en">Healthcare</rdfs:label>
    </owl:Class>
    


    <!-- http://www.grid.ac/ontology/Nonprofit -->

    <owl:Class rdf:about="http://www.grid.ac/ontology/Nonprofit">
        <rdfs:subClassOf rdf:resource="http://www.grid.ac/ontology/Organisation"/>
        <rdfs:comment xml:lang="en">Organisation that uses its surplus revenue to achieve its goals. Includes charities and other non-government research funding bodies.</rdfs:comment>
        <rdfs:label xml:lang="en">Nonprofit</rdfs:label>
    </owl:Class>
    


    <!-- http://www.grid.ac/ontology/Organisation -->

    <owl:Class rdf:about="http://www.grid.ac/ontology/Organisation">
        <rdfs:comment xml:lang="en">The top-level concept in the GRID hierarchy of organisation types.</rdfs:comment>
        <rdfs:label xml:lang="en">Organisation</rdfs:label>
    </owl:Class>
    


    <!-- http://www.grid.ac/ontology/Other -->

    <owl:Class rdf:about="http://www.grid.ac/ontology/Other">
        <rdfs:subClassOf rdf:resource="http://www.grid.ac/ontology/Organisation"/>
        <rdfs:comment xml:lang="en">Used in cases where none of the other defined types are suitable.</rdfs:comment>
        <rdfs:label xml:lang="en">Other</rdfs:label>
    </owl:Class>
</rdf:RDF>



<!-- Generated by the OWL API (version 4.2.5.20160517-0735) https://github.com/owlcs/owlapi -->

