@prefix dc: <http://purl.org/dc/elements/1.1/> .
@prefix ns1: <http://scigraph.springernature.com/ontologies/core/> .
@prefix ns2: <http://purl.org/dc/terms/> .
@prefix owl: <http://www.w3.org/2002/07/owl#> .
@prefix rdf: <http://www.w3.org/1999/02/22-rdf-syntax-ns#> .
@prefix rdfs: <http://www.w3.org/2000/01/rdf-schema#> .
@prefix sh: <http://www.w3.org/ns/shacl#> .
@prefix skos: <http://www.w3.org/2004/02/skos/core#> .
@prefix vann: <http://purl.org/vocab/vann/> .
@prefix void: <http://rdfs.org/ns/void#> .
@prefix xml: <http://www.w3.org/XML/1998/namespace> .
@prefix xsd: <http://www.w3.org/2001/XMLSchema#> .

ns1:AccessType a owl:Class ;
    rdfs:label "Class: Access type"@en ;
    ns1:namespace "access-types" ;
    rdfs:comment "The :AccessType class provides an instance from a categorisation of the various kinds of permissions/restrictions characterizing the way end users can access a product. In the case of online articles, for example, these can be 'Open Access' or 'Subscription'. Even though in most situations the products in question will be instances of :Publication (e.g. periodicals, issues, or specific components of these), in some cases other entities like datasets or websites may be qualified via an access type. The :AccessType categorisation is implemented as a SKOS concept scheme."@en ;
    rdfs:isDefinedBy ns1: ;
    rdfs:subClassOf ns1:Concept .

ns1:AggregationEvent a owl:Class ;
    rdfs:label "Class: Aggregation event"@en ;
    ns1:namespace "aggregation-events" ;
    rdfs:comment "The :AggregationEvent class groups together all events related to the construction of a publication."@en ;
    rdfs:isDefinedBy ns1: ;
    rdfs:subClassOf ns1:Event .

ns1:Annotation a owl:Class ;
    rdfs:label "Class: Annotation"@en ;
    ns1:namespace "annotations" ;
    rdfs:comment "The :Annotation class groups together all individuals that represents any entity used to annotate a document or artefact."@en ;
    rdfs:isDefinedBy ns1: ;
    rdfs:subClassOf ns1:Intangible .

ns1:CategorizationEvent a owl:Class ;
    rdfs:label "Class: Categorization event"@en ;
    ns1:namespace "categorization-events" ;
    rdfs:comment "The :CategorizationEvent class represents an event which annotates a thing with a category."@en ;
    rdfs:isDefinedBy ns1: ;
    rdfs:subClassOf ns1:AnnotationEvent .

ns1:ImpactFactorMetricsEvent a owl:Class ;
    rdfs:label "Class: Impact factor metrics event"@en ;
    ns1:namespace "impact-factor-metrics-events" ;
    rdfs:comment "The :ImpactFactorMetricsEvent class represents an event which annotates a thing with impact factor metrics information."@en ;
    rdfs:isDefinedBy ns1: ;
    rdfs:subClassOf ns1:MetricsEvent .

ns1:IndexCheckEvent a owl:Class ;
    rdfs:label "Class: Index check event"@en ;
    ns1:namespace "index-check-events" ;
    rdfs:comment "The :IndexCheckEvent class represents an event which annotates a thing with an index check."@en ;
    rdfs:isDefinedBy ns1: ;
    rdfs:subClassOf ns1:AnnotationEvent .

ns1:Tangible a owl:Class ;
    rdfs:label "Class: Tangible"@en ;
    ns1:namespace "tangibles" ;
    rdfs:comment "The :Tangible class groups together all entities with a spatial extension and that can participate in temporal events. Instances of :Tangible are normally the physical substrate of :Intangible entities, e.g. the physical realization of a book is the substrate for its symbolic contents."@en ;
    rdfs:isDefinedBy ns1: ;
    rdfs:subClassOf ns1:Thing .

ns1:abstract a owl:DatatypeProperty ;
    rdfs:label "Property: abstract"@en ;
    rdfs:comment "The :abstract property specifies the abstract for a publication as a plain string."@en ;
    rdfs:isDefinedBy ns1: ;
    rdfs:range xsd:string .

ns1:abstractRights a owl:DatatypeProperty ;
    rdfs:label "Property: abstract rights"@en ;
    rdfs:comment "The :abstractRights property specifies an access right to the abstract section of a publication as a string value."@en ;
    rdfs:domain ns1:Publication ;
    rdfs:isDefinedBy ns1: ;
    rdfs:range xsd:string ;
    rdfs:subPropertyOf ns1:accessRights .

ns1:abstractTranslated a owl:DatatypeProperty ;
    rdfs:label "Property: abstract translated"@en ;
    rdfs:comment "The :abstractTranslated property specifies the abstract for a publication as a language-tagged string."@en ;
    rdfs:isDefinedBy ns1: ;
    rdfs:range rdf:langString .

ns1:acronym a owl:DatatypeProperty ;
    rdfs:label "Property: acronym"@en ;
    rdfs:comment "The :acronym property specifies an abbreviation formed from the initial letters of other words."@en ;
    rdfs:domain ns1:Thing ;
    rdfs:isDefinedBy ns1: ;
    rdfs:range xsd:string ;
    rdfs:subPropertyOf ns1:nameInfo .

ns1:annotationAgent a owl:DatatypeProperty ;
    rdfs:label "Property: annotation agent"@en ;
    rdfs:comment "The :annotation agent property specifies a string value which records the annotator agent in an annotation event."@en ;
    rdfs:domain ns1:AnnotationEvent ;
    rdfs:isDefinedBy ns1: ;
    rdfs:range xsd:string .

ns1:annotationCategory a owl:DatatypeProperty ;
    rdfs:label "Property: annotation category"@en ;
    rdfs:comment "The :annotationCategory property specifies a category which is used to annotate a thing in an annotation event as a string value."@en ;
    rdfs:domain ns1:AnnotationEvent ;
    rdfs:isDefinedBy ns1: ;
    rdfs:range xsd:string .

ns1:articleId a owl:DatatypeProperty ;
    rdfs:label "Property: articleId"@en ;
    rdfs:comment "The :articleId property specifies an internal ID for an article."@en ;
    rdfs:domain ns1:Article ;
    rdfs:isDefinedBy ns1: ;
    rdfs:range xsd:string ;
    rdfs:subPropertyOf ns1:id .

ns1:articleType a owl:DatatypeProperty ;
    rdfs:label "Property: article type"@en ;
    rdfs:comment "The :articleType property specifies a string value for an article-type."@en ;
    rdfs:isDefinedBy ns1: ;
    rdfs:range xsd:string .

ns1:bibliographyRights a owl:DatatypeProperty ;
    rdfs:label "Property: bibliography rights"@en ;
    rdfs:comment "The :bibliographyRights property specifies an access right to the bibliography section of a publication as a string value."@en ;
    rdfs:domain ns1:Publication ;
    rdfs:isDefinedBy ns1: ;
    rdfs:range xsd:string ;
    rdfs:subPropertyOf ns1:accessRights .

ns1:body a owl:DatatypeProperty ;
    rdfs:label "Property: body"@en ;
    rdfs:comment "The :body property specifies the main body content of a publication as a language string."@en ;
    rdfs:domain ns1:Publication ;
    rdfs:isDefinedBy ns1: ;
    rdfs:range rdf:langString .

ns1:bodyHtmlRights a owl:DatatypeProperty ;
    rdfs:label "Property: body HTML rights"@en ;
    rdfs:comment "The :bodyHtmlRights property specifies an access right to the HTML body of a publication as a string value."@en ;
    rdfs:domain ns1:Publication ;
    rdfs:isDefinedBy ns1: ;
    rdfs:range xsd:string ;
    rdfs:subPropertyOf ns1:accessRights .

ns1:bodyPdfRights a owl:DatatypeProperty ;
    rdfs:label "Property: body PDF rights"@en ;
    rdfs:comment "The :bodyPdfRights property specifies an access right to the PDF body of a publication as a string value."@en ;
    rdfs:domain ns1:Publication ;
    rdfs:isDefinedBy ns1: ;
    rdfs:range xsd:string ;
    rdfs:subPropertyOf ns1:accessRights .

ns1:bodyXml a owl:DatatypeProperty ;
    rdfs:label "Property: body (XML)"@en ;
    rdfs:comment "The :bodyXml property specifies the main body content of a publication in XML format as a language string."@en ;
    rdfs:domain ns1:Publication ;
    rdfs:isDefinedBy ns1: ;
    rdfs:range rdf:langString .

ns1:bookType a owl:DatatypeProperty ;
    rdfs:label "Property: book type"@en ;
    rdfs:comment "The :bookType property specifies a string value for a book type."@en ;
    rdfs:isDefinedBy ns1: ;
    rdfs:range xsd:string .

ns1:category a owl:DatatypeProperty ;
    rdfs:label "Property: category"@en ;
    rdfs:comment "The :category property specifies the category, subject or topic of an entity as a string value."@en ;
    rdfs:domain ns1:Thing ;
    rdfs:isDefinedBy ns1: ;
    rdfs:range xsd:string .

ns1:chapterCount a owl:DatatypeProperty ;
    rdfs:label "Property: chapter count"@en ;
    rdfs:comment "The :chapterCount property specifies a total count for the number of chapters within a publication (e.g. a book)."@en ;
    rdfs:domain ns1:Publication ;
    rdfs:isDefinedBy ns1: ;
    rdfs:range xsd:integer ;
    rdfs:subPropertyOf ns1:count .

ns1:chapterNumber a owl:DatatypeProperty ;
    rdfs:label "Property: chapter number"@en ;
    rdfs:comment "The :chapterNumber property specifies the number of the chapter as a string value."@en ;
    rdfs:domain ns1:Publication ;
    rdfs:isDefinedBy ns1: ;
    rdfs:range xsd:string ;
    rdfs:subPropertyOf ns1:publicationNumber .

ns1:citationRank a owl:DatatypeProperty ;
    rdfs:label "Property: citationRank"@en ;
    rdfs:comment "The :citationRank property specifies the rank of a citation measurement as a string value."@en ;
    rdfs:domain ns1:MetricsEvent ;
    rdfs:isDefinedBy ns1: ;
    rdfs:range xsd:string .

ns1:city a owl:DatatypeProperty ;
    rdfs:label "Property: city"@en ;
    rdfs:comment "The :city property specifies the city location of a thing as a string value."@en ;
    rdfs:domain ns1:Thing ;
    rdfs:isDefinedBy ns1: ;
    rdfs:range xsd:string ;
    rdfs:subPropertyOf ns1:placeInfo .

ns1:code a owl:DatatypeProperty ;
    rdfs:label "Property: code"@en ;
    rdfs:comment "The :code property specifies an integer number representing an internal ID for an object. This property is used by the taxonomies for managing terms."@en ;
    rdfs:domain ns1:Concept ;
    rdfs:isDefinedBy ns1: ;
    rdfs:range xsd:integer .

ns1:content a owl:DatatypeProperty ;
    rdfs:label "Property: content"@en ;
    rdfs:comment "The :content property specifies a string type for the content of an article, e.g. 'full-text'."@en ;
    rdfs:domain ns1:Article ;
    rdfs:isDefinedBy ns1: ;
    rdfs:range xsd:string .

ns1:copyrightHolder a owl:DatatypeProperty ;
    rdfs:label "Property: copyright holder"@en ;
    rdfs:comment "The :copyrightHolder property specifies the copyright holder of a publication as a string value."@en ;
    rdfs:domain ns1:Publication ;
    rdfs:isDefinedBy ns1: ;
    rdfs:range xsd:string ;
    rdfs:subPropertyOf ns1:rights .

ns1:copyrightYear a owl:DatatypeProperty ;
    rdfs:label "Property: copyright year"@en ;
    rdfs:comment "The :copyrightYear property specifies the copyright year of a publication as a datetime year. This property typically appears together with the sg:copyrightHolder property."@en ;
    rdfs:domain ns1:Publication ;
    rdfs:isDefinedBy ns1: ;
    rdfs:range xsd:gYear ;
    rdfs:subPropertyOf ns1:rights .

ns1:country a owl:DatatypeProperty ;
    rdfs:label "Property: country"@en ;
    rdfs:comment "The :country property specifies the country location of a thing as a string value."@en ;
    rdfs:domain ns1:Thing ;
    rdfs:isDefinedBy ns1: ;
    rdfs:range xsd:string ;
    rdfs:subPropertyOf ns1:placeInfo .

ns1:coverDate a owl:DatatypeProperty ;
    rdfs:label "Property: cover date"@en ;
    rdfs:comment "The :coverDate property specifies the full date of a publication as it is displayed on its cover. This is not necessarily the actual date of publication."@en ;
    rdfs:domain ns1:Publication ;
    rdfs:isDefinedBy ns1: ;
    rdfs:range xsd:date ;
    rdfs:subPropertyOf ns1:dateInfo .

ns1:coverYear a owl:DatatypeProperty ;
    rdfs:label "Property: cover year"@en ;
    rdfs:comment "The :coverDate property specifies the year date of a publication as it is displayed on its cover. This is not necessarily the actual date of publication."@en ;
    rdfs:domain ns1:Publication ;
    rdfs:isDefinedBy ns1: ;
    rdfs:range xsd:gYear ;
    rdfs:subPropertyOf ns1:dateInfo .

ns1:coverYearMonth a owl:DatatypeProperty ;
    rdfs:label "Property: cover year-month"@en ;
    rdfs:comment "The :coverDate property specifies the year and month date of a publication as it is displayed on its cover. This is not necessarily the actual date of publication."@en ;
    rdfs:domain ns1:Publication ;
    rdfs:isDefinedBy ns1: ;
    rdfs:range xsd:gYearMonth ;
    rdfs:subPropertyOf ns1:dateInfo .

ns1:database a owl:DatatypeProperty ;
    rdfs:label "Property: database"@en ;
    rdfs:comment "The :database property specifies a database by a simple string value."@en ;
    rdfs:isDefinedBy ns1: ;
    rdfs:range xsd:string .

ns1:date a owl:DatatypeProperty ;
    rdfs:label "Property: date"@en ;
    rdfs:comment "The :date property specifies the full date for a thing, e.g. a publication or an event."@en ;
    rdfs:domain ns1:Thing ;
    rdfs:isDefinedBy ns1: ;
    rdfs:range xsd:date ;
    rdfs:subPropertyOf ns1:dateInfo .

ns1:dateEnd a owl:DatatypeProperty ;
    rdfs:label "Property: date end"@en ;
    rdfs:comment "The :dateEnd property specifies the end date for a thing, e.g. a publication or an event. Note that for a serial publication, this date relates to the publisher holdings which may not be the same as the actual publication end date."@en ;
    rdfs:domain ns1:Thing ;
    rdfs:isDefinedBy ns1: ;
    rdfs:range xsd:string ;
    rdfs:subPropertyOf ns1:dateInfo .

ns1:dateStart a owl:DatatypeProperty ;
    rdfs:label "Property: date start"@en ;
    rdfs:comment "The :dateStart property specifies the start date for a thing, e.g. a publication or an event. Note that for a serial publication, this date relates to the publisher holdings which may not be the same as the actual publication start date."@en ;
    rdfs:domain ns1:Thing ;
    rdfs:isDefinedBy ns1: ;
    rdfs:range xsd:string ;
    rdfs:subPropertyOf ns1:dateInfo .

ns1:datetime a owl:DatatypeProperty ;
    rdfs:label "Property: datetime"@en ;
    rdfs:comment "The :datetime property specifies a system-generated datetime for an entity."@en ;
    rdfs:domain ns1:Thing ;
    rdfs:isDefinedBy ns1: ;
    rdfs:range xsd:dateTime ;
    rdfs:subPropertyOf ns1:dateInfo .

ns1:dblpId a owl:DatatypeProperty ;
    rdfs:label "Property: DBLP ID"@en ;
    rdfs:comment "The :dblpId property specifies an ID within the DBLP publications database."@en ;
    rdfs:domain ns1:Thing ;
    rdfs:isDefinedBy ns1: ;
    rdfs:range xsd:string ;
    rdfs:subPropertyOf ns1:id .

ns1:ddsId a owl:DatatypeProperty ;
    rdfs:label "Property: DDS ID"@en ;
    rdfs:comment "The :ddsId property specifies an ID within the DDS dataset."@en ;
    rdfs:domain ns1:Thing ;
    rdfs:isDefinedBy ns1: ;
    rdfs:range xsd:string ;
    rdfs:subPropertyOf ns1:id .

ns1:ddsIdJournalBrand a owl:DatatypeProperty ;
    rdfs:label "Property: DDS ID (journal brand)"@en ;
    rdfs:comment "The :ddsIdJournalBrand property specifies an ID within the DDS dataset used for a journal brand."@en ;
    rdfs:domain ns1:Publication ;
    rdfs:isDefinedBy ns1: ;
    rdfs:range xsd:string .

ns1:description a owl:DatatypeProperty ;
    rdfs:label "Property: description"@en ;
    rdfs:comment "The :description property specifies a description for a Scigraph entity as a language string."@en ;
    rdfs:domain ns1:Thing ;
    rdfs:isDefinedBy ns1: ;
    rdfs:range rdf:langString .

ns1:dimensionsId a owl:DatatypeProperty ;
    rdfs:label "Property: Dimensions ID"@en ;
    rdfs:comment "The :dimensionsId property specifies an ID within the Dimensions dataset."@en ;
    rdfs:domain ns1:Thing ;
    rdfs:isDefinedBy ns1: ;
    rdfs:range xsd:string ;
    rdfs:subPropertyOf ns1:id .

ns1:doi a owl:DatatypeProperty ;
    rdfs:label "Property: DOI" ;
    rdfs:comment "The :doi property specifies a DOI number for a publication."@en ;
    rdfs:domain ns1:Publication ;
    rdfs:isDefinedBy ns1: ;
    rdfs:range xsd:string .

ns1:doiLink a owl:ObjectProperty ;
    rdfs:label "Property: DOI link"@en ;
    rdfs:comment "The :doiLink property relates a publication to the URI minted from the DOI."@en ;
    rdfs:domain ns1:Publication ;
    rdfs:isDefinedBy ns1: .

ns1:editionNumber a owl:DatatypeProperty ;
    rdfs:label "Property: edition number"@en ;
    rdfs:comment "The :editionNumber property specifies the number of the edition as a string value."@en ;
    rdfs:domain ns1:Publication ;
    rdfs:isDefinedBy ns1: ;
    rdfs:range xsd:string ;
    rdfs:subPropertyOf ns1:publicationNumber .

ns1:email a owl:DatatypeProperty ;
    rdfs:label "Property: email"@en ;
    rdfs:comment "The :email property specifies an email address."@en ;
    rdfs:isDefinedBy ns1: ;
    rdfs:range xsd:string .

ns1:endYear a owl:DatatypeProperty ;
    rdfs:label "Property: end year"@en ;
    rdfs:comment "The :endYear property specifies an end year for a thing."@en ;
    rdfs:domain ns1:Thing ;
    rdfs:isDefinedBy ns1: ;
    rdfs:range xsd:gYear ;
    rdfs:subPropertyOf ns1:dateInfo .

ns1:esmRights a owl:DatatypeProperty ;
    rdfs:label "Property: esm rights"@en ;
    rdfs:comment "The :esmRights property specifies an access right to the electronic supplementary material (ESM) section of a publication as a string value."@en ;
    rdfs:domain ns1:Publication ;
    rdfs:isDefinedBy ns1: ;
    rdfs:range xsd:string ;
    rdfs:subPropertyOf ns1:accessRights .

ns1:familyName a owl:DatatypeProperty ;
    rdfs:label "Property: family name" ;
    rdfs:comment "The :familyName property specifies the family name of a person."@en ;
    rdfs:domain ns1:Person ;
    rdfs:isDefinedBy ns1: ;
    rdfs:range xsd:string ;
    rdfs:subPropertyOf ns1:nameInfo .

ns1:fundingAmount a owl:DatatypeProperty ;
    rdfs:label "Property: funding amount"@en ;
    rdfs:comment "The :fundingAmount property specifies the total original funding for a grant as a decimal number."@en ;
    rdfs:domain ns1:Grant ;
    rdfs:isDefinedBy ns1: ;
    rdfs:range xsd:decimal .

ns1:fundingCurrency a owl:DatatypeProperty ;
    rdfs:label "Property: funding currency"@en ;
    rdfs:comment "The :fundingCurrency property specifies the currency for the original funding of a grant as a string."@en ;
    rdfs:domain ns1:Grant ;
    rdfs:isDefinedBy ns1: ;
    rdfs:range xsd:string .

ns1:givenName a owl:DatatypeProperty ;
    rdfs:label "Property: given name" ;
    rdfs:comment "The :givenName property specifies the given name of a person."@en ;
    rdfs:domain ns1:Person ;
    rdfs:isDefinedBy ns1: ;
    rdfs:range xsd:string ;
    rdfs:subPropertyOf ns1:nameInfo .

ns1:hasAnnotationAgent a owl:ObjectProperty ;
    rdfs:label "Property: has annotation agent"@en ;
    rdfs:comment "The :hasAnnotationAgent property specifies a resource which identifies the annotator agent in an annotation event."@en ;
    rdfs:domain ns1:AnnotationEvent ;
    rdfs:isDefinedBy ns1: ;
    rdfs:range ns1:Agent .

ns1:hasAnnotationCategory a owl:ObjectProperty ;
    rdfs:label "Property: has annotation category"@en ;
    rdfs:comment "The :hasAnnotationCategory property specifies a category which is used to annotate a thing in an annotation event. "@en ;
    rdfs:domain ns1:AnnotationEvent ;
    rdfs:isDefinedBy ns1: ;
    rdfs:range ns1:Category .

ns1:hasAnnotationThing a owl:ObjectProperty ;
    rdfs:label "Property: has annotation thing"@en ;
    rdfs:comment "The :hasAnnotationThing property specifies a thing which is the subject of an annotation event. "@en ;
    rdfs:domain ns1:AnnotationEvent ;
    rdfs:isDefinedBy ns1: ;
    rdfs:range owl:Thing .

ns1:hasCitationMetricsEvent a owl:ObjectProperty ;
    rdfs:label "Property: has citation metrics event"@en ;
    rdfs:comment "The :hasCitationMetricsEvent property specifies a resource which identifies a citation metrics event for a publication."@en ;
    rdfs:isDefinedBy ns1: ;
    rdfs:range ns1:CitationMetricsEvent ;
    rdfs:subPropertyOf ns1:hasMetricsEvent .

ns1:hasConference a owl:ObjectProperty ;
    rdfs:label "Property: has conference"@en ;
    rdfs:comment "The :hasConference property relates a publication (e.g. a conference proceedings volume) to the conference event it relates to."@en ;
    rdfs:domain ns1:Publication ;
    rdfs:isDefinedBy ns1: ;
    rdfs:range ns1:Conference .

ns1:hasContributingOrganization a owl:ObjectProperty ;
    rdfs:label "Property: has contributing organization"@en ;
    rdfs:comment "The :hasContributingOrganization property specifies an organization related to a publication contribution. This is a shortcut property for easy access."@en ;
    rdfs:domain ns1:Publication ;
    rdfs:isDefinedBy ns1: ;
    rdfs:range ns1:Organization .

ns1:hasFieldOfResearchCode a owl:ObjectProperty ;
    rdfs:label "Property: has field-of-research code"@en ;
    rdfs:comment "The :hasFieldOfResearchCode property relates an Australian and New Zealand Standard Research Classification (ANZSRC) Field of Research (FOR) code to a publication."@en ;
    rdfs:domain ns1:Publication ;
    rdfs:isDefinedBy ns1: ;
    rdfs:range ns1:FieldOfResearchCode ;
    rdfs:subPropertyOf ns1:hasCategory .

ns1:hasImpactFactorMetricsEvent a owl:ObjectProperty ;
    rdfs:label "Property: has impact factor metrics event"@en ;
    rdfs:comment "The :hasImpactFactorMetricsEvent property specifies a resource which identifies an impact factor metrics event for a journal brand."@en ;
    rdfs:domain ns1:JournalBrand ;
    rdfs:isDefinedBy ns1: ;
    rdfs:range ns1:MetricsEvent ;
    rdfs:subPropertyOf ns1:hasMetricsEvent .

ns1:hasPrincipalInvestigator a owl:ObjectProperty ;
    rdfs:label "Property: has principal investigator"@en ;
    rdfs:comment "The :hasPrincipalInvestigator property specifies the PI (principal investigator) associated with a grant."@en ;
    rdfs:domain ns1:Grant ;
    rdfs:isDefinedBy ns1: ;
    rdfs:range ns1:Person .

ns1:hasProduct a owl:ObjectProperty ;
    rdfs:label "Property: has product"@en ;
    rdfs:comment "The :hasProduct property relates an abstract work to the product which realizes it."@en ;
    rdfs:domain ns1:Work ;
    rdfs:isDefinedBy ns1: ;
    rdfs:range ns1:Product .

ns1:hasRecipientOrganization a owl:ObjectProperty ;
    rdfs:label "Property: has recipient organization"@en ;
    rdfs:comment "The :hasRecipientOrganization property specifies an organization that has received a grant."@en ;
    rdfs:domain ns1:Grant ;
    rdfs:isDefinedBy ns1: ;
    rdfs:range ns1:Organization .

ns1:hasTechnicalArticleType a owl:ObjectProperty ;
    rdfs:label "Property: has techincal-article-type"@en ;
    rdfs:comment "The :hasTechnicalArticleType relates an article to a technical-article-type."@en ;
    rdfs:domain ns1:Article ;
    rdfs:isDefinedBy ns1: ;
    rdfs:range ns1:TechnicalArticleType .

ns1:homepage a owl:ObjectProperty ;
    rdfs:label "Property: homepage" ;
    rdfs:comment "The :homepage property relates a Scigraph thing to the main page on the web that describes it."@en ;
    rdfs:domain ns1:Thing ;
    rdfs:isDefinedBy ns1: .

ns1:impactFactor a owl:DatatypeProperty ;
    rdfs:label "Property: impact factor"@en ;
    rdfs:comment "The :impactFactor property specifies the impact factor of a citation measurement as a decimal number."@en ;
    rdfs:domain ns1:MetricsEvent ;
    rdfs:isDefinedBy ns1: ;
    rdfs:range xsd:decimal .

ns1:impactFactorFiveYear a owl:DatatypeProperty ;
    rdfs:label "Property: impact factor (five year)"@en ;
    rdfs:comment "The :impactFactorFiveYear property specifies the five-years averaged impact factor of a citation measurement as a decimal number."@en ;
    rdfs:domain ns1:MetricsEvent ;
    rdfs:isDefinedBy ns1: ;
    rdfs:range xsd:decimal .

ns1:imprint a owl:DatatypeProperty ;
    rdfs:label "Property: imprint"@en ;
    rdfs:comment "The :imprint property specifies the imprint of a publication as a string value."@en ;
    rdfs:domain ns1:Publication ;
    rdfs:isDefinedBy ns1: ;
    rdfs:range xsd:string .

ns1:indexingDatabase a owl:DatatypeProperty ;
    rdfs:label "Property: indexing database"@en ;
    rdfs:comment "The :indexingDatabase property specifies the indexing database for an indexed publication as a string value."@en ;
    rdfs:domain ns1:Publication ;
    rdfs:isDefinedBy ns1: ;
    rdfs:range xsd:string .

ns1:intellectualUnitId a owl:DatatypeProperty ;
    rdfs:label "Property: intellectual unit ID"@en ;
    rdfs:comment "The :intellectualUnitId property specifies the ID for an intellectual unit within the BFlux model."@en ;
    rdfs:domain ns1:Publication ;
    rdfs:isDefinedBy ns1: ;
    rdfs:range xsd:string .

ns1:isActivePublication a owl:DatatypeProperty ;
    rdfs:label "Property: is active publication"@en ;
    rdfs:comment "The :isActivePublication property marks whether a :Publication is currently being published."@en ;
    rdfs:domain ns1:Publication ;
    rdfs:isDefinedBy ns1: ;
    rdfs:range xsd:boolean .

ns1:isAffiliationOf a owl:ObjectProperty ;
    rdfs:label "Property: is affiliation of" ;
    rdfs:comment "The :isAffiliationOf property is the inverse of the :hasAffiliation property."@en ;
    rdfs:isDefinedBy ns1: ;
    owl:inverseOf ns1:hasAffiliation .

ns1:isArticleOf a owl:ObjectProperty ;
    rdfs:label "Property: is article of"@en ;
    rdfs:comment "The :isArticleOf property is the inverse of the :hasArticle property."@en ;
    rdfs:isDefinedBy ns1: ;
    owl:inverseOf ns1:hasArticle .

ns1:isArticleTypeOf a owl:ObjectProperty ;
    rdfs:label "Property: is article type of"@en ;
    rdfs:comment "The :isArticleTypeOf property is the inverse of the :hasArticleType property."@en ;
    rdfs:isDefinedBy ns1: ;
    owl:inverseOf ns1:hasArticleType .

ns1:isBookChapterOf a owl:ObjectProperty ;
    rdfs:label "Property: is book chapter of"@en ;
    rdfs:comment "The :isBookChapterOf property is the inverse of the :hasBookChapter property."@en ;
    rdfs:isDefinedBy ns1: ;
    owl:inverseOf ns1:hasBookChapter .

ns1:isBookEditionOf a owl:ObjectProperty ;
    rdfs:label "Property: is book edition of"@en ;
    rdfs:comment "The :isBookEditionOf property is the inverse of the :hasBookEdition property."@en ;
    rdfs:isDefinedBy ns1: ;
    owl:inverseOf ns1:hasBookEdition .

ns1:isBookOf a owl:ObjectProperty ;
    rdfs:label "Property: is book of"@en ;
    rdfs:comment "The :isBookOf property is the inverse of the :hasBook property."@en ;
    rdfs:isDefinedBy ns1: ;
    owl:inverseOf ns1:hasBook .

ns1:isBookSeriesOf a owl:ObjectProperty ;
    rdfs:label "Property: is book series of"@en ;
    rdfs:comment "The :isBookSeriesOf property is the inverse of the :hasBookSeries property."@en ;
    rdfs:isDefinedBy ns1: ;
    owl:inverseOf ns1:hasBookSeries .

ns1:isCategoryOf a owl:ObjectProperty ;
    rdfs:label "Property: is category of"@en ;
    rdfs:comment "The :isCategoryOf property is the inverse of the :isCategoryOf property."@en ;
    rdfs:isDefinedBy ns1: ;
    owl:inverseOf ns1:hasCategory .

ns1:isConferenceSeriesOf a owl:ObjectProperty ;
    rdfs:label "Property: is conference series of"@en ;
    rdfs:comment "The :isConferenceSeriesOf property is the inverse of the :hasConferenceSeries property."@en ;
    rdfs:isDefinedBy ns1: ;
    owl:inverseOf ns1:hasConferenceSeries .

ns1:isContentPublished a owl:DatatypeProperty ;
    rdfs:label "Property: is content published"@en ;
    rdfs:comment "The :isContentPublished property marks whether a :Publication has published content."@en ;
    rdfs:domain ns1:Publication ;
    rdfs:isDefinedBy ns1: ;
    rdfs:range xsd:boolean .

ns1:isContributionOf a owl:ObjectProperty ;
    rdfs:label "Property: is contribution of"@en ;
    rdfs:comment "The :isContributionOf property is the inverse of the :hasContribution property."@en ;
    rdfs:isDefinedBy ns1: ;
    owl:inverseOf ns1:hasContribution .

ns1:isCorresponding a owl:DatatypeProperty ;
    rdfs:label "Property: is corresponding"@en ;
    rdfs:comment "The :isCorresponding property marks whether a :Contribution is by a corresponding author."@en ;
    rdfs:domain ns1:Contribution ;
    rdfs:isDefinedBy ns1: ;
    rdfs:range xsd:boolean .

ns1:isFieldOfResearchCodeOf a owl:ObjectProperty ;
    rdfs:label "Property: is field-of-research code of"@en ;
    rdfs:comment "The :isProductMarketCodeOf property is the inverse of the :hasProductMarketCode property."@en ;
    rdfs:isDefinedBy ns1: ;
    owl:inverseOf ns1:hasProductMarketCode .

ns1:isFundedPublicationOf a owl:ObjectProperty ;
    rdfs:label "Property: is funded publication of"@en ;
    rdfs:comment "The :isFundedPublicationOf property is the inverse of the :hasFundedPublication property."@en ;
    rdfs:isDefinedBy ns1: ;
    owl:inverseOf ns1:hasFundedPublication .

ns1:isFundingOrganizationOf a owl:ObjectProperty ;
    rdfs:label "Property: is funding organization of"@en ;
    rdfs:comment "The :isFundingOrganizationOf property is the inverse of the :hasFundingOrganization property."@en ;
    rdfs:isDefinedBy ns1: ;
    owl:inverseOf ns1:hasFundingOrganization .

ns1:isGroup a owl:DatatypeProperty ;
    rdfs:label "Property: is group"@en ;
    rdfs:comment "The :isGroup property marks whether a :Contribution name refers to a collective agent, i.e. a group of people or an institution."@en ;
    rdfs:domain ns1:Contribution ;
    rdfs:isDefinedBy ns1: ;
    rdfs:range xsd:boolean .

ns1:isHistoricalJournal a owl:DatatypeProperty ;
    rdfs:label "Property: is historical journal"@en ;
    rdfs:comment "The :isHistoricalJournal property marks whether a :Journal is an historical version of a more recent :Journal (marked by having a different ISSN). In order to retrieve the most recent version of it, the related :JournalBrand object should be used."@en ;
    rdfs:domain ns1:Publication ;
    rdfs:isDefinedBy ns1: ;
    rdfs:range xsd:boolean .

ns1:isIssueBased a owl:DatatypeProperty ;
    rdfs:label "Property: is issue-based"@en ;
    rdfs:comment "The :isIssueBased property marks whether a journal publishes issues."@en ;
    rdfs:domain ns1:Journal ;
    rdfs:isDefinedBy ns1: ;
    rdfs:range xsd:boolean .

ns1:isJournalBrandOf a owl:ObjectProperty ;
    rdfs:label "Property: is journal brand of"@en ;
    rdfs:comment "The :isJournalBrandOf property is the inverse of the :hasJournalBrand property."@en ;
    rdfs:isDefinedBy ns1: ;
    owl:inverseOf ns1:hasJournalBrand .

ns1:isJournalOf a owl:ObjectProperty ;
    rdfs:label "Property: is journal of"@en ;
    rdfs:comment "The :isJournalOf property is the inverse of the :hasJournal property."@en ;
    rdfs:isDefinedBy ns1: ;
    owl:inverseOf ns1:hasJournal .

ns1:isLeaf a owl:DatatypeProperty ;
    rdfs:label "Property: is leaf"@en ;
    rdfs:comment "The :isLeaf property marks whether a SKOS concept is a leaf SKOS concept."@en ;
    rdfs:domain ns1:Concept ;
    rdfs:isDefinedBy ns1: ;
    rdfs:range xsd:boolean .

ns1:isOpenAccess a owl:DatatypeProperty ;
    rdfs:label "Property: is open access"@en ;
    rdfs:comment "The :isOpenAccess property marks whether an article has an open access license."@en ;
    rdfs:domain ns1:Article ;
    rdfs:isDefinedBy ns1: ;
    rdfs:range xsd:boolean .

ns1:isOrganizationOf a owl:ObjectProperty ;
    rdfs:label "Property: is organization of"@en ;
    rdfs:comment "The :isOrganizationOf property is the inverse of the :hasOrganization property."@en ;
    rdfs:isDefinedBy ns1: ;
    rdfs:subPropertyOf ns1:isAgentOf ;
    owl:inverseOf ns1:hasOrganization .

ns1:isPersonOf a owl:ObjectProperty ;
    rdfs:label "Property: is person of"@en ;
    rdfs:comment "The :isPersonOf property is the inverse of the :hasPerson property."@en ;
    rdfs:isDefinedBy ns1: ;
    rdfs:subPropertyOf ns1:isAgentOf ;
    owl:inverseOf ns1:hasAgent .

ns1:isPrincipalInvestigatorOf a owl:ObjectProperty ;
    rdfs:label "Property: is principal investigator of"@en ;
    rdfs:comment "The :isPrincipalInvestigatorOf property is the inverse of the :hasPrincipalInvestigator property."@en ;
    rdfs:isDefinedBy ns1: ;
    owl:inverseOf ns1:hasPerson .

ns1:isProductMarketCodeOf a owl:ObjectProperty ;
    rdfs:label "Property: is product-market-code of"@en ;
    rdfs:comment "The :isProductMarketCodeOf property is the inverse of the :hasProductMarketCode property."@en ;
    rdfs:isDefinedBy ns1: ;
    owl:inverseOf ns1:hasAgent .

ns1:isPublicationOf a owl:ObjectProperty ;
    rdfs:label "Property: is publication of"@en ;
    rdfs:comment "The :isPublicationOf property is the inverse of the :hasPublication property."@en ;
    rdfs:isDefinedBy ns1: ;
    owl:inverseOf ns1:hasPublication .

ns1:isPublishEventOf a owl:ObjectProperty ;
    rdfs:label "Property: is publish event of"@en ;
    rdfs:comment "The :isPublishEventOf property is the inverse of the :hasPublishEvent property."@en ;
    rdfs:isDefinedBy ns1: ;
    owl:inverseOf ns1:hasPublishEvent .

ns1:isPublishStateOf a owl:ObjectProperty ;
    rdfs:label "Property: is publish state of"@en ;
    rdfs:comment "The :isPublishStateOf property is the inverse of the :hasPublishState property."@en ;
    rdfs:isDefinedBy ns1: ;
    owl:inverseOf ns1:hasPublishState .

ns1:isPublisherOf a owl:ObjectProperty ;
    rdfs:label "Property: is publisher of"@en ;
    rdfs:comment "The :isPublisherOf property is the inverse of the :hasPublisher property."@en ;
    rdfs:isDefinedBy ns1: ;
    owl:inverseOf ns1:hasPublisher .

ns1:isRecipientOrganizationOf a owl:ObjectProperty ;
    rdfs:label "Property: is recipient organization of"@en ;
    rdfs:comment "The :isRecipientOrganizationOf property is the inverse of the :hasRecipientOrganization property."@en ;
    rdfs:isDefinedBy ns1: ;
    owl:inverseOf ns1:hasAgent .

ns1:isReviewEventOf a owl:ObjectProperty ;
    rdfs:label "Property: is review event of"@en ;
    rdfs:comment "The :isReviewEventOf property is the inverse of the :hasReviewEvent property."@en ;
    rdfs:isDefinedBy ns1: ;
    owl:inverseOf ns1:hasReviewEvent .

ns1:isReviewStateOf a owl:ObjectProperty ;
    rdfs:label "Property: is review state of"@en ;
    rdfs:comment "The :isReviewStateOf property is the inverse of the :hasReviewState property."@en ;
    rdfs:isDefinedBy ns1: ;
    owl:inverseOf ns1:hasReviewState .

ns1:isRoot a owl:DatatypeProperty ;
    rdfs:label "Property: is root"@en ;
    rdfs:comment "The :isRoot property marks whether a SKOS concept is a SKOS top concept."@en ;
    rdfs:domain ns1:Concept ;
    rdfs:isDefinedBy ns1: ;
    rdfs:range xsd:boolean .

ns1:isRootOf a owl:ObjectProperty ;
    rdfs:label "Property: is root of"@en ;
    rdfs:comment "The :isRootOf property is the inverse of the :hasRoot property."@en ;
    rdfs:isDefinedBy ns1: ;
    owl:inverseOf ns1:hasRoot .

ns1:isSerialOf a owl:ObjectProperty ;
    rdfs:label "Property: is serial of"@en ;
    rdfs:comment "The :isSerialOf property is the inverse of the :hasSerial property."@en ;
    rdfs:isDefinedBy ns1: ;
    owl:inverseOf ns1:hasSerial .

ns1:isSubjectOf a owl:ObjectProperty ;
    rdfs:label "Property: is subject of"@en ;
    rdfs:comment "The :isSubjectOf property is the inverse of the :hasSubject property."@en ;
    rdfs:isDefinedBy ns1: ;
    owl:inverseOf ns1:hasSubject .

ns1:isWorkOf a owl:ObjectProperty ;
    rdfs:label "Property: has work"@en ;
    rdfs:comment "The :isWorkOf property is the inverse of the :hasWork property."@en ;
    rdfs:isDefinedBy ns1: ;
    owl:inverseOf ns1:hasWork .

ns1:isbn a owl:DatatypeProperty ;
    rdfs:label "Property: ISBN"@en ;
    rdfs:comment "The :isbn property specifies the ISBN number for a publication."@en ;
    rdfs:domain ns1:Publication ;
    rdfs:isDefinedBy ns1: ;
    rdfs:range xsd:string .

ns1:issnElectronic a owl:DatatypeProperty ;
    rdfs:label "Property: ISSN (electronic)" ;
    rdfs:comment "The :issnElectronic property specifies an ISSN number for a serial as an electronic publication."@en ;
    rdfs:domain ns1:Publication ;
    rdfs:isDefinedBy ns1: ;
    rdfs:range xsd:string ;
    rdfs:subPropertyOf ns1:issn .

ns1:issnPrint a owl:DatatypeProperty ;
    rdfs:label "Property: ISSN (print)" ;
    rdfs:comment "The :issnPrint property specifies an ISSN number for a serial as a print publication."@en ;
    rdfs:domain ns1:Publication ;
    rdfs:isDefinedBy ns1: ;
    rdfs:range xsd:string ;
    rdfs:subPropertyOf ns1:issn .

ns1:issue a owl:DatatypeProperty ;
    rdfs:label "Property: issue" ;
    rdfs:comment "The :issue property specifies an issue label for a publication."@en ;
    rdfs:domain ns1:Publication ;
    rdfs:isDefinedBy ns1: ;
    rdfs:range xsd:string .

ns1:issueEnd a owl:DatatypeProperty ;
    rdfs:label "Property: issue end"@en ;
    rdfs:comment "The :issueEnd property specifies the end issue for a serial publication. Note that this :issueEnd property relates to the publisher holdings which may not be the same as the actual publication issue end."@en ;
    rdfs:domain ns1:Publication ;
    rdfs:isDefinedBy ns1: ;
    rdfs:range xsd:string .

ns1:issueStart a owl:DatatypeProperty ;
    rdfs:label "Property: issue start"@en ;
    rdfs:comment "The :issueStart property specifies the start issue for a serial publication. Note that this :issueStart property relates to the publisher holdings which may not be the same as the actual publication issue start."@en ;
    rdfs:domain ns1:Publication ;
    rdfs:isDefinedBy ns1: ;
    rdfs:range xsd:string .

ns1:labelTreeDepth0 a owl:DatatypeProperty ;
    rdfs:label "Property: label (tree depth 0)"@en ;
    rdfs:comment "The :labelTreeDepth0 property specifies the label for a concept at a tree depth of 0."@en ;
    rdfs:domain skos:Concept ;
    rdfs:isDefinedBy ns1: ;
    rdfs:range xsd:string ;
    rdfs:subPropertyOf ns1:label .

ns1:labelTreeDepth1 a owl:DatatypeProperty ;
    rdfs:label "Property: label (tree depth 1)"@en ;
    rdfs:comment "The :labelTreeDepth1 property specifies the label for a concept at a tree depth of 1."@en ;
    rdfs:domain skos:Concept ;
    rdfs:isDefinedBy ns1: ;
    rdfs:range xsd:string ;
    rdfs:subPropertyOf ns1:label .

ns1:labelTreeDepth2 a owl:DatatypeProperty ;
    rdfs:label "Property: label (tree depth 2)"@en ;
    rdfs:comment "The :labelTreeDepth2 property specifies the label for a concept at a tree depth of 2."@en ;
    rdfs:domain skos:Concept ;
    rdfs:isDefinedBy ns1: ;
    rdfs:range xsd:string ;
    rdfs:subPropertyOf ns1:label .

ns1:labelTreeDepth3 a owl:DatatypeProperty ;
    rdfs:label "Property: label (tree depth 3)"@en ;
    rdfs:comment "The :labelTreeDepth3 property specifies the label for a concept at a tree depth of 3."@en ;
    rdfs:domain skos:Concept ;
    rdfs:isDefinedBy ns1: ;
    rdfs:range xsd:string ;
    rdfs:subPropertyOf ns1:label .

ns1:labelTreeDepth4 a owl:DatatypeProperty ;
    rdfs:label "Property: label (tree depth 4)"@en ;
    rdfs:comment "The :labelTreeDepth4 property specifies the label for a concept at a tree depth of 4."@en ;
    rdfs:domain skos:Concept ;
    rdfs:isDefinedBy ns1: ;
    rdfs:range xsd:string ;
    rdfs:subPropertyOf ns1:label .

ns1:labelTreeDepth5 a owl:DatatypeProperty ;
    rdfs:label "Property: label (tree depth 5)"@en ;
    rdfs:comment "The :labelTreeDepth5 property specifies the label for a concept at a tree depth of 5."@en ;
    rdfs:domain skos:Concept ;
    rdfs:isDefinedBy ns1: ;
    rdfs:range xsd:string ;
    rdfs:subPropertyOf ns1:label .

ns1:labelTreeDepth6 a owl:DatatypeProperty ;
    rdfs:label "Property: label (tree depth 6)"@en ;
    rdfs:comment "The :labelTreeDepth6 property specifies the label for a concept at a tree depth of 6."@en ;
    rdfs:domain skos:Concept ;
    rdfs:isDefinedBy ns1: ;
    rdfs:range xsd:string ;
    rdfs:subPropertyOf ns1:label .

ns1:labelTreeDepth7 a owl:DatatypeProperty ;
    rdfs:label "Property: label (tree depth 7)"@en ;
    rdfs:comment "The :labelTreeDepth7 property specifies the label for a concept at a tree depth of 7."@en ;
    rdfs:domain skos:Concept ;
    rdfs:isDefinedBy ns1: ;
    rdfs:range xsd:string ;
    rdfs:subPropertyOf ns1:label .

ns1:language a owl:DatatypeProperty ;
    rdfs:label "Property: language"@en ;
    rdfs:comment "The :language property specifies the language of a publication as a string value."@en ;
    rdfs:domain ns1:Publication ;
    rdfs:isDefinedBy ns1: ;
    rdfs:range xsd:string .

ns1:license a owl:DatatypeProperty ;
    rdfs:label "Property: license"@en ;
    rdfs:comment "The :license property specifies a the license terms for an object as a string."@en ;
    rdfs:isDefinedBy ns1: ;
    rdfs:range xsd:string .

ns1:medium a owl:DatatypeProperty ;
    rdfs:label "Property: medium"@en ;
    rdfs:comment "The :medium property specifies the medium in which a product is rendered as a string value."@en ;
    rdfs:domain ns1:Product ;
    rdfs:isDefinedBy ns1: ;
    rdfs:range xsd:string .

ns1:mesh a owl:ObjectProperty ;
    rdfs:label "Property: MeSH"@en ;
    rdfs:comment "The :mesh property relates a thing to a Medical Subject Heading (MeSH) term as a resource."@en ;
    rdfs:domain ns1:Thing ;
    rdfs:isDefinedBy ns1: ;
    rdfs:seeAlso <http://id.nlm.nih.gov/mesh/> .

ns1:meshTerm a owl:DatatypeProperty ;
    rdfs:label "Property: MeSH term"@en ;
    rdfs:comment "The :meshTerm property specifies a Medical Subject Heading (MeSH) term as a string."@en ;
    rdfs:domain ns1:Thing ;
    rdfs:isDefinedBy ns1: ;
    rdfs:range xsd:string ;
    rdfs:seeAlso <http://id.nlm.nih.gov/mesh/> .

ns1:metadataRights a owl:DatatypeProperty ;
    rdfs:label "Property: metadata rights"@en ;
    rdfs:comment "The :metadataRights property specifies an access right to the metadata section of a publication as a string value."@en ;
    rdfs:domain ns1:Publication ;
    rdfs:isDefinedBy ns1: ;
    rdfs:range xsd:string ;
    rdfs:subPropertyOf ns1:accessRights .

ns1:name a owl:DatatypeProperty ;
    rdfs:label "Property: name" ;
    rdfs:comment "The :name property specifies the full name for a thing."@en ;
    rdfs:domain ns1:Thing ;
    rdfs:isDefinedBy ns1: ;
    rdfs:range xsd:string ;
    rdfs:subPropertyOf ns1:nameInfo .

ns1:npgId a owl:DatatypeProperty ;
    rdfs:label "Property: NPG ID"@en ;
    rdfs:comment "The :npgId property specifies an ID within the Nature.com dataset."@en ;
    rdfs:domain ns1:Thing ;
    rdfs:isDefinedBy ns1: ;
    rdfs:range xsd:string ;
    rdfs:subPropertyOf ns1:id .

ns1:number a owl:DatatypeProperty ;
    rdfs:label "Property: number"@en ;
    rdfs:comment "The :number property specifies a sequence number for a thing, e.g. component such as a figure, or a conference number."@en ;
    rdfs:domain ns1:Thing ;
    rdfs:isDefinedBy ns1: ;
    rdfs:range xsd:integer .

ns1:oldCode a owl:DatatypeProperty ;
    rdfs:label "Property: old code"@en ;
    rdfs:comment "The :oldCode property specifies a number or string previously used by the domain ontologies as an ID for an entity."@en ;
    rdfs:domain ns1:Concept ;
    rdfs:isDefinedBy ns1: ;
    rdfs:range xsd:string .

ns1:openAccess a owl:DatatypeProperty ;
    rdfs:label "Property: open access"@en ;
    rdfs:comment "The :openAccess property specifies the open access policy of a publication as a string value."@en ;
    rdfs:domain ns1:Publication ;
    rdfs:isDefinedBy ns1: ;
    rdfs:range xsd:string .

ns1:order a owl:DatatypeProperty ;
    rdfs:label "Property: order"@en ;
    rdfs:comment "The :order property specifies a sequence number for an entity such as a figure, a dataset or a contributor."@en ;
    rdfs:domain ns1:Thing ;
    rdfs:isDefinedBy ns1: ;
    rdfs:range xsd:integer .

ns1:otherCode a owl:DatatypeProperty ;
    rdfs:label "Property: other code"@en ;
    rdfs:comment "The :otherCode property specifies a number or string used by external applications as an ID for an entity."@en ;
    rdfs:domain ns1:Concept ;
    rdfs:isDefinedBy ns1: ;
    rdfs:range xsd:string .

ns1:pageEnd a owl:DatatypeProperty ;
    rdfs:label "Property: page end" ;
    rdfs:comment "The :pageEnd property specifies an ending page number for a document."@en ;
    rdfs:domain ns1:Publication ;
    rdfs:isDefinedBy ns1: ;
    rdfs:range xsd:string .

ns1:pageStart a owl:DatatypeProperty ;
    rdfs:label "Property: page start" ;
    rdfs:comment "The :pageStart property specifies a starting page number for a document."@en ;
    rdfs:domain ns1:Publication ;
    rdfs:isDefinedBy ns1: ;
    rdfs:range xsd:string .

ns1:pages a owl:DatatypeProperty ;
    rdfs:label "Property: pages" ;
    rdfs:comment "The :pages property specifies a page range numbering for a document."@en ;
    rdfs:domain ns1:Publication ;
    rdfs:isDefinedBy ns1: ;
    rdfs:range xsd:string .

ns1:pcode a owl:DatatypeProperty ;
    rdfs:label "Property: pcode"@en ;
    rdfs:comment "The :pcode property specifies a unique ID for a publication. The term :pcode derives from product code and has been used as a unique ID for publications such as journals, blogs, etc."@en ;
    rdfs:domain ns1:Publication ;
    rdfs:isDefinedBy ns1: ;
    rdfs:range xsd:string .

ns1:pluralLabel a owl:DatatypeProperty ;
    rdfs:label "Property: plural label"@en ;
    rdfs:comment "The :pluralLabel property specifies a plural form for the preferred label."@en ;
    rdfs:isDefinedBy ns1: ;
    rdfs:range rdf:langString ;
    rdfs:subPropertyOf ns1:nameInfo .

ns1:publicationDateTime a owl:DatatypeProperty ;
    rdfs:label "Property: publication datetime"@en ;
    rdfs:comment "The :publicationDateTime property specifies the first known date of a publication, either in electronic form or print, including the time of publication."@en ;
    rdfs:domain ns1:Publication ;
    rdfs:isDefinedBy ns1: ;
    rdfs:range xsd:dateTime ;
    rdfs:subPropertyOf ns1:dateInfo .

ns1:publicationEndDate a owl:DatatypeProperty ;
    rdfs:label "Property: publication end date"@en ;
    rdfs:comment "The :publicationEndDate property specifies the full date of a publication's end as a string. Note that this date relates to the publisher holdings which may not be the same as the actual publication end date."@en ;
    rdfs:domain ns1:Publication ;
    rdfs:isDefinedBy ns1: ;
    rdfs:range xsd:date ;
    rdfs:subPropertyOf ns1:publicationDate .

ns1:publicationEndYear a owl:DatatypeProperty ;
    rdfs:label "Property: publication end year"@en ;
    rdfs:comment "The :publicationEndYear property specifies the year date of a publication's end as a string. Note that this date relates to the publisher holdings which may not be the same as the actual publication end date."@en ;
    rdfs:domain ns1:Publication ;
    rdfs:isDefinedBy ns1: ;
    rdfs:range xsd:gYear ;
    rdfs:subPropertyOf ns1:dateInfo .

ns1:publicationEndYearMonth a owl:DatatypeProperty ;
    rdfs:label "Property: publication end year-month"@en ;
    rdfs:comment "The :publicationEndYearMonth property specifies the year and month date of a publication's end as a string. Note that this date relates to the publisher holdings which may not be the same as the actual publication end date."@en ;
    rdfs:domain ns1:Publication ;
    rdfs:isDefinedBy ns1: ;
    rdfs:range xsd:gYearMonth ;
    rdfs:subPropertyOf ns1:dateInfo .

ns1:publicationName a owl:DatatypeProperty ;
    rdfs:label "Property: publication name"@en ;
    rdfs:comment "The :publicationName property specifies a string name for an external publication."@en ;
    rdfs:domain ns1:Publication ;
    rdfs:isDefinedBy ns1: ;
    rdfs:range xsd:string ;
    rdfs:subPropertyOf ns1:nameInfo .

ns1:publicationStartDate a owl:DatatypeProperty ;
    rdfs:label "Property: publication start date"@en ;
    rdfs:comment "The :publicationStartDate property specifies the full date of a publication's start as a string. Note that this date relates to the publisher holdings which may not be the same as the actual publication start date."@en ;
    rdfs:domain ns1:Publication ;
    rdfs:isDefinedBy ns1: ;
    rdfs:range xsd:date ;
    rdfs:subPropertyOf ns1:publicationDate .

ns1:publicationStartYear a owl:DatatypeProperty ;
    rdfs:label "Property: publication start year"@en ;
    rdfs:comment "The :publicationStartYear property specifies the year date of a publication's start as a string. Note that this date relates to the publisher holdings which may not be the same as the actual publication start date."@en ;
    rdfs:domain ns1:Publication ;
    rdfs:isDefinedBy ns1: ;
    rdfs:range xsd:gYear ;
    rdfs:subPropertyOf ns1:dateInfo .

ns1:publicationStartYearMonth a owl:DatatypeProperty ;
    rdfs:label "Property: publication start year-month"@en ;
    rdfs:comment "The :publicationStartYearMonth property specifies the year and month date of a publication's start as a string. Note that this date relates to the publisher holdings which may not be the same as the actual publication start date."@en ;
    rdfs:domain ns1:Publication ;
    rdfs:isDefinedBy ns1: ;
    rdfs:range xsd:gYearMonth ;
    rdfs:subPropertyOf ns1:dateInfo .

ns1:publicationYear a owl:DatatypeProperty ;
    rdfs:label "Property: publication year"@en ;
    rdfs:comment "The :publicationYear property specifies the first known year date of a publication, either in electronic form or print, as a string."@en ;
    rdfs:domain ns1:Publication ;
    rdfs:isDefinedBy ns1: ;
    rdfs:range xsd:gYear ;
    rdfs:subPropertyOf ns1:dateInfo .

ns1:publicationYearMonth a owl:DatatypeProperty ;
    rdfs:label "Property: publication year-month"@en ;
    rdfs:comment "The :publicationYearMonth property specifies the first known year and month date of a publication, either in electronic form or print, as a string."@en ;
    rdfs:domain ns1:Publication ;
    rdfs:isDefinedBy ns1: ;
    rdfs:range xsd:gYearMonth ;
    rdfs:subPropertyOf ns1:dateInfo .

ns1:publishedCity a owl:DatatypeProperty ;
    rdfs:label "Property: published city" ;
    rdfs:comment "The :publishedCity property specifies the name of a city, as it appears in the context of an event, e.g. a publication."@en ;
    rdfs:domain ns1:Event ;
    rdfs:isDefinedBy ns1: ;
    rdfs:range xsd:string ;
    rdfs:subPropertyOf ns1:nameInfo .

ns1:publishedCountry a owl:DatatypeProperty ;
    rdfs:label "Property: published country" ;
    rdfs:comment "The :publishedCountry property specifies the name of a country, as it appears in the context of an event, e.g. a publication."@en ;
    rdfs:domain ns1:Event ;
    rdfs:isDefinedBy ns1: ;
    rdfs:range xsd:string ;
    rdfs:subPropertyOf ns1:nameInfo .

ns1:publishedDivision a owl:DatatypeProperty ;
    rdfs:label "Property: published division" ;
    rdfs:comment "The :publishedDivision property specifies the name of a division, as it appears in the context of an event, e.g. a publication."@en ;
    rdfs:domain ns1:Event ;
    rdfs:isDefinedBy ns1: ;
    rdfs:range xsd:string ;
    rdfs:subPropertyOf ns1:nameInfo .

ns1:publishedFamilyName a owl:DatatypeProperty ;
    rdfs:label "Property: published family name" ;
    rdfs:comment "The :publishedFamilyName property specifies the family name of a person, as it appears in the context of an event, e.g. a publication."@en ;
    rdfs:domain ns1:Event ;
    rdfs:isDefinedBy ns1: ;
    rdfs:range xsd:string ;
    rdfs:subPropertyOf ns1:nameInfo .

ns1:publishedGivenName a owl:DatatypeProperty ;
    rdfs:label "Property: published given name" ;
    rdfs:comment "The :publishedGivenName property specifies the given name of a person, as it appears in the context of an event, e.g. a publication."@en ;
    rdfs:domain ns1:Event ;
    rdfs:isDefinedBy ns1: ;
    rdfs:range xsd:string ;
    rdfs:subPropertyOf ns1:nameInfo .

ns1:publishedName a owl:DatatypeProperty ;
    rdfs:label "Property: published name" ;
    rdfs:comment "The :publishedName property specifies the full name of a person, as it appears in the context of an event, e.g. a publication."@en ;
    rdfs:domain ns1:Event ;
    rdfs:isDefinedBy ns1: ;
    rdfs:range xsd:string ;
    rdfs:subPropertyOf ns1:nameInfo .

ns1:publishedPostbox a owl:DatatypeProperty ;
    rdfs:label "Property: published postbox" ;
    rdfs:comment "The :publishedPostbox property specifies the name of a postbox, as it appears in the context of an event, e.g. a publication."@en ;
    rdfs:domain ns1:Event ;
    rdfs:isDefinedBy ns1: ;
    rdfs:range xsd:string ;
    rdfs:subPropertyOf ns1:nameInfo .

ns1:publishedPostcode a owl:DatatypeProperty ;
    rdfs:label "Property: published postcode" ;
    rdfs:comment "The :publishedPostcode property specifies the name of a postcode, as it appears in the context of an event, e.g. a publication."@en ;
    rdfs:domain ns1:Event ;
    rdfs:isDefinedBy ns1: ;
    rdfs:range xsd:string ;
    rdfs:subPropertyOf ns1:nameInfo .

ns1:publishedState a owl:DatatypeProperty ;
    rdfs:label "Property: published state" ;
    rdfs:comment "The :publishedState property specifies the name of a state, as it appears in the context of an event, e.g. a publication."@en ;
    rdfs:domain ns1:Event ;
    rdfs:isDefinedBy ns1: ;
    rdfs:range xsd:string ;
    rdfs:subPropertyOf ns1:nameInfo .

ns1:publishedStreet a owl:DatatypeProperty ;
    rdfs:label "Property: published street" ;
    rdfs:comment "The :publishedStreet property specifies the name of a street, as it appears in the context of an event, e.g. a publication."@en ;
    rdfs:domain ns1:Event ;
    rdfs:isDefinedBy ns1: ;
    rdfs:range xsd:string ;
    rdfs:subPropertyOf ns1:nameInfo .

ns1:publisher a owl:DatatypeProperty ;
    rdfs:label "Property: publisher"@en ;
    rdfs:comment "The :publisher property specifies the publisher of a publication as a string value."@en ;
    rdfs:domain ns1:Publication ;
    rdfs:isDefinedBy ns1: ;
    rdfs:range xsd:string .

ns1:pubmedId a owl:DatatypeProperty ;
    rdfs:label "Property: PubMed ID"@en ;
    rdfs:comment "The :pubmedId property specifies an ID within the PubMed dataset."@en ;
    rdfs:domain ns1:Publication ;
    rdfs:isDefinedBy ns1: ;
    rdfs:range xsd:string ;
    rdfs:subPropertyOf ns1:id .

ns1:relation a owl:ObjectProperty ;
    rdfs:label "Property: relation"@en ;
    rdfs:comment "The :relation property relates a publication to a publication."@en ;
    rdfs:domain ns1:Publication ;
    rdfs:isDefinedBy ns1: ;
    rdfs:range ns1:Publication .

ns1:role a owl:DatatypeProperty ;
    rdfs:label "Property: role" ;
    rdfs:comment "The :role property specifies the role of an entity as a string, e.g. in the context of a :Contribution. This may be 'author' or 'editor'."@en ;
    rdfs:domain ns1:Thing ;
    rdfs:isDefinedBy ns1: ;
    rdfs:range xsd:string .

ns1:scigraphId a owl:DatatypeProperty ;
    rdfs:label "Property: Scigraph ID"@en ;
    rdfs:comment "The :scigraphId property provides a unique ID for a Scigraph thing. The :scigraphId value forms the local part of the full Scigraph URI for an entity name."@en ;
    rdfs:domain ns1:Thing ;
    rdfs:isDefinedBy ns1: ;
    rdfs:range xsd:string ;
    rdfs:subPropertyOf ns1:id .

ns1:score a owl:DatatypeProperty ;
    rdfs:label "Property: score"@en ;
    rdfs:comment "The :score property specifies an evaluation metric associated with an entity and derived from some test regime. The property value is expressed as a decimal number."@en ;
    rdfs:domain ns1:Thing ;
    rdfs:isDefinedBy ns1: ;
    rdfs:range xsd:decimal .

ns1:shortTitle a owl:DatatypeProperty ;
    rdfs:label "Property: short title" ;
    rdfs:comment "The :shortTitle property specifies an abbreviated title for a publication."@en ;
    rdfs:domain ns1:Publication ;
    rdfs:isDefinedBy ns1: ;
    rdfs:range xsd:string ;
    rdfs:subPropertyOf ns1:nameInfo .

ns1:startYear a owl:DatatypeProperty ;
    rdfs:label "Property: start year"@en ;
    rdfs:comment "The :startYear property specifies a start year for a thing."@en ;
    rdfs:domain ns1:Thing ;
    rdfs:isDefinedBy ns1: ;
    rdfs:range xsd:gYear ;
    rdfs:subPropertyOf ns1:dateInfo .

ns1:submittedBy a owl:DatatypeProperty ;
    rdfs:label "Property: submitted by"@en ;
    rdfs:comment "The :submittedBy property specifies the email address of a submitter. This property is used to record who submitted a new definition for a :Subject term."@en ;
    rdfs:domain ns1:Subject ;
    rdfs:isDefinedBy ns1: ;
    rdfs:range xsd:string .

ns1:subtitle a owl:DatatypeProperty ;
    rdfs:label "Property: subtitle"@en ;
    rdfs:comment "The :subtitle property specifies a subtitle for a thing as a string value."@en ;
    rdfs:domain ns1:Thing ;
    rdfs:isDefinedBy ns1: ;
    rdfs:range xsd:string ;
    rdfs:subPropertyOf ns1:nameInfo .

ns1:subtitleXml a owl:DatatypeProperty ;
    rdfs:label "Property: subtitle (XML)"@en ;
    rdfs:comment "The :subtitleXml property specifies a subtitle in XML format for a thing as a string value."@en ;
    rdfs:domain ns1:Thing ;
    rdfs:isDefinedBy ns1: ;
    rdfs:range xsd:string ;
    rdfs:subPropertyOf ns1:nameInfo .

ns1:subtypeLabel a owl:DatatypeProperty ;
    rdfs:label "Property: subtype label"@en ;
    rdfs:comment "The :subtypeLabel property specifies a label for a subject subtyoe."@en ;
    rdfs:domain ns1:Subject ;
    rdfs:isDefinedBy ns1: ;
    rdfs:range xsd:string ;
    rdfs:subPropertyOf ns1:nameInfo .

ns1:test a owl:DatatypeProperty ;
    rdfs:label "Property: test"@en ;
    rdfs:comment "The :test property specifies a general string test property."@en ;
    rdfs:isDefinedBy ns1: .

ns1:timestamp a owl:DatatypeProperty ;
    rdfs:label "Property: timestamp"@en ;
    rdfs:comment "The :timestamp property specifies a generic timestamp for an object."@en ;
    rdfs:isDefinedBy ns1: ;
    rdfs:range xsd:integer .

ns1:title a owl:DatatypeProperty ;
    rdfs:label "Property: title"@en ;
    rdfs:comment "The :title property specifies a title for a thing as a plain string."@en ;
    rdfs:domain ns1:Thing ;
    rdfs:isDefinedBy ns1: ;
    rdfs:range xsd:string ;
    rdfs:subPropertyOf ns1:nameInfo .

ns1:titleAddedYear a owl:DatatypeProperty ;
    rdfs:label "Property: title added year"@en ;
    rdfs:comment "The :titleAddedYear property specifies the year date in which a publication was added to the database."@en ;
    rdfs:domain ns1:Publication ;
    rdfs:isDefinedBy ns1: ;
    rdfs:range xsd:gYear ;
    rdfs:subPropertyOf ns1:dateInfo .

ns1:titleTranslated a owl:DatatypeProperty ;
    rdfs:label "Property: title translated"@en ;
    rdfs:comment "The :titleTranslated property specifies a title for a thing as a language-tagged string."@en ;
    rdfs:domain ns1:Thing ;
    rdfs:isDefinedBy ns1: ;
    rdfs:range rdf:langString ;
    rdfs:subPropertyOf ns1:nameInfo .

ns1:titleXml a owl:DatatypeProperty ;
    rdfs:label "Property: title (XML)"@en ;
    rdfs:comment "The :titleXml property specifies a title in XML format for a thing as a string value."@en ;
    rdfs:domain ns1:Thing ;
    rdfs:isDefinedBy ns1: ;
    rdfs:range xsd:string ;
    rdfs:subPropertyOf ns1:nameInfo .

ns1:treeDepth a owl:DatatypeProperty ;
    rdfs:label "Property: tree depth"@en ;
    rdfs:comment "The :treeDepth property specifies the depth of a term within a taxonomy tree. This property is generally computed by a build-time rule"@en ;
    rdfs:domain ns1:Concept ;
    rdfs:isDefinedBy ns1: ;
    rdfs:range xsd:integer .

ns1:volume a owl:DatatypeProperty ;
    rdfs:label "Property: volume" ;
    rdfs:comment "The :volume property specifies a volume label for a publication."@en ;
    rdfs:domain ns1:Publication ;
    rdfs:isDefinedBy ns1: ;
    rdfs:range xsd:string .

ns1:volumeCount a owl:DatatypeProperty ;
    rdfs:label "Property: volume count"@en ;
    rdfs:comment "The :volumeCount property specifies a total count for the number of volumes within a publication."@en ;
    rdfs:domain ns1:Publication ;
    rdfs:isDefinedBy ns1: ;
    rdfs:range xsd:integer ;
    rdfs:subPropertyOf ns1:count .

ns1:volumeEnd a owl:DatatypeProperty ;
    rdfs:label "Property: volume end"@en ;
    rdfs:comment "The :volumeEnd property specifies the end volume for a serial publication. Note that this :volumeEnd property relates to the publisher holdings which may not be the same as the actual publication volume end."@en ;
    rdfs:domain ns1:Publication ;
    rdfs:isDefinedBy ns1: ;
    rdfs:range xsd:string .

ns1:volumeStart a owl:DatatypeProperty ;
    rdfs:label "Property: volume start"@en ;
    rdfs:comment "The :volumeStart property specifies the start volume for a serial publication. Note that this :volumeStart property relates to the publisher holdings which may not be the same as the actual publication volume start."@en ;
    rdfs:domain ns1:Publication ;
    rdfs:isDefinedBy ns1: ;
    rdfs:range xsd:string .

ns1:year a owl:DatatypeProperty ;
    rdfs:label "Property: year"@en ;
    rdfs:comment "The :date property specifies the year date of an event as a string."@en ;
    rdfs:domain ns1:Event ;
    rdfs:isDefinedBy ns1: ;
    rdfs:range xsd:gYear ;
    rdfs:subPropertyOf ns1:dateInfo .

ns1:yearMonth a owl:DatatypeProperty ;
    rdfs:label "Property: year-month"@en ;
    rdfs:comment "The :date property specifies the year and month date of an event as a string."@en ;
    rdfs:domain ns1:Event ;
    rdfs:isDefinedBy ns1: ;
    rdfs:range xsd:gYearMonth ;
    rdfs:subPropertyOf ns1:dateInfo .

ns1:Affiliation a owl:Class ;
    rdfs:label "Class: Affiliation"@en ;
    ns1:namespace "affiliations" ;
    rdfs:comment "The :Affiliation class groups together events that describe the affiliation of a person with a specific organization (eg university, research institution)."@en ;
    rdfs:isDefinedBy ns1: ;
    rdfs:subClassOf ns1:Event .

ns1:ArticleType a owl:Class ;
    rdfs:label "Class: Article type"@en ;
    ns1:namespace "article-types" ;
    rdfs:comment "The :ArticleType class represents the various kinds of publication which can be used to index and group (Macmillan) content published by Springer Nature. The instances of :ArticleType are organised hierarchically using the SKOS vocabulary."@en ;
    rdfs:isDefinedBy ns1: ;
    rdfs:subClassOf ns1:Concept .

ns1:BookEdition a owl:Class ;
    rdfs:label "Class: Book edition"@en ;
    ns1:namespace "book-editions" ;
    rdfs:comment "The :BookEdition class represents a non-serial work, or monograph, which gathers together separate physical book renditions."@en ;
    rdfs:isDefinedBy ns1: ;
    rdfs:subClassOf ns1:Monograph .

ns1:BookSeries a owl:Class ;
    rdfs:label "Class: Book series"@en ;
    ns1:namespace "book-series" ;
    rdfs:comment "The :BookSeries class represents a sequence of books having certain characteristics in common that are formally identified together as a group."@en ;
    rdfs:isDefinedBy ns1: ;
    rdfs:subClassOf ns1:Serial .

ns1:CitationMetricsEvent a owl:Class ;
    rdfs:label "Class: Citation metrics event"@en ;
    ns1:namespace "citation-metrics-events" ;
    rdfs:comment "The :CitationMetricsEvent class represents an event which annotates a thing with citation metrics information."@en ;
    rdfs:isDefinedBy ns1: ;
    rdfs:subClassOf ns1:MetricsEvent .

ns1:ConferenceSeries a owl:Class ;
    rdfs:label "Class: Conference series"@en ;
    ns1:namespace "conference-series" ;
    rdfs:comment "The :ConferenceSeries class refers to a set of scholarly conference events organized in a common format or under a common title or theme."@en ;
    rdfs:isDefinedBy ns1: ;
    rdfs:subClassOf ns1:Concept .

ns1:Contract a owl:Class ;
    rdfs:label "Class: Contract"@en ;
    ns1:namespace "contracts" ;
    rdfs:comment "The :Contract class represents a legal agreement."@en ;
    rdfs:isDefinedBy ns1: ;
    rdfs:subClassOf ns1:Intangible .

ns1:FieldOfResearchCode a owl:Class ;
    rdfs:label "Class: Field of Research (FOR) code"@en ;
    ns1:namespace "field-of-research-codes" ;
    rdfs:comment "The :FieldOfResearchCode class represents an Australian and New Zealand Standard Research Classification (ANZSRC) Field of Research (FOR) code which can be used to categorise the contents of a publication. The instances of :FieldOfResearchCode are organised hierarchically using the SKOS vocabulary."@en ;
    rdfs:isDefinedBy ns1: ;
    rdfs:subClassOf ns1:Category .

ns1:Monograph a owl:Class ;
    rdfs:label "Class: Monograph"@en ;
    ns1:namespace "monographs" ;
    rdfs:comment "The :Monograph class represents publications which appear separately in a new edition. For example, a book-edition."@en ;
    rdfs:isDefinedBy ns1: ;
    rdfs:subClassOf ns1:Work .

ns1:ProductMarketCode a owl:Class ;
    rdfs:label "Class: Product market code"@en ;
    ns1:namespace "product-market-codes" ;
    rdfs:comment "The :ProductMarketCode class represents a ..."@en ;
    rdfs:isDefinedBy ns1: ;
    rdfs:subClassOf ns1:Concept .

ns1:PublishState a owl:Class ;
    rdfs:label "Class: Publish state"@en ;
    ns1:namespace "publish-states" ;
    rdfs:comment "The :PublishState class provides a categorisation of the possible states a document may have after it has been published. For example, whether it’s an 'Advanced online publication' or an 'Issue publication'.  This categorisation is implemented as a SKOS vocabulary."@en ;
    rdfs:isDefinedBy ns1: ;
    rdfs:subClassOf ns1:PublicationState .

ns1:ReviewState a owl:Class ;
    rdfs:label "Class: Review state"@en ;
    ns1:namespace "review-states" ;
    rdfs:comment "The :ReviewState class provides a categorisation of the possible states a document may have as a result of a reviewing process. For example, whether it’s been 'Received' or 'Accepted'.  This categorisation is implemented as a SKOS vocabulary."@en ;
    rdfs:isDefinedBy ns1: ;
    rdfs:subClassOf ns1:PublicationState .

ns1:TechnicalArticleType a owl:Class ;
    rdfs:label "Class: Technical article type"@en ;
    ns1:namespace "technical-article-types" ;
    rdfs:comment "The :TechnicalArticleType class represents the various technical kinds of publication which can be used to index and group content published by Springer Nature. These types are used in the A++ XML. The instances of :TechnicalArticleType are organised non-hierarchically using the SKOS vocabulary."@en ;
    rdfs:isDefinedBy ns1: ;
    rdfs:subClassOf ns1:Concept .

ns1:conceptScheme a rdf:Property,
        owl:AnnotationProperty ;
    rdfs:label "Property: concept scheme"@en ;
    rdfs:comment "The :conceptScheme property specifies the SKOS concept scheme used in creating instances of this class."@en ;
    rdfs:isDefinedBy ns1: ;
    rdfs:subPropertyOf ns1:conceptScheme .

ns1:example a rdf:Property,
        owl:AnnotationProperty ;
    rdfs:label "Property: example"@en ;
    rdfs:comment "The :example property specifies an example of an entity. This property is similar to void:exampleResource. But see also skos:example."@en ;
    rdfs:isDefinedBy ns1: ;
    rdfs:seeAlso void:exampleResource ;
    rdfs:subPropertyOf ns1:example .

ns1:hasAffiliation a owl:ObjectProperty ;
    rdfs:label "Property: has affiliation" ;
    rdfs:comment "The :hasAffiliation property specifies the affiliation details of an agent, as it appears in the context of a publication contribution. Note that in most cases this information is non disambiguated or incomplete e.g. we may have an affiliation name but not an identifier."@en ;
    rdfs:domain ns1:Contribution ;
    rdfs:isDefinedBy ns1: ;
    rdfs:range ns1:Affiliation .

ns1:hasArticle a owl:ObjectProperty ;
    rdfs:label "Property: has article"@en ;
    rdfs:comment "The :hasArticle property relates a publication-event to an article."@en ;
    rdfs:domain ns1:PublicationEvent ;
    rdfs:isDefinedBy ns1: ;
    rdfs:range ns1:Article .

ns1:hasArticleType a owl:ObjectProperty ;
    rdfs:label "Property: has article-type"@en ;
    rdfs:comment "The :hasArticleType relates an article to an article-type."@en ;
    rdfs:domain ns1:Article ;
    rdfs:isDefinedBy ns1: ;
    rdfs:range ns1:ArticleType .

ns1:hasBook a owl:ObjectProperty ;
    rdfs:label "Property: has book"@en ;
    rdfs:comment "The :hasBook property relates a chapter to a book which contains it."@en ;
    rdfs:domain ns1:BookChapter ;
    rdfs:isDefinedBy ns1: ;
    rdfs:range ns1:Book .

ns1:hasBookChapter a owl:ObjectProperty ;
    rdfs:label "Property: has book chapter"@en ;
    rdfs:comment "The :hasBookChapter property relates a book to a chapter contained within it."@en ;
    rdfs:domain ns1:Book ;
    rdfs:isDefinedBy ns1: ;
    rdfs:range ns1:BookChapter .

ns1:hasBookEdition a owl:ObjectProperty ;
    rdfs:label "Property: has book edition"@en ;
    rdfs:comment "The :hasBookEdition property relates a publication (e.g. a book or book chapter) to the book edition which it belongs to."@en ;
    rdfs:domain ns1:Publication ;
    rdfs:isDefinedBy ns1: ;
    rdfs:range ns1:BookEdition .

ns1:hasBookSeries a owl:ObjectProperty ;
    rdfs:label "Property: has book series"@en ;
    rdfs:comment "The :hasBookSeries property relates a book to the book series in which it appears."@en ;
    rdfs:domain ns1:Book ;
    rdfs:isDefinedBy ns1: ;
    rdfs:range ns1:BookSeries .

ns1:hasConferenceSeries a owl:ObjectProperty ;
    rdfs:label "Property: has conference series"@en ;
    rdfs:comment "The :hasConferenceSeries property relates a conference to its series."@en ;
    rdfs:domain ns1:Conference ;
    rdfs:isDefinedBy ns1: ;
    rdfs:range ns1:ConferenceSeries .

ns1:hasContribution a owl:ObjectProperty ;
    rdfs:label "Property: has contribution"@en ;
    rdfs:comment "The :hasContribution property relates a Scigraph entity to a contributor-event that specifies the role an agent has in the context of the history of that entity. For example, a person could be the author, editor, reviewer of different publications at different times."@en ;
    rdfs:domain ns1:Thing ;
    rdfs:isDefinedBy ns1: ;
    rdfs:range ns1:Contribution .

ns1:hasFundedPublication a owl:ObjectProperty ;
    rdfs:label "Property: has funded publication"@en ;
    rdfs:comment "The :hasFundedPublication property specifies a publication produced as an outcome of a grant to a funded project."@en ;
    rdfs:domain ns1:Grant ;
    rdfs:isDefinedBy ns1: ;
    rdfs:range ns1:Publication .

ns1:hasFundingOrganization a owl:ObjectProperty ;
    rdfs:label "Property: has funding organization"@en ;
    rdfs:comment "The :hasFundingOrganization property specifies an organization that has funded a grant."@en ;
    rdfs:domain ns1:Grant ;
    rdfs:isDefinedBy ns1: ;
    rdfs:range ns1:Organization .

ns1:hasJournal a owl:ObjectProperty ;
    rdfs:label "Property: has journal"@en ;
    rdfs:comment "The :hasJournal property relates a publication to a journal."@en ;
    rdfs:isDefinedBy ns1: ;
    rdfs:range ns1:Journal .

ns1:hasJournalBrand a owl:ObjectProperty ;
    rdfs:label "Property: has journal brand"@en ;
    rdfs:comment "The :hasJournalBrand property relates a publication to a journal brand."@en ;
    rdfs:isDefinedBy ns1: ;
    rdfs:range ns1:JournalBrand .

ns1:hasOrganization a owl:ObjectProperty ;
    rdfs:label "Property: has organization"@en ;
    rdfs:comment "The :hasOrganization property specifies an organization related to an event or one of its subclasses."@en ;
    rdfs:domain ns1:Event ;
    rdfs:isDefinedBy ns1: ;
    rdfs:range ns1:Organization ;
    rdfs:subPropertyOf ns1:hasAgent .

ns1:hasPerson a owl:ObjectProperty ;
    rdfs:label "Property: has person"@en ;
    rdfs:comment "The :hasPerson property specifies a person related to an event or one of its subclasses. For example, the author of a :ContributionEvent. "@en ;
    rdfs:domain ns1:Event ;
    rdfs:isDefinedBy ns1: ;
    rdfs:range ns1:Person ;
    rdfs:subPropertyOf ns1:hasAgent .

ns1:hasProductMarketCode a owl:ObjectProperty ;
    rdfs:label "Property: has product-market-code"@en ;
    rdfs:comment "The :hasProductMarketCode property relates a product-market-code to a publication."@en ;
    rdfs:domain ns1:Publication ;
    rdfs:isDefinedBy ns1: ;
    rdfs:range ns1:ProductMarketCode ;
    rdfs:subPropertyOf ns1:hasCategory .

ns1:hasPublication a owl:ObjectProperty ;
    rdfs:label "Property: has publication"@en ;
    rdfs:comment "The :hasPublication property relates a publication-event to a publication."@en ;
    rdfs:domain ns1:PublicationEvent ;
    rdfs:isDefinedBy ns1: ;
    rdfs:range ns1:Publication .

ns1:hasPublishEvent a owl:ObjectProperty ;
    rdfs:label "Property: has publish event"@en ;
    rdfs:comment "The :hasPublishEvent property relates a publication to a publish-event that describes some recognized change in the status of a publication's publish history."@en ;
    rdfs:domain ns1:Publication ;
    rdfs:isDefinedBy ns1: ;
    rdfs:range ns1:PublishEvent .

ns1:hasPublishState a owl:ObjectProperty ;
    rdfs:label "Property: has publish state"@en ;
    rdfs:comment "The :hasPublishState property relates a publish-event to a publish-state that describes some recognized change in the status of a publication's publish history."@en ;
    rdfs:domain ns1:PublishEvent ;
    rdfs:isDefinedBy ns1: ;
    rdfs:range ns1:PublishState .

ns1:hasPublisher a owl:ObjectProperty ;
    rdfs:label "Property: has publisher"@en ;
    rdfs:comment "The :hasPublisher property relates a publication to the organization that publishes it."@en ;
    rdfs:domain ns1:Publication ;
    rdfs:isDefinedBy ns1: ;
    rdfs:range ns1:Publisher .

ns1:hasReviewEvent a owl:ObjectProperty ;
    rdfs:label "Property: has review event"@en ;
    rdfs:comment "The :hasReviewEvent property relates a publication to a review-event that describes some recognized change in the status of a publication's review history."@en ;
    rdfs:domain ns1:Publication ;
    rdfs:isDefinedBy ns1: ;
    rdfs:range ns1:ReviewEvent .

ns1:hasReviewState a owl:ObjectProperty ;
    rdfs:label "Property: has review state"@en ;
    rdfs:comment "The :hasReviewState property relates a review-event to a review-state that describes some recognized change in the status of a publication's review history."@en ;
    rdfs:domain ns1:ReviewEvent ;
    rdfs:isDefinedBy ns1: ;
    rdfs:range ns1:ReviewState .

ns1:hasRoot a owl:ObjectProperty ;
    rdfs:label "Property: has root"@en ;
    rdfs:comment "The :hasRoot property relates a :Concept instance to a toplevel :Concept instance within the same domain model."@en ;
    rdfs:domain ns1:Concept ;
    rdfs:isDefinedBy ns1: ;
    rdfs:range ns1:Concept .

ns1:hasSerial a owl:ObjectProperty ;
    rdfs:label "Property: has serial"@en ;
    rdfs:comment "The :hasSerial property relates a publication to a serial."@en ;
    rdfs:domain ns1:Publication ;
    rdfs:isDefinedBy ns1: ;
    rdfs:range ns1:Serial .

ns1:hasWork a owl:ObjectProperty ;
    rdfs:label "Property: has work"@en ;
    rdfs:comment "The :hasWork property relates a product to an abstract work from which it derives, or which contains it."@en ;
    rdfs:domain ns1:Product ;
    rdfs:isDefinedBy ns1: ;
    rdfs:range ns1:Work .

ns1:keyProperty a rdf:Property,
        owl:AnnotationProperty ;
    rdfs:label "Property: key property"@en ;
    rdfs:comment "The :keyProperty property specifies which are the properties used to unambiguously identify an entity type."@en ;
    rdfs:isDefinedBy ns1: ;
    rdfs:subPropertyOf ns1:keyProperty .

ns1:namespace a rdf:Property,
        owl:AnnotationProperty ;
    rdfs:label "Property: namespace"@en ;
    rdfs:comment "The :namespace property provides the RDF namespace used in creating instances of a class."@en ;
    rdfs:isDefinedBy ns1: ;
    rdfs:subPropertyOf ns1:namespace .

ns1:otherWebpage a rdf:Property,
        owl:ObjectProperty ;
    rdfs:label "Property: other web page"@en ;
    rdfs:comment "The :otherWebpage property relates a Scigraph thing to a generic page on the web."@en ;
    rdfs:domain ns1:Thing ;
    rdfs:isDefinedBy ns1: ;
    rdfs:subPropertyOf ns1:otherWebpage .

ns1:replacedBy a owl:ObjectProperty ;
    rdfs:label "Property: replaced by"@en ;
    rdfs:comment "The :replacedBy property relates a thing to another thing that replaces it."@en ;
    rdfs:isDefinedBy ns1: ;
    owl:inverseOf ns1:replaces .

ns1:replaces a owl:ObjectProperty ;
    rdfs:label "Property: replaces"@en ;
    rdfs:comment "The :replaces property relates a thing to another thing that it replaces."@en ;
    rdfs:isDefinedBy ns1: ;
    owl:inverseOf ns1:replacedBy .

ns1:shapeDataClient a rdf:Property,
        owl:AnnotationProperty ;
    rdfs:label "Property: shape data client"@en ;
    rdfs:comment "The :shapeDataClient property specifies the data client that a SHACL shape is prepared for. The client may be a data source for imports, or a data sink for exports. See :shapeType for the shape data flow direction. Note that the client may be specified currently as a string, although later is intended to reference a data-clients: taxonomy term."@en ;
    rdfs:isDefinedBy ns1: ;
    rdfs:subPropertyOf ns1:shapeDataClient .

ns1:shapeDataGraph a rdf:Property,
        owl:AnnotationProperty ;
    rdfs:label "Property: shape data graph"@en ;
    rdfs:comment "The :shapeDataGraph property specifies the data graph that a SHACL shape will be applied to."@en ;
    rdfs:isDefinedBy ns1: ;
    rdfs:subPropertyOf ns1:shapeDataGraph .

ns1:shapeType a rdf:Property,
        owl:AnnotationProperty ;
    rdfs:label "Property: shape type"@en ;
    rdfs:comment "The :shapeType property specifies whether a SHACL shape is used primarily for data ingestion (\"import\") or for data publishing ()\"export\")."@en ;
    rdfs:isDefinedBy ns1: ;
    rdfs:subPropertyOf ns1:shapeType .

ns1:webpage a rdf:Property,
        owl:ObjectProperty ;
    rdfs:label "Property: web page"@en ;
    rdfs:comment "The :webpage property relates a Scigraph thing to a page on the web that describes it."@en ;
    rdfs:domain ns1:Thing ;
    rdfs:isDefinedBy ns1: ;
    rdfs:subPropertyOf ns1:webpage .

ns1:BookChapter a owl:Class ;
    rdfs:label "Class: Book chapter"@en ;
    ns1:namespace "book-chapters" ;
    rdfs:comment "The :BookChapter class represents a defined chapter of a book, usually with a separate title or number."@en ;
    rdfs:isDefinedBy ns1: ;
    rdfs:subClassOf ns1:Product .

ns1:Conference a owl:Class ;
    rdfs:label "Class: Conference"@en ;
    ns1:namespace "conferences" ;
    rdfs:comment "The :Conference represents a formal meeting of people with a shared interest, typically one that takes place over several days."@en ;
    rdfs:isDefinedBy ns1: ;
    rdfs:subClassOf ns1:Event .

ns1:Journal a owl:Class ;
    rdfs:label "Class: Journal"@en ;
    ns1:namespace "journals" ;
    rdfs:comment "The :Journal class represents a scholarly serial publication which is realized as a product publication in a particular medium (print, online, or CD-ROM)."@en ;
    rdfs:isDefinedBy ns1: ;
    rdfs:subClassOf ns1:Product .

ns1:JournalBrand a owl:Class ;
    rdfs:label "Class: Journal brand"@en ;
    ns1:namespace "journal-brands" ;
    rdfs:comment "The :JournalBrand class represents a scholarly serial publication, considered from both the scholarly and the commercial perspectives. Thus a journal brand is more than the sum of its product publications; it is an entity characterised by many properties, e.g. its founders, its impact factor, etc."@en ;
    rdfs:isDefinedBy ns1: ;
    rdfs:subClassOf ns1:Serial .

ns1:PublicationState a owl:Class ;
    rdfs:label "Class: Publication state"@en ;
    ns1:namespace "publication-states" ;
    rdfs:comment "The :PublicationState class groups together publish-state and review-state individuals."@en ;
    rdfs:isDefinedBy ns1: ;
    rdfs:subClassOf ns1:Concept .

ns1:PublishEvent a owl:Class ;
    rdfs:label "Class: Publish event"@en ;
    ns1:namespace "publish-events" ;
    rdfs:comment "The :PublishEvent class represents events related to the publication of a document. This is intended in a strict sense, i.e. the time when a publication is made 'public'. In order to differentiate these events further, the :PublishState vocabulary is used."@en ;
    rdfs:isDefinedBy ns1: ;
    rdfs:subClassOf ns1:PublicationEvent .

ns1:ReviewEvent a owl:Class ;
    rdfs:label "Class: Review event"@en ;
    ns1:namespace "review-events" ;
    rdfs:comment "The :ReviewEvent class models events related to the reviewing of a document (before its publication). In order to differentiate these events further, the :ReviewState vocabulary is used."@en ;
    rdfs:isDefinedBy ns1: ;
    rdfs:subClassOf ns1:PublicationEvent .

ns1:count a owl:DatatypeProperty ;
    rdfs:label "Property: count"@en ;
    rdfs:comment "The :count property specifies a count value."@en ;
    rdfs:isDefinedBy ns1: ;
    rdfs:range xsd:integer .

ns1:hasMetricsEvent a owl:ObjectProperty ;
    rdfs:label "Property: has metrics event"@en ;
    rdfs:comment "The :hasMetricsEvent property specifies a resource which identifies a metrics event for a publication."@en ;
    rdfs:domain ns1:Publication ;
    rdfs:isDefinedBy ns1: ;
    rdfs:range ns1:MetricsEvent .

ns1:hasSubject a rdf:Property,
        owl:ObjectProperty ;
    rdfs:label "Property: has subject"@en ;
    rdfs:comment "The :hasSubject property relates a publication to a subject term which describes one of the main topics the publication is about."@en ;
    rdfs:domain ns1:Publication ;
    rdfs:isDefinedBy ns1: ;
    rdfs:range ns1:Subject ;
    rdfs:subPropertyOf ns1:hasCategory,
        ns1:hasSubject .

ns1:isAgentOf a owl:ObjectProperty ;
    rdfs:label "Property: is agent of"@en ;
    rdfs:comment "The :isAgentOf property is the inverse of the :hasAgent property."@en ;
    rdfs:isDefinedBy ns1: ;
    owl:inverseOf ns1:hasAgent .

ns1:issn a owl:DatatypeProperty ;
    rdfs:label "Property: ISSN" ;
    rdfs:comment "The :issn property specifies an ISSN number for a serial."@en ;
    rdfs:domain ns1:Publication ;
    rdfs:isDefinedBy ns1: ;
    rdfs:range xsd:string .

ns1:placeInfo a owl:DatatypeProperty ;
    rdfs:label "Property: place info"@en ;
    rdfs:comment "The :placeInfo property is used for grouping all properties describing the location of a thing."@en ;
    rdfs:isDefinedBy ns1: ;
    rdfs:range xsd:string .

ns1:publicationDate a owl:DatatypeProperty ;
    rdfs:label "Property: publication date"@en ;
    rdfs:comment "The :publicationDate property specifies the first known full date of a publication, either in electronic form or print, as a string."@en ;
    rdfs:domain ns1:Publication ;
    rdfs:isDefinedBy ns1: ;
    rdfs:range xsd:date ;
    rdfs:subPropertyOf ns1:dateInfo .

ns1:publicationNumber a owl:DatatypeProperty ;
    rdfs:label "Property: publication number"@en ;
    rdfs:comment "The :publicationNumber property specifies the number of the publication as a string value. Note: this property is used primarily for grouping purposes. "@en ;
    rdfs:domain ns1:Publication ;
    rdfs:isDefinedBy ns1: ;
    rdfs:range xsd:string .

ns1:Book a owl:Class ;
    rdfs:label "Class: Book"@en ;
    ns1:namespace "books" ;
    rdfs:comment "The :Book class represents a non-serial document that is complete in one volume or a designated finite number of volumes. A book may be manifested as a physical printed publication in hard or soft cover form, or in digital format as an 'e-book'."@en ;
    rdfs:isDefinedBy ns1: ;
    rdfs:subClassOf ns1:Product .

ns1:Category a owl:Class ;
    rdfs:label "Class: Category"@en ;
    ns1:namespace "categories" ;
    rdfs:comment "The :Category class represents a topic, field of study or research area which can be used to categorise the contents of a publication. More specific categorization classes may be used."@en ;
    rdfs:isDefinedBy ns1: ;
    rdfs:subClassOf ns1:Concept .

ns1:Serial a owl:Class ;
    rdfs:label "Class: Serial"@en ;
    ns1:namespace "serials" ;
    rdfs:comment "The :Serial class represents publications which appear in a new edition on a regular schedule. For example, a journal, a magazine or a blog. The :PublishEvent class is used to provide more details about the time, place and other contextual information relevant to when a new edition gets published."@en ;
    rdfs:isDefinedBy ns1: ;
    rdfs:subClassOf ns1:Work .

ns1:Subject a owl:Class ;
    rdfs:label "Class: Subject"@en ;
    ns1:namespace "subjects" ;
    rdfs:comment "The :Subject class represents a Springer Nature topic, field of study or research area which can be used to categorise the contents of a publication. The instances of :Subject are organised hierarchically using the SKOS vocabulary."@en ;
    rdfs:isDefinedBy ns1: ;
    rdfs:subClassOf ns1:Category .

ns1:rights a owl:DatatypeProperty ;
    rdfs:label "Property: rights"@en ;
    rdfs:comment "The :rights property is not intended to be used directly but is supplied to group together, and facilitate querying of, various rights attributes, such as  copyright and access rights."@en ;
    rdfs:domain ns1:Publication ;
    rdfs:isDefinedBy ns1: ;
    rdfs:range rdfs:Literal .

ns1:Agent a owl:Class ;
    rdfs:label "Class: Agent"@en ;
    ns1:namespace "agents" ;
    rdfs:comment "The :Agent class groups together all entities that can be the subject of an action. These can be single persons (:Person), or groups of people organised as a legal entity (:Organization)."@en ;
    rdfs:isDefinedBy ns1: ;
    rdfs:subClassOf ns1:Thing .

ns1:Contribution a owl:Class ;
    rdfs:label "Class: Contribution"@en ;
    ns1:namespace "contributions" ;
    rdfs:comment "The :Contribution class represents events related to the making of a Scigraph entity, from the point of view of its authors, editors, or any other :Agent involved in the creation of the work."@en ;
    rdfs:isDefinedBy ns1: ;
    rdfs:subClassOf ns1:Event .

ns1:Intangible a owl:Class ;
    rdfs:label "Class: Intangible"@en ;
    ns1:namespace "intangibles" ;
    rdfs:comment "The :Intangible class groups together all individuals which do not exist in the physical world (i.e. have no extension in spacetime)."@en ;
    rdfs:isDefinedBy ns1: ;
    rdfs:subClassOf ns1:Thing .

ns1:Organization a owl:Class ;
    rdfs:label "Class: Organization"@en ;
    ns1:namespace "organizations" ;
    rdfs:comment "The :Organization class represents an organised body of people normally having a legal status."@en ;
    rdfs:isDefinedBy ns1: ;
    rdfs:subClassOf ns1:Agent .

ns1:Person a owl:Class ;
    rdfs:label "Class: Person"@en ;
    ns1:namespace "persons" ;
    rdfs:comment "The :Person class represents a single person entity."@en ;
    rdfs:isDefinedBy ns1: ;
    rdfs:subClassOf ns1:Agent .

ns1:PublicationEvent a owl:Class ;
    rdfs:label "Class: Publication event"@en ;
    ns1:namespace "publication-events" ;
    rdfs:comment "The :PublicationEvent class groups together events that happen within the publishing process, broadly conceived. For example, the submission of an article, or the acceptance of a paper."@en ;
    rdfs:isDefinedBy ns1: ;
    rdfs:subClassOf ns1:Event .

ns1:Work a owl:Class ;
    rdfs:label "Class: Work"@en ;
    ns1:namespace "works" ;
    rdfs:comment "The :Work class groups together all individuals (or part of) created as the result of the publishing process. Note that we are not referring here to the physical artefacts, but just their abstract counterparts."@en ;
    rdfs:isDefinedBy ns1: ;
    rdfs:subClassOf ns1:Publication .

ns1:hasCategory a owl:ObjectProperty ;
    rdfs:label "Property: has category"@en ;
    rdfs:comment "The :hasCategory property relates a category to a publication."@en ;
    rdfs:domain ns1:Publication ;
    rdfs:isDefinedBy ns1: ;
    rdfs:range rdfs:Resource .

ns1:Article a owl:Class ;
    rdfs:label "Class: Article"@en ;
    ns1:namespace "articles" ;
    rdfs:comment "The :Article class represents a scholarly work normally published as an item of a serial publication. In particular, this concept refers to the abstract notion of an article, rather than any of its realisations after it becomes embodied via a physical medium. With reference to the FRBR model [http://www.ifla.org/publications/functional-requirements-for-bibliographic-records], an :Article can be mapped directly to the frbr:Expression concept. It is worth noting though that within the Scigraph Core Ontology we do not have any notion of a frbr:Work. Hence multiple versions of the same article (e.g. language translations, or revisions) are characterised as such simply by means of some relationship."@en ;
    rdfs:isDefinedBy ns1: ;
    rdfs:subClassOf ns1:Product .

ns1:Grant a owl:Class ;
    rdfs:label "Class: Grant"@en ;
    ns1:namespace "grants" ;
    rdfs:comment "The :Grant class represents a funding award for a research project as a contract."@en ;
    rdfs:isDefinedBy ns1: ;
    rdfs:subClassOf ns1:Contract .

ns1:accessRights a owl:DatatypeProperty ;
    rdfs:label "Property: accessRights"@en ;
    rdfs:comment "The :accessRights property specifies an access right to a publication (or part of it) as a string value."@en ;
    rdfs:domain ns1:Publication ;
    rdfs:isDefinedBy ns1: ;
    rdfs:range xsd:string ;
    rdfs:subPropertyOf ns1:rights .

ns1:hasAgent a owl:ObjectProperty ;
    rdfs:label "Property: has agent"@en ;
    rdfs:comment "The :hasAgent property specifies an agent related to an event or one of its subclasses. Note: this property is abstract as it is mainly used for grouping sub-properties like sg:hasPerson."@en ;
    rdfs:domain ns1:Event ;
    rdfs:isDefinedBy ns1: ;
    rdfs:range ns1:Agent .

ns1:MetricsEvent a owl:Class ;
    rdfs:label "Class: Metrics event"@en ;
    ns1:namespace "metrics-events" ;
    rdfs:comment "The :MetricsEvent class represents an event which annotates a thing with metrics information."@en ;
    rdfs:isDefinedBy ns1: ;
    rdfs:subClassOf ns1:AnnotationEvent .

ns1:Product a owl:Class ;
    rdfs:label "Class: Product"@en ;
    ns1:namespace "products" ;
    rdfs:comment "The :Product class groups together all publications which were created to be distributed and consumed as individual, self-contained entities."@en ;
    rdfs:isDefinedBy ns1: ;
    rdfs:subClassOf ns1:Publication .

ns1:id a owl:DatatypeProperty ;
    rdfs:label "Property: ID"@en ;
    rdfs:comment "The :id property provides a root property for all Scigraph identity properties."@en ;
    rdfs:domain ns1:Thing ;
    rdfs:isDefinedBy ns1: ;
    rdfs:range xsd:string .

ns1:AnnotationEvent a owl:Class ;
    rdfs:label "Class: Annotation event"@en ;
    ns1:namespace "annotation-events" ;
    rdfs:comment "The :AnnotationEvent class groups together all events describing the process of adding notes or marking up a thing."@en ;
    rdfs:isDefinedBy ns1: ;
    rdfs:subClassOf ns1:Event .

ns1:label a owl:DatatypeProperty ;
    rdfs:label "Property: label"@en ;
    rdfs:comment "The :label property specifies a label for a thing as a string value."@en ;
    rdfs:domain ns1:Thing ;
    rdfs:isDefinedBy ns1: ;
    rdfs:range xsd:string .

ns1:Concept a owl:Class ;
    rdfs:label "Class: Concept"@en ;
    ns1:namespace "concepts" ;
    rdfs:comment "The :Concept class groups together  all domain-specific categorisations relevant to the Springer Nature publishing world. All of the :Concept categorisations are implemented as self-contained reusable SKOS vocabularies (although not all of them are taxonomies in the strict sense of hierarchical vocabularies)."@en ;
    rdfs:isDefinedBy ns1: ;
    rdfs:subClassOf ns1:Intangible .

ns1:dateInfo a owl:DatatypeProperty ;
    rdfs:label "Property: dateInfo"@en ;
    rdfs:comment "The :dateInfo property is an abstract property used to group together all date-related properties."@en ;
    rdfs:isDefinedBy ns1: .

ns1:Event a owl:Class ;
    rdfs:label "Class: Event"@en ;
    ns1:namespace "events" ;
    rdfs:comment "The :Event class groups together events of varying granularity. Events differ from :Intangible entities because they have an extension in time; they differ from :Tangible entities because they do not have an extension in space."@en ;
    rdfs:isDefinedBy ns1: ;
    rdfs:subClassOf ns1:Thing .

ns1:nameInfo a owl:DatatypeProperty ;
    rdfs:label "Property: name info"@en ;
    rdfs:comment "The :nameInfo property is used for grouping all properties describing names, titles or labels for an object."@en ;
    rdfs:domain ns1:Thing ;
    rdfs:isDefinedBy ns1: .

ns1:Thing a owl:Class ;
    rdfs:label "Class: Thing"@en ;
    ns1:namespace "things" ;
    rdfs:comment "The :Thing class groups together all individuals used by Springer Nature within the Springer Nature publishing world."@en ;
    rdfs:isDefinedBy ns1: ;
    rdfs:subClassOf owl:Thing .

ns1:Publication a owl:Class ;
    rdfs:label "Class: Publication"@en ;
    ns1:namespace "publications" ;
    rdfs:comment "The :Publication class groups together all individuals (or part of) created as the result of the publishing process. Note that we are not referring here to the physical artefacts, but just their abstract counterparts."@en ;
    rdfs:isDefinedBy ns1: ;
    rdfs:subClassOf ns1:Intangible .

ns1: a owl:Ontology ;
    rdfs:label "Springer Nature SciGraph Core Ontology"@en ;
    dc:creator "Michele Pasin <mailto:michele.pasin@springernature.com>",
        "Tony Hammond <mailto:tony.hammond@springernature.com>" ;
    dc:publisher "Springer Nature" ;
    dc:rights "This work is distributed under a Creative Commons Attribution-NonCommercial 4.0 International (CC BY-NC 4.0) Public License <https://creativecommons.org/licenses/by-nc/4.0/>."@en ;
    ns2:license <https://creativecommons.org/licenses/by-nc/4.0/> ;
    vann:preferredNamespacePrefix "sg" ;
    vann:preferredNamespaceUri "http://scigraph.springernature.com/ontologies/core/" ;
    ns1:webpage <http://scigraph.springernature.com> ;
    rdfs:comment "The Springer Nature SciGraph Core Ontology is a formal model providing definitions for the key concepts of interest to content publishing at Springer Nature."@en ;
    rdfs:isDefinedBy ns1: ;
    owl:versionInfo "1.2.0" .


